chore: update stage0

stage0/stdlib/Init/Tactics.c
@@ -72,6 +72,7 @@ static lean_object* l_Lean_Parser_Tactic_first___closed__9;
 static lean_object* l_Lean_Parser_Tactic_induction___closed__12;
 LEAN_EXPORT lean_object* l_Lean_Parser_Tactic_tacticRfl;
 static lean_object* l_Lean_Parser_Tactic_generalize___closed__2;
+static lean_object* l_Lean_Parser_Tactic___aux__Init__Tactics______macroRules__Lean__Parser__Tactic__tacticNext___x3d_x3e____1___closed__7;
 LEAN_EXPORT lean_object* l_Lean_Parser_Tactic_rwSeq;
 LEAN_EXPORT lean_object* l_Lean_Parser_Tactic_traceMessage;
 static lean_object* l_Lean_Parser_Tactic_config___closed__8;
@@ -81,7 +82,6 @@ static lean_object* l_Lean_Parser_Tactic_acRfl___closed__4;
 static lean_object* l_Lean_Parser_Tactic_intro___closed__9;
 static lean_object* l_Lean_Parser_Tactic___aux__Init__Tactics______macroRules__Lean__Parser__Tactic__tacticTrivial__6___closed__7;
 static lean_object* l_Lean_Parser_Tactic_revert___closed__9;
-static lean_object* l_Lean_Parser_Tactic_inductionAlt___closed__19;
 LEAN_EXPORT lean_object* l_Lean_Parser_Tactic___aux__Init__Tactics______macroRules__Lean__Parser__Tactic__tacticHave_x27____1(lean_object*, lean_object*, lean_object*);
 static lean_object* l_Lean_Parser_Tactic_failIfSuccess___closed__6;
 static lean_object* l_Lean_Parser_Tactic_delta___closed__1;
@@ -169,7 +169,6 @@ static lean_object* l_Lean_Parser_Tactic_rotateRight___closed__4;
 LEAN_EXPORT lean_object* l_Lean_Parser_Tactic_inductionAlts;
 static lean_object* l_Lean_Parser_Tactic___aux__Init__Tactics______macroRules__Lean__Parser__Tactic__tacticHave____1___closed__1;
 static lean_object* l_Lean_Parser_Tactic_rename___closed__3;
-static lean_object* l_Lean_Parser_Tactic___aux__Init__Tactics______macroRules__Lean__Parser__Tactic__tacticAdmit__1___closed__21;
 LEAN_EXPORT lean_object* l_Lean_Parser_Tactic___aux__Init__Tactics______macroRules__Lean__Parser__Tactic__tacticHave____1(lean_object*, lean_object*, lean_object*);
 static lean_object* l_Lean_Parser_Tactic_withUnfoldingAll___closed__5;
 static lean_object* l_Lean_Parser_Tactic_specialize___closed__6;
@@ -209,11 +208,13 @@ LEAN_EXPORT lean_object* l_Lean_Parser_Tactic_tacticUnhygienic__;
 static lean_object* l_Lean_Parser_Tactic_generalizeArg___closed__1;
 static lean_object* l_Lean_Parser_Tactic_inductionAlt___closed__4;
 LEAN_EXPORT lean_object* l_Lean_Parser_Tactic_inductionAlt;
+static lean_object* l_Lean_binderIdent___closed__14;
 static lean_object* l_Lean_Parser_Tactic_dsimp___closed__9;
 LEAN_EXPORT lean_object* l_Lean_Parser_Tactic___aux__Init__Tactics______macroRules__Lean__Parser__Tactic__tacticExists___x2c_x2c__1(lean_object*, lean_object*, lean_object*);
 static lean_object* l_Lean_Parser_Tactic_tacticTrivial___closed__4;
 static lean_object* l_Lean_Parser_Tactic_case___closed__11;
 static lean_object* l_Lean_binderIdent___closed__5;
+static lean_object* l_Lean_Parser_Tactic___aux__Init__Tactics______macroRules__Lean__Parser__Tactic__tacticNext___x3d_x3e____1___closed__9;
 static lean_object* l_Lean_Parser_Tactic_tacticLet_____closed__4;
 static lean_object* l_Lean_Parser_Tactic_unfold___closed__8;
 static lean_object* l_Lean_Parser_Tactic_refl___closed__4;
@@ -289,6 +290,7 @@ static lean_object* l_Lean_Parser_Tactic_tacticHave_x27_____closed__6;
 static lean_object* l_Lean_Parser_Tactic_revert___closed__4;
 static lean_object* l_Lean_Parser_Tactic_rwRule___closed__6;
 static lean_object* l_Lean_Parser_Tactic___aux__Init__Tactics______macroRules__Lean__Parser__Tactic__tacticHave____1___closed__3;
+static lean_object* l_Lean_Parser_Tactic___aux__Init__Tactics______macroRules__Lean__Parser__Tactic__tacticNext___x3d_x3e____1___closed__8;
 static lean_object* l_Lean_Parser_Tactic_location___closed__5;
 static lean_object* l_Lean_Parser_Tactic_tacticLet_____closed__9;
 static lean_object* l___aux__Init__Tactics______macroRules__tacticGet__elem__tactic__trivial__2___closed__16;
@@ -416,7 +418,6 @@ static lean_object* l___aux__Init__Tactics______macroRules__term_____x5b___x5d_x
 static lean_object* l_Lean_Parser_Tactic_checkpoint___closed__5;
 static lean_object* l_Lean_Parser_Tactic_refine___closed__3;
 static lean_object* l_Lean_Parser_Tactic_induction___closed__16;
-static lean_object* l_Lean_Parser_Tactic___aux__Init__Tactics______macroRules__Lean__Parser__Tactic__tacticAdmit__1___closed__20;
 static lean_object* l_Lean_Parser_Tactic_withReducibleAndInstances___closed__2;
 LEAN_EXPORT lean_object* l_Lean_Parser_Tactic_cases;
 static lean_object* l_Lean_Parser_Tactic_traceMessage___closed__3;
@@ -511,7 +512,6 @@ LEAN_EXPORT lean_object* l_Lean_Parser_Tactic_simpStar;
 static lean_object* l_Lean_Parser_Tactic_revert___closed__5;
 static lean_object* l_Lean_Parser_Tactic___aux__Init__Tactics______macroRules__Lean__Parser__Tactic__tacticShow____1___closed__4;
 static lean_object* l_Lean_Parser_Tactic___aux__Init__Tactics______macroRules__Lean__Parser__Tactic__tacticInfer__instance__1___closed__3;
-static lean_object* l_Lean_Parser_Tactic___aux__Init__Tactics______macroRules__Lean__Parser__Tactic__tacticAdmit__1___closed__22;
 static lean_object* l_Lean_Parser_Tactic_tacticRfl___closed__3;
 static lean_object* l_Lean_Parser_Tactic_simpAll___closed__6;
 static lean_object* l_Lean_Parser_Tactic_split___closed__6;
@@ -617,7 +617,6 @@ static lean_object* l_Lean_Parser_Tactic___aux__Init__Tactics______macroRules__L
 static lean_object* l_Lean_Parser_Tactic_withAnnotateState___closed__14;
 static lean_object* l_Lean_Parser_Tactic_inductionAlt___closed__3;
 LEAN_EXPORT lean_object* l_Lean_Parser_Tactic_injections;
-static lean_object* l_Lean_Parser_Tactic_inductionAlt___closed__18;
 static lean_object* l_Lean_Parser_Tactic_intro___closed__7;
 static lean_object* l_Lean_Parser_Tactic_case_x27___closed__9;
 static lean_object* l_Lean_Parser_Tactic_inductionAlt___closed__15;
@@ -724,7 +723,6 @@ static lean_object* l_Lean_Parser_Tactic_tacticRfl_x27___closed__4;
 LEAN_EXPORT lean_object* l_Lean_Parser_Tactic_tacticLet__;
 static lean_object* l_Lean_Parser_Tactic_tacticRfl___closed__1;
 static lean_object* l_Lean_Parser_Tactic_intros___closed__4;
-static lean_object* l_Lean_Parser_Tactic___aux__Init__Tactics______macroRules__Lean__Parser__Tactic__tacticAdmit__1___closed__23;
 static lean_object* l_Lean_Parser_Tactic_change___closed__6;
 static lean_object* l_Lean_Parser_Tactic_tacticHave_x27___x3a_x3d_____closed__7;
 static lean_object* l_Lean_Parser_Tactic_tacticHave___x3a_x3d_____closed__1;
@@ -827,6 +825,7 @@ static lean_object* l_Lean_Parser_Tactic_unfold___closed__5;
 static lean_object* l_Lean_Parser_Tactic_inductionAlt___closed__17;
 static lean_object* l_Lean_Parser_Tactic_first___closed__5;
 static lean_object* l_Lean_Parser_Tactic_substVars___closed__3;
+static lean_object* l_Lean_Parser_Tactic___aux__Init__Tactics______macroRules__Lean__Parser__Tactic__tacticNext___x3d_x3e____1___closed__10;
 static lean_object* l_Lean_Parser_Tactic_case___closed__1;
 static lean_object* l_Lean_Parser_Tactic_tacticHave_____closed__1;
 lean_object* l_Lean_Syntax_getArgs(lean_object*);
@@ -1261,27 +1260,37 @@ static lean_object* _init_l_Lean_binderIdent___closed__10() {
 _start:
 {
 lean_object* x_1; 
-x_1 = lean_mk_string_from_bytes("_", 1);
+x_1 = lean_mk_string_from_bytes("hole", 4);
 return x_1;
 }
 }
 static lean_object* _init_l_Lean_binderIdent___closed__11() {
 _start:
 {
-lean_object* x_1; lean_object* x_2; 
-x_1 = l_Lean_binderIdent___closed__10;
-x_2 = lean_alloc_ctor(5, 1, 0);
-lean_ctor_set(x_2, 0, x_1);
-return x_2;
+lean_object* x_1; lean_object* x_2; lean_object* x_3; 
+x_1 = lean_box(0);
+x_2 = l_Lean_binderIdent___closed__10;
+x_3 = l_Lean_Name_str___override(x_1, x_2);
+return x_3;
 }
 }
 static lean_object* _init_l_Lean_binderIdent___closed__12() {
 _start:
 {
+lean_object* x_1; lean_object* x_2; 
+x_1 = l_Lean_binderIdent___closed__11;
+x_2 = lean_alloc_ctor(0, 1, 0);
+lean_ctor_set(x_2, 0, x_1);
+return x_2;
+}
+}
+static lean_object* _init_l_Lean_binderIdent___closed__13() {
+_start:
+{
 lean_object* x_1; lean_object* x_2; lean_object* x_3; lean_object* x_4; 
 x_1 = l_Lean_binderIdent___closed__6;
 x_2 = l_Lean_binderIdent___closed__9;
-x_3 = l_Lean_binderIdent___closed__11;
+x_3 = l_Lean_binderIdent___closed__12;
 x_4 = lean_alloc_ctor(2, 3, 0);
 lean_ctor_set(x_4, 0, x_1);
 lean_ctor_set(x_4, 1, x_2);
@@ -1289,13 +1298,13 @@ lean_ctor_set(x_4, 2, x_3);
 return x_4;
 }
 }
-static lean_object* _init_l_Lean_binderIdent___closed__13() {
+static lean_object* _init_l_Lean_binderIdent___closed__14() {
 _start:
 {
 lean_object* x_1; lean_object* x_2; lean_object* x_3; lean_object* x_4; 
 x_1 = l_Lean_binderIdent___closed__3;
 x_2 = l_Lean_binderIdent___closed__4;
-x_3 = l_Lean_binderIdent___closed__12;
+x_3 = l_Lean_binderIdent___closed__13;
 x_4 = lean_alloc_ctor(9, 3, 0);
 lean_ctor_set(x_4, 0, x_1);
 lean_ctor_set(x_4, 1, x_2);
@@ -1307,7 +1316,7 @@ static lean_object* _init_l_Lean_binderIdent() {
 _start:
 {
 lean_object* x_1; 
-x_1 = l_Lean_binderIdent___closed__13;
+x_1 = l_Lean_binderIdent___closed__14;
 return x_1;
 }
 }
@@ -1837,7 +1846,7 @@ _start:
 lean_object* x_1; lean_object* x_2; lean_object* x_3; lean_object* x_4; 
 x_1 = l_Lean_Parser_Tactic_withAnnotateState___closed__8;
 x_2 = l_Lean_Parser_Tactic_intro___closed__15;
-x_3 = l_Lean_binderIdent___closed__12;
+x_3 = l_Lean_binderIdent___closed__13;
 x_4 = lean_alloc_ctor(2, 3, 0);
 lean_ctor_set(x_4, 0, x_1);
 lean_ctor_set(x_4, 1, x_2);
@@ -3166,13 +3175,49 @@ return x_1;
 static lean_object* _init_l_Lean_Parser_Tactic___aux__Init__Tactics______macroRules__Lean__Parser__Tactic__tacticNext___x3d_x3e____1___closed__1() {
 _start:
 {
+lean_object* x_1; 
+x_1 = lean_mk_string_from_bytes("Term", 4);
+return x_1;
+}
+}
+static lean_object* _init_l_Lean_Parser_Tactic___aux__Init__Tactics______macroRules__Lean__Parser__Tactic__tacticNext___x3d_x3e____1___closed__2() {
+_start:
+{
+lean_object* x_1; lean_object* x_2; lean_object* x_3; 
+x_1 = l_Lean_Parser_Tactic_withAnnotateState___closed__2;
+x_2 = l_Lean_Parser_Tactic___aux__Init__Tactics______macroRules__Lean__Parser__Tactic__tacticNext___x3d_x3e____1___closed__1;
+x_3 = l_Lean_Name_str___override(x_1, x_2);
+return x_3;
+}
+}
+static lean_object* _init_l_Lean_Parser_Tactic___aux__Init__Tactics______macroRules__Lean__Parser__Tactic__tacticNext___x3d_x3e____1___closed__3() {
+_start:
+{
+lean_object* x_1; lean_object* x_2; lean_object* x_3; 
+x_1 = l_Lean_Parser_Tactic___aux__Init__Tactics______macroRules__Lean__Parser__Tactic__tacticNext___x3d_x3e____1___closed__2;
+x_2 = l_Lean_binderIdent___closed__10;
+x_3 = l_Lean_Name_str___override(x_1, x_2);
+return x_3;
+}
+}
+static lean_object* _init_l_Lean_Parser_Tactic___aux__Init__Tactics______macroRules__Lean__Parser__Tactic__tacticNext___x3d_x3e____1___closed__4() {
+_start:
+{
+lean_object* x_1; 
+x_1 = lean_mk_string_from_bytes("_", 1);
+return x_1;
+}
+}
+static lean_object* _init_l_Lean_Parser_Tactic___aux__Init__Tactics______macroRules__Lean__Parser__Tactic__tacticNext___x3d_x3e____1___closed__5() {
+_start:
+{
 lean_object* x_1; lean_object* x_2; 
 x_1 = lean_unsigned_to_nat(1u);
 x_2 = lean_mk_empty_array_with_capacity(x_1);
 return x_2;
 }
 }
-static lean_object* _init_l_Lean_Parser_Tactic___aux__Init__Tactics______macroRules__Lean__Parser__Tactic__tacticNext___x3d_x3e____1___closed__2() {
+static lean_object* _init_l_Lean_Parser_Tactic___aux__Init__Tactics______macroRules__Lean__Parser__Tactic__tacticNext___x3d_x3e____1___closed__6() {
 _start:
 {
 lean_object* x_1; 
@@ -3180,17 +3225,17 @@ x_1 = lean_mk_string_from_bytes("null", 4);
 return x_1;
 }
 }
-static lean_object* _init_l_Lean_Parser_Tactic___aux__Init__Tactics______macroRules__Lean__Parser__Tactic__tacticNext___x3d_x3e____1___closed__3() {
+static lean_object* _init_l_Lean_Parser_Tactic___aux__Init__Tactics______macroRules__Lean__Parser__Tactic__tacticNext___x3d_x3e____1___closed__7() {
 _start:
 {
 lean_object* x_1; lean_object* x_2; lean_object* x_3; 
 x_1 = lean_box(0);
-x_2 = l_Lean_Parser_Tactic___aux__Init__Tactics______macroRules__Lean__Parser__Tactic__tacticNext___x3d_x3e____1___closed__2;
+x_2 = l_Lean_Parser_Tactic___aux__Init__Tactics______macroRules__Lean__Parser__Tactic__tacticNext___x3d_x3e____1___closed__6;
 x_3 = l_Lean_Name_str___override(x_1, x_2);
 return x_3;
 }
 }
-static lean_object* _init_l_Lean_Parser_Tactic___aux__Init__Tactics______macroRules__Lean__Parser__Tactic__tacticNext___x3d_x3e____1___closed__4() {
+static lean_object* _init_l_Lean_Parser_Tactic___aux__Init__Tactics______macroRules__Lean__Parser__Tactic__tacticNext___x3d_x3e____1___closed__8() {
 _start:
 {
 lean_object* x_1; lean_object* x_2; 
@@ -3199,7 +3244,7 @@ x_2 = lean_mk_empty_array_with_capacity(x_1);
 return x_2;
 }
 }
-static lean_object* _init_l_Lean_Parser_Tactic___aux__Init__Tactics______macroRules__Lean__Parser__Tactic__tacticNext___x3d_x3e____1___closed__5() {
+static lean_object* _init_l_Lean_Parser_Tactic___aux__Init__Tactics______macroRules__Lean__Parser__Tactic__tacticNext___x3d_x3e____1___closed__9() {
 _start:
 {
 lean_object* x_1; 
@@ -3207,7 +3252,7 @@ x_1 = lean_mk_string_from_bytes("=>", 2);
 return x_1;
 }
 }
-static lean_object* _init_l_Lean_Parser_Tactic___aux__Init__Tactics______macroRules__Lean__Parser__Tactic__tacticNext___x3d_x3e____1___closed__6() {
+static lean_object* _init_l_Lean_Parser_Tactic___aux__Init__Tactics______macroRules__Lean__Parser__Tactic__tacticNext___x3d_x3e____1___closed__10() {
 _start:
 {
 lean_object* x_1; lean_object* x_2; 
@@ -3248,105 +3293,117 @@ x_13 = l_Lean_MonadRef_mkInfoFromRefPos___at___aux__Init__Notation______macroRul
 x_14 = !lean_is_exclusive(x_13);
 if (x_14 == 0)
 {
-lean_object* x_15; lean_object* x_16; lean_object* x_17; lean_object* x_18; lean_object* x_19; lean_object* x_20; lean_object* x_21; lean_object* x_22; lean_object* x_23; lean_object* x_24; lean_object* x_25; lean_object* x_26; lean_object* x_27; lean_object* x_28; lean_object* x_29; lean_object* x_30; lean_object* x_31; lean_object* x_32; lean_object* x_33; lean_object* x_34; lean_object* x_35; lean_object* x_36; lean_object* x_37; lean_object* x_38; 
+lean_object* x_15; lean_object* x_16; lean_object* x_17; lean_object* x_18; lean_object* x_19; lean_object* x_20; lean_object* x_21; lean_object* x_22; lean_object* x_23; lean_object* x_24; lean_object* x_25; lean_object* x_26; lean_object* x_27; lean_object* x_28; lean_object* x_29; lean_object* x_30; lean_object* x_31; lean_object* x_32; lean_object* x_33; lean_object* x_34; lean_object* x_35; lean_object* x_36; lean_object* x_37; lean_object* x_38; lean_object* x_39; lean_object* x_40; lean_object* x_41; 
 x_15 = lean_ctor_get(x_13, 0);
 x_16 = l_Lean_Parser_Tactic_case___closed__1;
 lean_inc(x_15);
 x_17 = lean_alloc_ctor(2, 2, 0);
 lean_ctor_set(x_17, 0, x_15);
 lean_ctor_set(x_17, 1, x_16);
-x_18 = l_Lean_binderIdent___closed__10;
+x_18 = l_Lean_Parser_Tactic___aux__Init__Tactics______macroRules__Lean__Parser__Tactic__tacticNext___x3d_x3e____1___closed__4;
 lean_inc(x_15);
 x_19 = lean_alloc_ctor(2, 2, 0);
 lean_ctor_set(x_19, 0, x_15);
 lean_ctor_set(x_19, 1, x_18);
-x_20 = l_Lean_Parser_Tactic___aux__Init__Tactics______macroRules__Lean__Parser__Tactic__tacticNext___x3d_x3e____1___closed__1;
+x_20 = l_Lean_Parser_Tactic___aux__Init__Tactics______macroRules__Lean__Parser__Tactic__tacticNext___x3d_x3e____1___closed__5;
 x_21 = lean_array_push(x_20, x_19);
 x_22 = lean_box(2);
-x_23 = l_Lean_binderIdent___closed__4;
+x_23 = l_Lean_Parser_Tactic___aux__Init__Tactics______macroRules__Lean__Parser__Tactic__tacticNext___x3d_x3e____1___closed__3;
 x_24 = lean_alloc_ctor(1, 3, 0);
 lean_ctor_set(x_24, 0, x_22);
 lean_ctor_set(x_24, 1, x_23);
 lean_ctor_set(x_24, 2, x_21);
-x_25 = l_Lean_Parser_Tactic___aux__Init__Tactics______macroRules__Lean__Parser__Tactic__tacticNext___x3d_x3e____1___closed__4;
-x_26 = l_Array_appendCore___rarg(x_25, x_12);
+x_25 = lean_array_push(x_20, x_24);
+x_26 = l_Lean_binderIdent___closed__4;
+x_27 = lean_alloc_ctor(1, 3, 0);
+lean_ctor_set(x_27, 0, x_22);
+lean_ctor_set(x_27, 1, x_26);
+lean_ctor_set(x_27, 2, x_25);
+x_28 = l_Lean_Parser_Tactic___aux__Init__Tactics______macroRules__Lean__Parser__Tactic__tacticNext___x3d_x3e____1___closed__8;
+x_29 = l_Array_appendCore___rarg(x_28, x_12);
 lean_dec(x_12);
-x_27 = l_Lean_Parser_Tactic___aux__Init__Tactics______macroRules__Lean__Parser__Tactic__tacticNext___x3d_x3e____1___closed__3;
-x_28 = lean_alloc_ctor(1, 3, 0);
-lean_ctor_set(x_28, 0, x_22);
-lean_ctor_set(x_28, 1, x_27);
-lean_ctor_set(x_28, 2, x_26);
-x_29 = l_Lean_Parser_Tactic___aux__Init__Tactics______macroRules__Lean__Parser__Tactic__tacticNext___x3d_x3e____1___closed__5;
-x_30 = lean_alloc_ctor(2, 2, 0);
-lean_ctor_set(x_30, 0, x_15);
-lean_ctor_set(x_30, 1, x_29);
-x_31 = l_Lean_Parser_Tactic___aux__Init__Tactics______macroRules__Lean__Parser__Tactic__tacticNext___x3d_x3e____1___closed__6;
-x_32 = lean_array_push(x_31, x_17);
-x_33 = lean_array_push(x_32, x_24);
-x_34 = lean_array_push(x_33, x_28);
-x_35 = lean_array_push(x_34, x_30);
-x_36 = lean_array_push(x_35, x_11);
-x_37 = l_Lean_Parser_Tactic_case___closed__2;
-x_38 = lean_alloc_ctor(1, 3, 0);
-lean_ctor_set(x_38, 0, x_22);
-lean_ctor_set(x_38, 1, x_37);
-lean_ctor_set(x_38, 2, x_36);
-lean_ctor_set(x_13, 0, x_38);
+x_30 = l_Lean_Parser_Tactic___aux__Init__Tactics______macroRules__Lean__Parser__Tactic__tacticNext___x3d_x3e____1___closed__7;
+x_31 = lean_alloc_ctor(1, 3, 0);
+lean_ctor_set(x_31, 0, x_22);
+lean_ctor_set(x_31, 1, x_30);
+lean_ctor_set(x_31, 2, x_29);
+x_32 = l_Lean_Parser_Tactic___aux__Init__Tactics______macroRules__Lean__Parser__Tactic__tacticNext___x3d_x3e____1___closed__9;
+x_33 = lean_alloc_ctor(2, 2, 0);
+lean_ctor_set(x_33, 0, x_15);
+lean_ctor_set(x_33, 1, x_32);
+x_34 = l_Lean_Parser_Tactic___aux__Init__Tactics______macroRules__Lean__Parser__Tactic__tacticNext___x3d_x3e____1___closed__10;
+x_35 = lean_array_push(x_34, x_17);
+x_36 = lean_array_push(x_35, x_27);
+x_37 = lean_array_push(x_36, x_31);
+x_38 = lean_array_push(x_37, x_33);
+x_39 = lean_array_push(x_38, x_11);
+x_40 = l_Lean_Parser_Tactic_case___closed__2;
+x_41 = lean_alloc_ctor(1, 3, 0);
+lean_ctor_set(x_41, 0, x_22);
+lean_ctor_set(x_41, 1, x_40);
+lean_ctor_set(x_41, 2, x_39);
+lean_ctor_set(x_13, 0, x_41);
 return x_13;
 }
 else
 {
-lean_object* x_39; lean_object* x_40; lean_object* x_41; lean_object* x_42; lean_object* x_43; lean_object* x_44; lean_object* x_45; lean_object* x_46; lean_object* x_47; lean_object* x_48; lean_object* x_49; lean_object* x_50; lean_object* x_51; lean_object* x_52; lean_object* x_53; lean_object* x_54; lean_object* x_55; lean_object* x_56; lean_object* x_57; lean_object* x_58; lean_object* x_59; lean_object* x_60; lean_object* x_61; lean_object* x_62; lean_object* x_63; lean_object* x_64; 
-x_39 = lean_ctor_get(x_13, 0);
-x_40 = lean_ctor_get(x_13, 1);
-lean_inc(x_40);
-lean_inc(x_39);
+lean_object* x_42; lean_object* x_43; lean_object* x_44; lean_object* x_45; lean_object* x_46; lean_object* x_47; lean_object* x_48; lean_object* x_49; lean_object* x_50; lean_object* x_51; lean_object* x_52; lean_object* x_53; lean_object* x_54; lean_object* x_55; lean_object* x_56; lean_object* x_57; lean_object* x_58; lean_object* x_59; lean_object* x_60; lean_object* x_61; lean_object* x_62; lean_object* x_63; lean_object* x_64; lean_object* x_65; lean_object* x_66; lean_object* x_67; lean_object* x_68; lean_object* x_69; lean_object* x_70; 
+x_42 = lean_ctor_get(x_13, 0);
+x_43 = lean_ctor_get(x_13, 1);
+lean_inc(x_43);
+lean_inc(x_42);
 lean_dec(x_13);
-x_41 = l_Lean_Parser_Tactic_case___closed__1;
-lean_inc(x_39);
-x_42 = lean_alloc_ctor(2, 2, 0);
-lean_ctor_set(x_42, 0, x_39);
-lean_ctor_set(x_42, 1, x_41);
-x_43 = l_Lean_binderIdent___closed__10;
-lean_inc(x_39);
-x_44 = lean_alloc_ctor(2, 2, 0);
-lean_ctor_set(x_44, 0, x_39);
-lean_ctor_set(x_44, 1, x_43);
-x_45 = l_Lean_Parser_Tactic___aux__Init__Tactics______macroRules__Lean__Parser__Tactic__tacticNext___x3d_x3e____1___closed__1;
-x_46 = lean_array_push(x_45, x_44);
-x_47 = lean_box(2);
-x_48 = l_Lean_binderIdent___closed__4;
-x_49 = lean_alloc_ctor(1, 3, 0);
-lean_ctor_set(x_49, 0, x_47);
-lean_ctor_set(x_49, 1, x_48);
-lean_ctor_set(x_49, 2, x_46);
-x_50 = l_Lean_Parser_Tactic___aux__Init__Tactics______macroRules__Lean__Parser__Tactic__tacticNext___x3d_x3e____1___closed__4;
-x_51 = l_Array_appendCore___rarg(x_50, x_12);
-lean_dec(x_12);
-x_52 = l_Lean_Parser_Tactic___aux__Init__Tactics______macroRules__Lean__Parser__Tactic__tacticNext___x3d_x3e____1___closed__3;
-x_53 = lean_alloc_ctor(1, 3, 0);
-lean_ctor_set(x_53, 0, x_47);
-lean_ctor_set(x_53, 1, x_52);
-lean_ctor_set(x_53, 2, x_51);
-x_54 = l_Lean_Parser_Tactic___aux__Init__Tactics______macroRules__Lean__Parser__Tactic__tacticNext___x3d_x3e____1___closed__5;
-x_55 = lean_alloc_ctor(2, 2, 0);
-lean_ctor_set(x_55, 0, x_39);
+x_44 = l_Lean_Parser_Tactic_case___closed__1;
+lean_inc(x_42);
+x_45 = lean_alloc_ctor(2, 2, 0);
+lean_ctor_set(x_45, 0, x_42);
+lean_ctor_set(x_45, 1, x_44);
+x_46 = l_Lean_Parser_Tactic___aux__Init__Tactics______macroRules__Lean__Parser__Tactic__tacticNext___x3d_x3e____1___closed__4;
+lean_inc(x_42);
+x_47 = lean_alloc_ctor(2, 2, 0);
+lean_ctor_set(x_47, 0, x_42);
+lean_ctor_set(x_47, 1, x_46);
+x_48 = l_Lean_Parser_Tactic___aux__Init__Tactics______macroRules__Lean__Parser__Tactic__tacticNext___x3d_x3e____1___closed__5;
+x_49 = lean_array_push(x_48, x_47);
+x_50 = lean_box(2);
+x_51 = l_Lean_Parser_Tactic___aux__Init__Tactics______macroRules__Lean__Parser__Tactic__tacticNext___x3d_x3e____1___closed__3;
+x_52 = lean_alloc_ctor(1, 3, 0);
+lean_ctor_set(x_52, 0, x_50);
+lean_ctor_set(x_52, 1, x_51);
+lean_ctor_set(x_52, 2, x_49);
+x_53 = lean_array_push(x_48, x_52);
+x_54 = l_Lean_binderIdent___closed__4;
+x_55 = lean_alloc_ctor(1, 3, 0);
+lean_ctor_set(x_55, 0, x_50);
 lean_ctor_set(x_55, 1, x_54);
-x_56 = l_Lean_Parser_Tactic___aux__Init__Tactics______macroRules__Lean__Parser__Tactic__tacticNext___x3d_x3e____1___closed__6;
-x_57 = lean_array_push(x_56, x_42);
-x_58 = lean_array_push(x_57, x_49);
-x_59 = lean_array_push(x_58, x_53);
-x_60 = lean_array_push(x_59, x_55);
-x_61 = lean_array_push(x_60, x_11);
-x_62 = l_Lean_Parser_Tactic_case___closed__2;
-x_63 = lean_alloc_ctor(1, 3, 0);
-lean_ctor_set(x_63, 0, x_47);
-lean_ctor_set(x_63, 1, x_62);
-lean_ctor_set(x_63, 2, x_61);
-x_64 = lean_alloc_ctor(0, 2, 0);
-lean_ctor_set(x_64, 0, x_63);
-lean_ctor_set(x_64, 1, x_40);
-return x_64;
+lean_ctor_set(x_55, 2, x_53);
+x_56 = l_Lean_Parser_Tactic___aux__Init__Tactics______macroRules__Lean__Parser__Tactic__tacticNext___x3d_x3e____1___closed__8;
+x_57 = l_Array_appendCore___rarg(x_56, x_12);
+lean_dec(x_12);
+x_58 = l_Lean_Parser_Tactic___aux__Init__Tactics______macroRules__Lean__Parser__Tactic__tacticNext___x3d_x3e____1___closed__7;
+x_59 = lean_alloc_ctor(1, 3, 0);
+lean_ctor_set(x_59, 0, x_50);
+lean_ctor_set(x_59, 1, x_58);
+lean_ctor_set(x_59, 2, x_57);
+x_60 = l_Lean_Parser_Tactic___aux__Init__Tactics______macroRules__Lean__Parser__Tactic__tacticNext___x3d_x3e____1___closed__9;
+x_61 = lean_alloc_ctor(2, 2, 0);
+lean_ctor_set(x_61, 0, x_42);
+lean_ctor_set(x_61, 1, x_60);
+x_62 = l_Lean_Parser_Tactic___aux__Init__Tactics______macroRules__Lean__Parser__Tactic__tacticNext___x3d_x3e____1___closed__10;
+x_63 = lean_array_push(x_62, x_45);
+x_64 = lean_array_push(x_63, x_55);
+x_65 = lean_array_push(x_64, x_59);
+x_66 = lean_array_push(x_65, x_61);
+x_67 = lean_array_push(x_66, x_11);
+x_68 = l_Lean_Parser_Tactic_case___closed__2;
+x_69 = lean_alloc_ctor(1, 3, 0);
+lean_ctor_set(x_69, 0, x_50);
+lean_ctor_set(x_69, 1, x_68);
+lean_ctor_set(x_69, 2, x_67);
+x_70 = lean_alloc_ctor(0, 2, 0);
+lean_ctor_set(x_70, 0, x_69);
+lean_ctor_set(x_70, 1, x_43);
+return x_70;
 }
 }
 }
@@ -4783,8 +4840,8 @@ _start:
 {
 lean_object* x_1; lean_object* x_2; lean_object* x_3; lean_object* x_4; 
 x_1 = lean_box(2);
-x_2 = l_Lean_Parser_Tactic___aux__Init__Tactics______macroRules__Lean__Parser__Tactic__tacticNext___x3d_x3e____1___closed__3;
-x_3 = l_Lean_Parser_Tactic___aux__Init__Tactics______macroRules__Lean__Parser__Tactic__tacticNext___x3d_x3e____1___closed__4;
+x_2 = l_Lean_Parser_Tactic___aux__Init__Tactics______macroRules__Lean__Parser__Tactic__tacticNext___x3d_x3e____1___closed__7;
+x_3 = l_Lean_Parser_Tactic___aux__Init__Tactics______macroRules__Lean__Parser__Tactic__tacticNext___x3d_x3e____1___closed__8;
 x_4 = lean_alloc_ctor(1, 3, 0);
 lean_ctor_set(x_4, 0, x_1);
 lean_ctor_set(x_4, 1, x_2);
@@ -4846,7 +4903,7 @@ x_23 = l_Lean_Parser_Tactic_skip___closed__1;
 x_24 = lean_alloc_ctor(2, 2, 0);
 lean_ctor_set(x_24, 0, x_12);
 lean_ctor_set(x_24, 1, x_23);
-x_25 = l_Lean_Parser_Tactic___aux__Init__Tactics______macroRules__Lean__Parser__Tactic__tacticNext___x3d_x3e____1___closed__1;
+x_25 = l_Lean_Parser_Tactic___aux__Init__Tactics______macroRules__Lean__Parser__Tactic__tacticNext___x3d_x3e____1___closed__5;
 x_26 = lean_array_push(x_25, x_24);
 x_27 = l_Lean_Parser_Tactic_skip___closed__2;
 x_28 = lean_alloc_ctor(1, 3, 0);
@@ -4861,7 +4918,7 @@ lean_ctor_set(x_32, 0, x_20);
 lean_ctor_set(x_32, 1, x_21);
 lean_ctor_set(x_32, 2, x_31);
 x_33 = lean_array_push(x_25, x_32);
-x_34 = l_Lean_Parser_Tactic___aux__Init__Tactics______macroRules__Lean__Parser__Tactic__tacticNext___x3d_x3e____1___closed__3;
+x_34 = l_Lean_Parser_Tactic___aux__Init__Tactics______macroRules__Lean__Parser__Tactic__tacticNext___x3d_x3e____1___closed__7;
 x_35 = lean_alloc_ctor(1, 3, 0);
 lean_ctor_set(x_35, 0, x_20);
 lean_ctor_set(x_35, 1, x_34);
@@ -4942,7 +4999,7 @@ x_68 = l_Lean_Parser_Tactic_skip___closed__1;
 x_69 = lean_alloc_ctor(2, 2, 0);
 lean_ctor_set(x_69, 0, x_56);
 lean_ctor_set(x_69, 1, x_68);
-x_70 = l_Lean_Parser_Tactic___aux__Init__Tactics______macroRules__Lean__Parser__Tactic__tacticNext___x3d_x3e____1___closed__1;
+x_70 = l_Lean_Parser_Tactic___aux__Init__Tactics______macroRules__Lean__Parser__Tactic__tacticNext___x3d_x3e____1___closed__5;
 x_71 = lean_array_push(x_70, x_69);
 x_72 = l_Lean_Parser_Tactic_skip___closed__2;
 x_73 = lean_alloc_ctor(1, 3, 0);
@@ -4957,7 +5014,7 @@ lean_ctor_set(x_77, 0, x_65);
 lean_ctor_set(x_77, 1, x_66);
 lean_ctor_set(x_77, 2, x_76);
 x_78 = lean_array_push(x_70, x_77);
-x_79 = l_Lean_Parser_Tactic___aux__Init__Tactics______macroRules__Lean__Parser__Tactic__tacticNext___x3d_x3e____1___closed__3;
+x_79 = l_Lean_Parser_Tactic___aux__Init__Tactics______macroRules__Lean__Parser__Tactic__tacticNext___x3d_x3e____1___closed__7;
 x_80 = lean_alloc_ctor(1, 3, 0);
 lean_ctor_set(x_80, 0, x_65);
 lean_ctor_set(x_80, 1, x_79);
@@ -5169,7 +5226,7 @@ lean_inc(x_16);
 x_29 = lean_alloc_ctor(2, 2, 0);
 lean_ctor_set(x_29, 0, x_16);
 lean_ctor_set(x_29, 1, x_28);
-x_30 = l_Lean_Parser_Tactic___aux__Init__Tactics______macroRules__Lean__Parser__Tactic__tacticNext___x3d_x3e____1___closed__1;
+x_30 = l_Lean_Parser_Tactic___aux__Init__Tactics______macroRules__Lean__Parser__Tactic__tacticNext___x3d_x3e____1___closed__5;
 x_31 = lean_array_push(x_30, x_29);
 x_32 = l_Lean_Parser_Tactic_skip___closed__2;
 x_33 = lean_alloc_ctor(1, 3, 0);
@@ -5202,7 +5259,7 @@ lean_ctor_set(x_47, 0, x_23);
 lean_ctor_set(x_47, 1, x_24);
 lean_ctor_set(x_47, 2, x_46);
 x_48 = lean_array_push(x_30, x_47);
-x_49 = l_Lean_Parser_Tactic___aux__Init__Tactics______macroRules__Lean__Parser__Tactic__tacticNext___x3d_x3e____1___closed__3;
+x_49 = l_Lean_Parser_Tactic___aux__Init__Tactics______macroRules__Lean__Parser__Tactic__tacticNext___x3d_x3e____1___closed__7;
 x_50 = lean_alloc_ctor(1, 3, 0);
 lean_ctor_set(x_50, 0, x_23);
 lean_ctor_set(x_50, 1, x_49);
@@ -5292,7 +5349,7 @@ lean_inc(x_76);
 x_90 = lean_alloc_ctor(2, 2, 0);
 lean_ctor_set(x_90, 0, x_76);
 lean_ctor_set(x_90, 1, x_89);
-x_91 = l_Lean_Parser_Tactic___aux__Init__Tactics______macroRules__Lean__Parser__Tactic__tacticNext___x3d_x3e____1___closed__1;
+x_91 = l_Lean_Parser_Tactic___aux__Init__Tactics______macroRules__Lean__Parser__Tactic__tacticNext___x3d_x3e____1___closed__5;
 x_92 = lean_array_push(x_91, x_90);
 x_93 = l_Lean_Parser_Tactic_skip___closed__2;
 x_94 = lean_alloc_ctor(1, 3, 0);
@@ -5325,7 +5382,7 @@ lean_ctor_set(x_108, 0, x_84);
 lean_ctor_set(x_108, 1, x_85);
 lean_ctor_set(x_108, 2, x_107);
 x_109 = lean_array_push(x_91, x_108);
-x_110 = l_Lean_Parser_Tactic___aux__Init__Tactics______macroRules__Lean__Parser__Tactic__tacticNext___x3d_x3e____1___closed__3;
+x_110 = l_Lean_Parser_Tactic___aux__Init__Tactics______macroRules__Lean__Parser__Tactic__tacticNext___x3d_x3e____1___closed__7;
 x_111 = lean_alloc_ctor(1, 3, 0);
 lean_ctor_set(x_111, 0, x_84);
 lean_ctor_set(x_111, 1, x_110);
@@ -5536,7 +5593,7 @@ x_11 = l_Lean_Parser_Tactic_refl___closed__3;
 x_12 = lean_alloc_ctor(2, 2, 0);
 lean_ctor_set(x_12, 0, x_10);
 lean_ctor_set(x_12, 1, x_11);
-x_13 = l_Lean_Parser_Tactic___aux__Init__Tactics______macroRules__Lean__Parser__Tactic__tacticNext___x3d_x3e____1___closed__1;
+x_13 = l_Lean_Parser_Tactic___aux__Init__Tactics______macroRules__Lean__Parser__Tactic__tacticNext___x3d_x3e____1___closed__5;
 x_14 = lean_array_push(x_13, x_12);
 x_15 = lean_box(2);
 x_16 = l_Lean_Parser_Tactic_refl___closed__2;
@@ -5545,7 +5602,7 @@ lean_ctor_set(x_17, 0, x_15);
 lean_ctor_set(x_17, 1, x_16);
 lean_ctor_set(x_17, 2, x_14);
 x_18 = lean_array_push(x_13, x_17);
-x_19 = l_Lean_Parser_Tactic___aux__Init__Tactics______macroRules__Lean__Parser__Tactic__tacticNext___x3d_x3e____1___closed__3;
+x_19 = l_Lean_Parser_Tactic___aux__Init__Tactics______macroRules__Lean__Parser__Tactic__tacticNext___x3d_x3e____1___closed__7;
 x_20 = lean_alloc_ctor(1, 3, 0);
 lean_ctor_set(x_20, 0, x_15);
 lean_ctor_set(x_20, 1, x_19);
@@ -5571,7 +5628,7 @@ x_26 = l_Lean_Parser_Tactic_refl___closed__3;
 x_27 = lean_alloc_ctor(2, 2, 0);
 lean_ctor_set(x_27, 0, x_24);
 lean_ctor_set(x_27, 1, x_26);
-x_28 = l_Lean_Parser_Tactic___aux__Init__Tactics______macroRules__Lean__Parser__Tactic__tacticNext___x3d_x3e____1___closed__1;
+x_28 = l_Lean_Parser_Tactic___aux__Init__Tactics______macroRules__Lean__Parser__Tactic__tacticNext___x3d_x3e____1___closed__5;
 x_29 = lean_array_push(x_28, x_27);
 x_30 = lean_box(2);
 x_31 = l_Lean_Parser_Tactic_refl___closed__2;
@@ -5580,7 +5637,7 @@ lean_ctor_set(x_32, 0, x_30);
 lean_ctor_set(x_32, 1, x_31);
 lean_ctor_set(x_32, 2, x_29);
 x_33 = lean_array_push(x_28, x_32);
-x_34 = l_Lean_Parser_Tactic___aux__Init__Tactics______macroRules__Lean__Parser__Tactic__tacticNext___x3d_x3e____1___closed__3;
+x_34 = l_Lean_Parser_Tactic___aux__Init__Tactics______macroRules__Lean__Parser__Tactic__tacticNext___x3d_x3e____1___closed__7;
 x_35 = lean_alloc_ctor(1, 3, 0);
 lean_ctor_set(x_35, 0, x_30);
 lean_ctor_set(x_35, 1, x_34);
@@ -5807,7 +5864,7 @@ x_26 = l_Lean_Parser_Tactic_tacticRfl___closed__3;
 x_27 = lean_alloc_ctor(2, 2, 0);
 lean_ctor_set(x_27, 0, x_10);
 lean_ctor_set(x_27, 1, x_26);
-x_28 = l_Lean_Parser_Tactic___aux__Init__Tactics______macroRules__Lean__Parser__Tactic__tacticNext___x3d_x3e____1___closed__1;
+x_28 = l_Lean_Parser_Tactic___aux__Init__Tactics______macroRules__Lean__Parser__Tactic__tacticNext___x3d_x3e____1___closed__5;
 x_29 = lean_array_push(x_28, x_27);
 x_30 = lean_box(2);
 x_31 = l_Lean_Parser_Tactic_tacticRfl___closed__2;
@@ -5825,7 +5882,7 @@ lean_ctor_set(x_38, 0, x_30);
 lean_ctor_set(x_38, 1, x_37);
 lean_ctor_set(x_38, 2, x_36);
 x_39 = lean_array_push(x_28, x_38);
-x_40 = l_Lean_Parser_Tactic___aux__Init__Tactics______macroRules__Lean__Parser__Tactic__tacticNext___x3d_x3e____1___closed__3;
+x_40 = l_Lean_Parser_Tactic___aux__Init__Tactics______macroRules__Lean__Parser__Tactic__tacticNext___x3d_x3e____1___closed__7;
 x_41 = lean_alloc_ctor(1, 3, 0);
 lean_ctor_set(x_41, 0, x_30);
 lean_ctor_set(x_41, 1, x_40);
@@ -5870,7 +5927,7 @@ x_60 = lean_alloc_ctor(1, 3, 0);
 lean_ctor_set(x_60, 0, x_30);
 lean_ctor_set(x_60, 1, x_46);
 lean_ctor_set(x_60, 2, x_59);
-x_61 = l_Lean_Parser_Tactic___aux__Init__Tactics______macroRules__Lean__Parser__Tactic__tacticNext___x3d_x3e____1___closed__6;
+x_61 = l_Lean_Parser_Tactic___aux__Init__Tactics______macroRules__Lean__Parser__Tactic__tacticNext___x3d_x3e____1___closed__10;
 x_62 = lean_array_push(x_61, x_14);
 x_63 = lean_array_push(x_62, x_19);
 x_64 = lean_array_push(x_63, x_21);
@@ -5942,7 +5999,7 @@ x_91 = l_Lean_Parser_Tactic_tacticRfl___closed__3;
 x_92 = lean_alloc_ctor(2, 2, 0);
 lean_ctor_set(x_92, 0, x_74);
 lean_ctor_set(x_92, 1, x_91);
-x_93 = l_Lean_Parser_Tactic___aux__Init__Tactics______macroRules__Lean__Parser__Tactic__tacticNext___x3d_x3e____1___closed__1;
+x_93 = l_Lean_Parser_Tactic___aux__Init__Tactics______macroRules__Lean__Parser__Tactic__tacticNext___x3d_x3e____1___closed__5;
 x_94 = lean_array_push(x_93, x_92);
 x_95 = lean_box(2);
 x_96 = l_Lean_Parser_Tactic_tacticRfl___closed__2;
@@ -5960,7 +6017,7 @@ lean_ctor_set(x_103, 0, x_95);
 lean_ctor_set(x_103, 1, x_102);
 lean_ctor_set(x_103, 2, x_101);
 x_104 = lean_array_push(x_93, x_103);
-x_105 = l_Lean_Parser_Tactic___aux__Init__Tactics______macroRules__Lean__Parser__Tactic__tacticNext___x3d_x3e____1___closed__3;
+x_105 = l_Lean_Parser_Tactic___aux__Init__Tactics______macroRules__Lean__Parser__Tactic__tacticNext___x3d_x3e____1___closed__7;
 x_106 = lean_alloc_ctor(1, 3, 0);
 lean_ctor_set(x_106, 0, x_95);
 lean_ctor_set(x_106, 1, x_105);
@@ -6005,7 +6062,7 @@ x_125 = lean_alloc_ctor(1, 3, 0);
 lean_ctor_set(x_125, 0, x_95);
 lean_ctor_set(x_125, 1, x_111);
 lean_ctor_set(x_125, 2, x_124);
-x_126 = l_Lean_Parser_Tactic___aux__Init__Tactics______macroRules__Lean__Parser__Tactic__tacticNext___x3d_x3e____1___closed__6;
+x_126 = l_Lean_Parser_Tactic___aux__Init__Tactics______macroRules__Lean__Parser__Tactic__tacticNext___x3d_x3e____1___closed__10;
 x_127 = lean_array_push(x_126, x_79);
 x_128 = lean_array_push(x_127, x_84);
 x_129 = lean_array_push(x_128, x_86);
@@ -6159,7 +6216,7 @@ static lean_object* _init_l_Lean_Parser_Tactic___aux__Init__Tactics______macroRu
 _start:
 {
 lean_object* x_1; 
-x_1 = lean_mk_string_from_bytes("Term", 4);
+x_1 = lean_mk_string_from_bytes("app", 3);
 return x_1;
 }
 }
@@ -6167,7 +6224,7 @@ static lean_object* _init_l_Lean_Parser_Tactic___aux__Init__Tactics______macroRu
 _start:
 {
 lean_object* x_1; lean_object* x_2; lean_object* x_3; 
-x_1 = l_Lean_Parser_Tactic_withAnnotateState___closed__2;
+x_1 = l_Lean_Parser_Tactic___aux__Init__Tactics______macroRules__Lean__Parser__Tactic__tacticNext___x3d_x3e____1___closed__2;
 x_2 = l_Lean_Parser_Tactic___aux__Init__Tactics______macroRules__Lean__Parser__Tactic__tacticAdmit__1___closed__1;
 x_3 = l_Lean_Name_str___override(x_1, x_2);
 return x_3;
@@ -6177,7 +6234,7 @@ static lean_object* _init_l_Lean_Parser_Tactic___aux__Init__Tactics______macroRu
 _start:
 {
 lean_object* x_1; 
-x_1 = lean_mk_string_from_bytes("app", 3);
+x_1 = lean_mk_string_from_bytes("explicit", 8);
 return x_1;
 }
 }
@@ -6185,7 +6242,7 @@ static lean_object* _init_l_Lean_Parser_Tactic___aux__Init__Tactics______macroRu
 _start:
 {
 lean_object* x_1; lean_object* x_2; lean_object* x_3; 
-x_1 = l_Lean_Parser_Tactic___aux__Init__Tactics______macroRules__Lean__Parser__Tactic__tacticAdmit__1___closed__2;
+x_1 = l_Lean_Parser_Tactic___aux__Init__Tactics______macroRules__Lean__Parser__Tactic__tacticNext___x3d_x3e____1___closed__2;
 x_2 = l_Lean_Parser_Tactic___aux__Init__Tactics______macroRules__Lean__Parser__Tactic__tacticAdmit__1___closed__3;
 x_3 = l_Lean_Name_str___override(x_1, x_2);
 return x_3;
@@ -6195,29 +6252,11 @@ static lean_object* _init_l_Lean_Parser_Tactic___aux__Init__Tactics______macroRu
 _start:
 {
 lean_object* x_1; 
-x_1 = lean_mk_string_from_bytes("explicit", 8);
-return x_1;
-}
-}
-static lean_object* _init_l_Lean_Parser_Tactic___aux__Init__Tactics______macroRules__Lean__Parser__Tactic__tacticAdmit__1___closed__6() {
-_start:
-{
-lean_object* x_1; lean_object* x_2; lean_object* x_3; 
-x_1 = l_Lean_Parser_Tactic___aux__Init__Tactics______macroRules__Lean__Parser__Tactic__tacticAdmit__1___closed__2;
-x_2 = l_Lean_Parser_Tactic___aux__Init__Tactics______macroRules__Lean__Parser__Tactic__tacticAdmit__1___closed__5;
-x_3 = l_Lean_Name_str___override(x_1, x_2);
-return x_3;
-}
-}
-static lean_object* _init_l_Lean_Parser_Tactic___aux__Init__Tactics______macroRules__Lean__Parser__Tactic__tacticAdmit__1___closed__7() {
-_start:
-{
-lean_object* x_1; 
 x_1 = lean_mk_string_from_bytes("@", 1);
 return x_1;
 }
 }
-static lean_object* _init_l_Lean_Parser_Tactic___aux__Init__Tactics______macroRules__Lean__Parser__Tactic__tacticAdmit__1___closed__8() {
+static lean_object* _init_l_Lean_Parser_Tactic___aux__Init__Tactics______macroRules__Lean__Parser__Tactic__tacticAdmit__1___closed__6() {
 _start:
 {
 lean_object* x_1; 
@@ -6225,27 +6264,49 @@ x_1 = lean_mk_string_from_bytes("sorryAx", 7);
 return x_1;
 }
 }
-static lean_object* _init_l_Lean_Parser_Tactic___aux__Init__Tactics______macroRules__Lean__Parser__Tactic__tacticAdmit__1___closed__9() {
+static lean_object* _init_l_Lean_Parser_Tactic___aux__Init__Tactics______macroRules__Lean__Parser__Tactic__tacticAdmit__1___closed__7() {
 _start:
 {
 lean_object* x_1; lean_object* x_2; 
-x_1 = l_Lean_Parser_Tactic___aux__Init__Tactics______macroRules__Lean__Parser__Tactic__tacticAdmit__1___closed__8;
+x_1 = l_Lean_Parser_Tactic___aux__Init__Tactics______macroRules__Lean__Parser__Tactic__tacticAdmit__1___closed__6;
 x_2 = lean_string_utf8_byte_size(x_1);
 return x_2;
 }
 }
-static lean_object* _init_l_Lean_Parser_Tactic___aux__Init__Tactics______macroRules__Lean__Parser__Tactic__tacticAdmit__1___closed__10() {
+static lean_object* _init_l_Lean_Parser_Tactic___aux__Init__Tactics______macroRules__Lean__Parser__Tactic__tacticAdmit__1___closed__8() {
 _start:
 {
 lean_object* x_1; lean_object* x_2; lean_object* x_3; lean_object* x_4; 
-x_1 = l_Lean_Parser_Tactic___aux__Init__Tactics______macroRules__Lean__Parser__Tactic__tacticAdmit__1___closed__8;
+x_1 = l_Lean_Parser_Tactic___aux__Init__Tactics______macroRules__Lean__Parser__Tactic__tacticAdmit__1___closed__6;
 x_2 = lean_unsigned_to_nat(0u);
-x_3 = l_Lean_Parser_Tactic___aux__Init__Tactics______macroRules__Lean__Parser__Tactic__tacticAdmit__1___closed__9;
+x_3 = l_Lean_Parser_Tactic___aux__Init__Tactics______macroRules__Lean__Parser__Tactic__tacticAdmit__1___closed__7;
 x_4 = lean_alloc_ctor(0, 3, 0);
 lean_ctor_set(x_4, 0, x_1);
 lean_ctor_set(x_4, 1, x_2);
 lean_ctor_set(x_4, 2, x_3);
 return x_4;
+}
+}
+static lean_object* _init_l_Lean_Parser_Tactic___aux__Init__Tactics______macroRules__Lean__Parser__Tactic__tacticAdmit__1___closed__9() {
+_start:
+{
+lean_object* x_1; lean_object* x_2; lean_object* x_3; 
+x_1 = lean_box(0);
+x_2 = l_Lean_Parser_Tactic___aux__Init__Tactics______macroRules__Lean__Parser__Tactic__tacticAdmit__1___closed__6;
+x_3 = l_Lean_Name_str___override(x_1, x_2);
+return x_3;
+}
+}
+static lean_object* _init_l_Lean_Parser_Tactic___aux__Init__Tactics______macroRules__Lean__Parser__Tactic__tacticAdmit__1___closed__10() {
+_start:
+{
+lean_object* x_1; lean_object* x_2; lean_object* x_3; 
+x_1 = lean_box(0);
+x_2 = l_Lean_Parser_Tactic___aux__Init__Tactics______macroRules__Lean__Parser__Tactic__tacticAdmit__1___closed__9;
+x_3 = lean_alloc_ctor(0, 2, 0);
+lean_ctor_set(x_3, 0, x_2);
+lean_ctor_set(x_3, 1, x_1);
+return x_3;
 }
 }
 static lean_object* _init_l_Lean_Parser_Tactic___aux__Init__Tactics______macroRules__Lean__Parser__Tactic__tacticAdmit__1___closed__11() {
@@ -6253,54 +6314,14 @@ _start:
 {
 lean_object* x_1; lean_object* x_2; lean_object* x_3; 
 x_1 = lean_box(0);
-x_2 = l_Lean_Parser_Tactic___aux__Init__Tactics______macroRules__Lean__Parser__Tactic__tacticAdmit__1___closed__8;
-x_3 = l_Lean_Name_str___override(x_1, x_2);
-return x_3;
-}
-}
-static lean_object* _init_l_Lean_Parser_Tactic___aux__Init__Tactics______macroRules__Lean__Parser__Tactic__tacticAdmit__1___closed__12() {
-_start:
-{
-lean_object* x_1; lean_object* x_2; lean_object* x_3; 
-x_1 = lean_box(0);
-x_2 = l_Lean_Parser_Tactic___aux__Init__Tactics______macroRules__Lean__Parser__Tactic__tacticAdmit__1___closed__11;
-x_3 = lean_alloc_ctor(0, 2, 0);
-lean_ctor_set(x_3, 0, x_2);
-lean_ctor_set(x_3, 1, x_1);
-return x_3;
-}
-}
-static lean_object* _init_l_Lean_Parser_Tactic___aux__Init__Tactics______macroRules__Lean__Parser__Tactic__tacticAdmit__1___closed__13() {
-_start:
-{
-lean_object* x_1; lean_object* x_2; lean_object* x_3; 
-x_1 = lean_box(0);
-x_2 = l_Lean_Parser_Tactic___aux__Init__Tactics______macroRules__Lean__Parser__Tactic__tacticAdmit__1___closed__12;
+x_2 = l_Lean_Parser_Tactic___aux__Init__Tactics______macroRules__Lean__Parser__Tactic__tacticAdmit__1___closed__10;
 x_3 = lean_alloc_ctor(1, 2, 0);
 lean_ctor_set(x_3, 0, x_2);
 lean_ctor_set(x_3, 1, x_1);
 return x_3;
 }
 }
-static lean_object* _init_l_Lean_Parser_Tactic___aux__Init__Tactics______macroRules__Lean__Parser__Tactic__tacticAdmit__1___closed__14() {
-_start:
-{
-lean_object* x_1; 
-x_1 = lean_mk_string_from_bytes("hole", 4);
-return x_1;
-}
-}
-static lean_object* _init_l_Lean_Parser_Tactic___aux__Init__Tactics______macroRules__Lean__Parser__Tactic__tacticAdmit__1___closed__15() {
-_start:
-{
-lean_object* x_1; lean_object* x_2; lean_object* x_3; 
-x_1 = l_Lean_Parser_Tactic___aux__Init__Tactics______macroRules__Lean__Parser__Tactic__tacticAdmit__1___closed__2;
-x_2 = l_Lean_Parser_Tactic___aux__Init__Tactics______macroRules__Lean__Parser__Tactic__tacticAdmit__1___closed__14;
-x_3 = l_Lean_Name_str___override(x_1, x_2);
-return x_3;
-}
-}
-static lean_object* _init_l_Lean_Parser_Tactic___aux__Init__Tactics______macroRules__Lean__Parser__Tactic__tacticAdmit__1___closed__16() {
+static lean_object* _init_l_Lean_Parser_Tactic___aux__Init__Tactics______macroRules__Lean__Parser__Tactic__tacticAdmit__1___closed__12() {
 _start:
 {
 lean_object* x_1; lean_object* x_2; 
@@ -6309,13 +6330,13 @@ x_2 = lean_string_utf8_byte_size(x_1);
 return x_2;
 }
 }
-static lean_object* _init_l_Lean_Parser_Tactic___aux__Init__Tactics______macroRules__Lean__Parser__Tactic__tacticAdmit__1___closed__17() {
+static lean_object* _init_l_Lean_Parser_Tactic___aux__Init__Tactics______macroRules__Lean__Parser__Tactic__tacticAdmit__1___closed__13() {
 _start:
 {
 lean_object* x_1; lean_object* x_2; lean_object* x_3; lean_object* x_4; 
 x_1 = l_Lean_Parser_Tactic___aux__Init__Tactics______macroRules__Lean__Parser__Tactic__tacticRfl_x27__1___closed__7;
 x_2 = lean_unsigned_to_nat(0u);
-x_3 = l_Lean_Parser_Tactic___aux__Init__Tactics______macroRules__Lean__Parser__Tactic__tacticAdmit__1___closed__16;
+x_3 = l_Lean_Parser_Tactic___aux__Init__Tactics______macroRules__Lean__Parser__Tactic__tacticAdmit__1___closed__12;
 x_4 = lean_alloc_ctor(0, 3, 0);
 lean_ctor_set(x_4, 0, x_1);
 lean_ctor_set(x_4, 1, x_2);
@@ -6323,7 +6344,7 @@ lean_ctor_set(x_4, 2, x_3);
 return x_4;
 }
 }
-static lean_object* _init_l_Lean_Parser_Tactic___aux__Init__Tactics______macroRules__Lean__Parser__Tactic__tacticAdmit__1___closed__18() {
+static lean_object* _init_l_Lean_Parser_Tactic___aux__Init__Tactics______macroRules__Lean__Parser__Tactic__tacticAdmit__1___closed__14() {
 _start:
 {
 lean_object* x_1; lean_object* x_2; lean_object* x_3; 
@@ -6333,7 +6354,7 @@ x_3 = l_Lean_Name_str___override(x_1, x_2);
 return x_3;
 }
 }
-static lean_object* _init_l_Lean_Parser_Tactic___aux__Init__Tactics______macroRules__Lean__Parser__Tactic__tacticAdmit__1___closed__19() {
+static lean_object* _init_l_Lean_Parser_Tactic___aux__Init__Tactics______macroRules__Lean__Parser__Tactic__tacticAdmit__1___closed__15() {
 _start:
 {
 lean_object* x_1; 
@@ -6341,44 +6362,44 @@ x_1 = lean_mk_string_from_bytes("Bool", 4);
 return x_1;
 }
 }
-static lean_object* _init_l_Lean_Parser_Tactic___aux__Init__Tactics______macroRules__Lean__Parser__Tactic__tacticAdmit__1___closed__20() {
+static lean_object* _init_l_Lean_Parser_Tactic___aux__Init__Tactics______macroRules__Lean__Parser__Tactic__tacticAdmit__1___closed__16() {
 _start:
 {
 lean_object* x_1; lean_object* x_2; lean_object* x_3; 
 x_1 = lean_box(0);
-x_2 = l_Lean_Parser_Tactic___aux__Init__Tactics______macroRules__Lean__Parser__Tactic__tacticAdmit__1___closed__19;
+x_2 = l_Lean_Parser_Tactic___aux__Init__Tactics______macroRules__Lean__Parser__Tactic__tacticAdmit__1___closed__15;
 x_3 = l_Lean_Name_str___override(x_1, x_2);
 return x_3;
 }
 }
-static lean_object* _init_l_Lean_Parser_Tactic___aux__Init__Tactics______macroRules__Lean__Parser__Tactic__tacticAdmit__1___closed__21() {
+static lean_object* _init_l_Lean_Parser_Tactic___aux__Init__Tactics______macroRules__Lean__Parser__Tactic__tacticAdmit__1___closed__17() {
 _start:
 {
 lean_object* x_1; lean_object* x_2; lean_object* x_3; 
-x_1 = l_Lean_Parser_Tactic___aux__Init__Tactics______macroRules__Lean__Parser__Tactic__tacticAdmit__1___closed__20;
+x_1 = l_Lean_Parser_Tactic___aux__Init__Tactics______macroRules__Lean__Parser__Tactic__tacticAdmit__1___closed__16;
 x_2 = l_Lean_Parser_Tactic___aux__Init__Tactics______macroRules__Lean__Parser__Tactic__tacticRfl_x27__1___closed__7;
 x_3 = l_Lean_Name_str___override(x_1, x_2);
 return x_3;
 }
 }
-static lean_object* _init_l_Lean_Parser_Tactic___aux__Init__Tactics______macroRules__Lean__Parser__Tactic__tacticAdmit__1___closed__22() {
+static lean_object* _init_l_Lean_Parser_Tactic___aux__Init__Tactics______macroRules__Lean__Parser__Tactic__tacticAdmit__1___closed__18() {
 _start:
 {
 lean_object* x_1; lean_object* x_2; lean_object* x_3; 
 x_1 = lean_box(0);
-x_2 = l_Lean_Parser_Tactic___aux__Init__Tactics______macroRules__Lean__Parser__Tactic__tacticAdmit__1___closed__21;
+x_2 = l_Lean_Parser_Tactic___aux__Init__Tactics______macroRules__Lean__Parser__Tactic__tacticAdmit__1___closed__17;
 x_3 = lean_alloc_ctor(0, 2, 0);
 lean_ctor_set(x_3, 0, x_2);
 lean_ctor_set(x_3, 1, x_1);
 return x_3;
 }
 }
-static lean_object* _init_l_Lean_Parser_Tactic___aux__Init__Tactics______macroRules__Lean__Parser__Tactic__tacticAdmit__1___closed__23() {
+static lean_object* _init_l_Lean_Parser_Tactic___aux__Init__Tactics______macroRules__Lean__Parser__Tactic__tacticAdmit__1___closed__19() {
 _start:
 {
 lean_object* x_1; lean_object* x_2; lean_object* x_3; 
 x_1 = lean_box(0);
-x_2 = l_Lean_Parser_Tactic___aux__Init__Tactics______macroRules__Lean__Parser__Tactic__tacticAdmit__1___closed__22;
+x_2 = l_Lean_Parser_Tactic___aux__Init__Tactics______macroRules__Lean__Parser__Tactic__tacticAdmit__1___closed__18;
 x_3 = lean_alloc_ctor(1, 2, 0);
 lean_ctor_set(x_3, 0, x_2);
 lean_ctor_set(x_3, 1, x_1);
@@ -6421,17 +6442,17 @@ lean_inc(x_10);
 x_14 = lean_alloc_ctor(2, 2, 0);
 lean_ctor_set(x_14, 0, x_10);
 lean_ctor_set(x_14, 1, x_13);
-x_15 = l_Lean_Parser_Tactic___aux__Init__Tactics______macroRules__Lean__Parser__Tactic__tacticAdmit__1___closed__7;
+x_15 = l_Lean_Parser_Tactic___aux__Init__Tactics______macroRules__Lean__Parser__Tactic__tacticAdmit__1___closed__5;
 lean_inc(x_10);
 x_16 = lean_alloc_ctor(2, 2, 0);
 lean_ctor_set(x_16, 0, x_10);
 lean_ctor_set(x_16, 1, x_15);
-x_17 = l_Lean_Parser_Tactic___aux__Init__Tactics______macroRules__Lean__Parser__Tactic__tacticAdmit__1___closed__11;
+x_17 = l_Lean_Parser_Tactic___aux__Init__Tactics______macroRules__Lean__Parser__Tactic__tacticAdmit__1___closed__9;
 lean_inc(x_11);
 lean_inc(x_12);
 x_18 = l_Lean_addMacroScope(x_12, x_17, x_11);
-x_19 = l_Lean_Parser_Tactic___aux__Init__Tactics______macroRules__Lean__Parser__Tactic__tacticAdmit__1___closed__10;
-x_20 = l_Lean_Parser_Tactic___aux__Init__Tactics______macroRules__Lean__Parser__Tactic__tacticAdmit__1___closed__13;
+x_19 = l_Lean_Parser_Tactic___aux__Init__Tactics______macroRules__Lean__Parser__Tactic__tacticAdmit__1___closed__8;
+x_20 = l_Lean_Parser_Tactic___aux__Init__Tactics______macroRules__Lean__Parser__Tactic__tacticAdmit__1___closed__11;
 lean_inc(x_10);
 x_21 = lean_alloc_ctor(3, 4, 0);
 lean_ctor_set(x_21, 0, x_10);
@@ -6442,27 +6463,27 @@ x_22 = l_Lean_Parser_Tactic___aux__Init__Tactics______macroRules__Lean__Parser__
 x_23 = lean_array_push(x_22, x_16);
 x_24 = lean_array_push(x_23, x_21);
 x_25 = lean_box(2);
-x_26 = l_Lean_Parser_Tactic___aux__Init__Tactics______macroRules__Lean__Parser__Tactic__tacticAdmit__1___closed__6;
+x_26 = l_Lean_Parser_Tactic___aux__Init__Tactics______macroRules__Lean__Parser__Tactic__tacticAdmit__1___closed__4;
 x_27 = lean_alloc_ctor(1, 3, 0);
 lean_ctor_set(x_27, 0, x_25);
 lean_ctor_set(x_27, 1, x_26);
 lean_ctor_set(x_27, 2, x_24);
-x_28 = l_Lean_binderIdent___closed__10;
+x_28 = l_Lean_Parser_Tactic___aux__Init__Tactics______macroRules__Lean__Parser__Tactic__tacticNext___x3d_x3e____1___closed__4;
 lean_inc(x_10);
 x_29 = lean_alloc_ctor(2, 2, 0);
 lean_ctor_set(x_29, 0, x_10);
 lean_ctor_set(x_29, 1, x_28);
-x_30 = l_Lean_Parser_Tactic___aux__Init__Tactics______macroRules__Lean__Parser__Tactic__tacticNext___x3d_x3e____1___closed__1;
+x_30 = l_Lean_Parser_Tactic___aux__Init__Tactics______macroRules__Lean__Parser__Tactic__tacticNext___x3d_x3e____1___closed__5;
 x_31 = lean_array_push(x_30, x_29);
-x_32 = l_Lean_Parser_Tactic___aux__Init__Tactics______macroRules__Lean__Parser__Tactic__tacticAdmit__1___closed__15;
+x_32 = l_Lean_Parser_Tactic___aux__Init__Tactics______macroRules__Lean__Parser__Tactic__tacticNext___x3d_x3e____1___closed__3;
 x_33 = lean_alloc_ctor(1, 3, 0);
 lean_ctor_set(x_33, 0, x_25);
 lean_ctor_set(x_33, 1, x_32);
 lean_ctor_set(x_33, 2, x_31);
-x_34 = l_Lean_Parser_Tactic___aux__Init__Tactics______macroRules__Lean__Parser__Tactic__tacticAdmit__1___closed__18;
+x_34 = l_Lean_Parser_Tactic___aux__Init__Tactics______macroRules__Lean__Parser__Tactic__tacticAdmit__1___closed__14;
 x_35 = l_Lean_addMacroScope(x_12, x_34, x_11);
-x_36 = l_Lean_Parser_Tactic___aux__Init__Tactics______macroRules__Lean__Parser__Tactic__tacticAdmit__1___closed__17;
-x_37 = l_Lean_Parser_Tactic___aux__Init__Tactics______macroRules__Lean__Parser__Tactic__tacticAdmit__1___closed__23;
+x_36 = l_Lean_Parser_Tactic___aux__Init__Tactics______macroRules__Lean__Parser__Tactic__tacticAdmit__1___closed__13;
+x_37 = l_Lean_Parser_Tactic___aux__Init__Tactics______macroRules__Lean__Parser__Tactic__tacticAdmit__1___closed__19;
 x_38 = lean_alloc_ctor(3, 4, 0);
 lean_ctor_set(x_38, 0, x_10);
 lean_ctor_set(x_38, 1, x_36);
@@ -6470,14 +6491,14 @@ lean_ctor_set(x_38, 2, x_35);
 lean_ctor_set(x_38, 3, x_37);
 x_39 = lean_array_push(x_22, x_33);
 x_40 = lean_array_push(x_39, x_38);
-x_41 = l_Lean_Parser_Tactic___aux__Init__Tactics______macroRules__Lean__Parser__Tactic__tacticNext___x3d_x3e____1___closed__3;
+x_41 = l_Lean_Parser_Tactic___aux__Init__Tactics______macroRules__Lean__Parser__Tactic__tacticNext___x3d_x3e____1___closed__7;
 x_42 = lean_alloc_ctor(1, 3, 0);
 lean_ctor_set(x_42, 0, x_25);
 lean_ctor_set(x_42, 1, x_41);
 lean_ctor_set(x_42, 2, x_40);
 x_43 = lean_array_push(x_22, x_27);
 x_44 = lean_array_push(x_43, x_42);
-x_45 = l_Lean_Parser_Tactic___aux__Init__Tactics______macroRules__Lean__Parser__Tactic__tacticAdmit__1___closed__4;
+x_45 = l_Lean_Parser_Tactic___aux__Init__Tactics______macroRules__Lean__Parser__Tactic__tacticAdmit__1___closed__2;
 x_46 = lean_alloc_ctor(1, 3, 0);
 lean_ctor_set(x_46, 0, x_25);
 lean_ctor_set(x_46, 1, x_45);
@@ -6521,17 +6542,17 @@ lean_inc(x_56);
 x_61 = lean_alloc_ctor(2, 2, 0);
 lean_ctor_set(x_61, 0, x_56);
 lean_ctor_set(x_61, 1, x_60);
-x_62 = l_Lean_Parser_Tactic___aux__Init__Tactics______macroRules__Lean__Parser__Tactic__tacticAdmit__1___closed__7;
+x_62 = l_Lean_Parser_Tactic___aux__Init__Tactics______macroRules__Lean__Parser__Tactic__tacticAdmit__1___closed__5;
 lean_inc(x_56);
 x_63 = lean_alloc_ctor(2, 2, 0);
 lean_ctor_set(x_63, 0, x_56);
 lean_ctor_set(x_63, 1, x_62);
-x_64 = l_Lean_Parser_Tactic___aux__Init__Tactics______macroRules__Lean__Parser__Tactic__tacticAdmit__1___closed__11;
+x_64 = l_Lean_Parser_Tactic___aux__Init__Tactics______macroRules__Lean__Parser__Tactic__tacticAdmit__1___closed__9;
 lean_inc(x_58);
 lean_inc(x_59);
 x_65 = l_Lean_addMacroScope(x_59, x_64, x_58);
-x_66 = l_Lean_Parser_Tactic___aux__Init__Tactics______macroRules__Lean__Parser__Tactic__tacticAdmit__1___closed__10;
-x_67 = l_Lean_Parser_Tactic___aux__Init__Tactics______macroRules__Lean__Parser__Tactic__tacticAdmit__1___closed__13;
+x_66 = l_Lean_Parser_Tactic___aux__Init__Tactics______macroRules__Lean__Parser__Tactic__tacticAdmit__1___closed__8;
+x_67 = l_Lean_Parser_Tactic___aux__Init__Tactics______macroRules__Lean__Parser__Tactic__tacticAdmit__1___closed__11;
 lean_inc(x_56);
 x_68 = lean_alloc_ctor(3, 4, 0);
 lean_ctor_set(x_68, 0, x_56);
@@ -6542,27 +6563,27 @@ x_69 = l_Lean_Parser_Tactic___aux__Init__Tactics______macroRules__Lean__Parser__
 x_70 = lean_array_push(x_69, x_63);
 x_71 = lean_array_push(x_70, x_68);
 x_72 = lean_box(2);
-x_73 = l_Lean_Parser_Tactic___aux__Init__Tactics______macroRules__Lean__Parser__Tactic__tacticAdmit__1___closed__6;
+x_73 = l_Lean_Parser_Tactic___aux__Init__Tactics______macroRules__Lean__Parser__Tactic__tacticAdmit__1___closed__4;
 x_74 = lean_alloc_ctor(1, 3, 0);
 lean_ctor_set(x_74, 0, x_72);
 lean_ctor_set(x_74, 1, x_73);
 lean_ctor_set(x_74, 2, x_71);
-x_75 = l_Lean_binderIdent___closed__10;
+x_75 = l_Lean_Parser_Tactic___aux__Init__Tactics______macroRules__Lean__Parser__Tactic__tacticNext___x3d_x3e____1___closed__4;
 lean_inc(x_56);
 x_76 = lean_alloc_ctor(2, 2, 0);
 lean_ctor_set(x_76, 0, x_56);
 lean_ctor_set(x_76, 1, x_75);
-x_77 = l_Lean_Parser_Tactic___aux__Init__Tactics______macroRules__Lean__Parser__Tactic__tacticNext___x3d_x3e____1___closed__1;
+x_77 = l_Lean_Parser_Tactic___aux__Init__Tactics______macroRules__Lean__Parser__Tactic__tacticNext___x3d_x3e____1___closed__5;
 x_78 = lean_array_push(x_77, x_76);
-x_79 = l_Lean_Parser_Tactic___aux__Init__Tactics______macroRules__Lean__Parser__Tactic__tacticAdmit__1___closed__15;
+x_79 = l_Lean_Parser_Tactic___aux__Init__Tactics______macroRules__Lean__Parser__Tactic__tacticNext___x3d_x3e____1___closed__3;
 x_80 = lean_alloc_ctor(1, 3, 0);
 lean_ctor_set(x_80, 0, x_72);
 lean_ctor_set(x_80, 1, x_79);
 lean_ctor_set(x_80, 2, x_78);
-x_81 = l_Lean_Parser_Tactic___aux__Init__Tactics______macroRules__Lean__Parser__Tactic__tacticAdmit__1___closed__18;
+x_81 = l_Lean_Parser_Tactic___aux__Init__Tactics______macroRules__Lean__Parser__Tactic__tacticAdmit__1___closed__14;
 x_82 = l_Lean_addMacroScope(x_59, x_81, x_58);
-x_83 = l_Lean_Parser_Tactic___aux__Init__Tactics______macroRules__Lean__Parser__Tactic__tacticAdmit__1___closed__17;
-x_84 = l_Lean_Parser_Tactic___aux__Init__Tactics______macroRules__Lean__Parser__Tactic__tacticAdmit__1___closed__23;
+x_83 = l_Lean_Parser_Tactic___aux__Init__Tactics______macroRules__Lean__Parser__Tactic__tacticAdmit__1___closed__13;
+x_84 = l_Lean_Parser_Tactic___aux__Init__Tactics______macroRules__Lean__Parser__Tactic__tacticAdmit__1___closed__19;
 x_85 = lean_alloc_ctor(3, 4, 0);
 lean_ctor_set(x_85, 0, x_56);
 lean_ctor_set(x_85, 1, x_83);
@@ -6570,14 +6591,14 @@ lean_ctor_set(x_85, 2, x_82);
 lean_ctor_set(x_85, 3, x_84);
 x_86 = lean_array_push(x_69, x_80);
 x_87 = lean_array_push(x_86, x_85);
-x_88 = l_Lean_Parser_Tactic___aux__Init__Tactics______macroRules__Lean__Parser__Tactic__tacticNext___x3d_x3e____1___closed__3;
+x_88 = l_Lean_Parser_Tactic___aux__Init__Tactics______macroRules__Lean__Parser__Tactic__tacticNext___x3d_x3e____1___closed__7;
 x_89 = lean_alloc_ctor(1, 3, 0);
 lean_ctor_set(x_89, 0, x_72);
 lean_ctor_set(x_89, 1, x_88);
 lean_ctor_set(x_89, 2, x_87);
 x_90 = lean_array_push(x_69, x_74);
 x_91 = lean_array_push(x_90, x_89);
-x_92 = l_Lean_Parser_Tactic___aux__Init__Tactics______macroRules__Lean__Parser__Tactic__tacticAdmit__1___closed__4;
+x_92 = l_Lean_Parser_Tactic___aux__Init__Tactics______macroRules__Lean__Parser__Tactic__tacticAdmit__1___closed__2;
 x_93 = lean_alloc_ctor(1, 3, 0);
 lean_ctor_set(x_93, 0, x_72);
 lean_ctor_set(x_93, 1, x_92);
@@ -6704,17 +6725,17 @@ lean_inc(x_10);
 x_14 = lean_alloc_ctor(2, 2, 0);
 lean_ctor_set(x_14, 0, x_10);
 lean_ctor_set(x_14, 1, x_13);
-x_15 = l_Lean_Parser_Tactic___aux__Init__Tactics______macroRules__Lean__Parser__Tactic__tacticAdmit__1___closed__7;
+x_15 = l_Lean_Parser_Tactic___aux__Init__Tactics______macroRules__Lean__Parser__Tactic__tacticAdmit__1___closed__5;
 lean_inc(x_10);
 x_16 = lean_alloc_ctor(2, 2, 0);
 lean_ctor_set(x_16, 0, x_10);
 lean_ctor_set(x_16, 1, x_15);
-x_17 = l_Lean_Parser_Tactic___aux__Init__Tactics______macroRules__Lean__Parser__Tactic__tacticAdmit__1___closed__11;
+x_17 = l_Lean_Parser_Tactic___aux__Init__Tactics______macroRules__Lean__Parser__Tactic__tacticAdmit__1___closed__9;
 lean_inc(x_11);
 lean_inc(x_12);
 x_18 = l_Lean_addMacroScope(x_12, x_17, x_11);
-x_19 = l_Lean_Parser_Tactic___aux__Init__Tactics______macroRules__Lean__Parser__Tactic__tacticAdmit__1___closed__10;
-x_20 = l_Lean_Parser_Tactic___aux__Init__Tactics______macroRules__Lean__Parser__Tactic__tacticAdmit__1___closed__13;
+x_19 = l_Lean_Parser_Tactic___aux__Init__Tactics______macroRules__Lean__Parser__Tactic__tacticAdmit__1___closed__8;
+x_20 = l_Lean_Parser_Tactic___aux__Init__Tactics______macroRules__Lean__Parser__Tactic__tacticAdmit__1___closed__11;
 lean_inc(x_10);
 x_21 = lean_alloc_ctor(3, 4, 0);
 lean_ctor_set(x_21, 0, x_10);
@@ -6725,27 +6746,27 @@ x_22 = l_Lean_Parser_Tactic___aux__Init__Tactics______macroRules__Lean__Parser__
 x_23 = lean_array_push(x_22, x_16);
 x_24 = lean_array_push(x_23, x_21);
 x_25 = lean_box(2);
-x_26 = l_Lean_Parser_Tactic___aux__Init__Tactics______macroRules__Lean__Parser__Tactic__tacticAdmit__1___closed__6;
+x_26 = l_Lean_Parser_Tactic___aux__Init__Tactics______macroRules__Lean__Parser__Tactic__tacticAdmit__1___closed__4;
 x_27 = lean_alloc_ctor(1, 3, 0);
 lean_ctor_set(x_27, 0, x_25);
 lean_ctor_set(x_27, 1, x_26);
 lean_ctor_set(x_27, 2, x_24);
-x_28 = l_Lean_binderIdent___closed__10;
+x_28 = l_Lean_Parser_Tactic___aux__Init__Tactics______macroRules__Lean__Parser__Tactic__tacticNext___x3d_x3e____1___closed__4;
 lean_inc(x_10);
 x_29 = lean_alloc_ctor(2, 2, 0);
 lean_ctor_set(x_29, 0, x_10);
 lean_ctor_set(x_29, 1, x_28);
-x_30 = l_Lean_Parser_Tactic___aux__Init__Tactics______macroRules__Lean__Parser__Tactic__tacticNext___x3d_x3e____1___closed__1;
+x_30 = l_Lean_Parser_Tactic___aux__Init__Tactics______macroRules__Lean__Parser__Tactic__tacticNext___x3d_x3e____1___closed__5;
 x_31 = lean_array_push(x_30, x_29);
-x_32 = l_Lean_Parser_Tactic___aux__Init__Tactics______macroRules__Lean__Parser__Tactic__tacticAdmit__1___closed__15;
+x_32 = l_Lean_Parser_Tactic___aux__Init__Tactics______macroRules__Lean__Parser__Tactic__tacticNext___x3d_x3e____1___closed__3;
 x_33 = lean_alloc_ctor(1, 3, 0);
 lean_ctor_set(x_33, 0, x_25);
 lean_ctor_set(x_33, 1, x_32);
 lean_ctor_set(x_33, 2, x_31);
-x_34 = l_Lean_Parser_Tactic___aux__Init__Tactics______macroRules__Lean__Parser__Tactic__tacticAdmit__1___closed__18;
+x_34 = l_Lean_Parser_Tactic___aux__Init__Tactics______macroRules__Lean__Parser__Tactic__tacticAdmit__1___closed__14;
 x_35 = l_Lean_addMacroScope(x_12, x_34, x_11);
-x_36 = l_Lean_Parser_Tactic___aux__Init__Tactics______macroRules__Lean__Parser__Tactic__tacticAdmit__1___closed__17;
-x_37 = l_Lean_Parser_Tactic___aux__Init__Tactics______macroRules__Lean__Parser__Tactic__tacticAdmit__1___closed__23;
+x_36 = l_Lean_Parser_Tactic___aux__Init__Tactics______macroRules__Lean__Parser__Tactic__tacticAdmit__1___closed__13;
+x_37 = l_Lean_Parser_Tactic___aux__Init__Tactics______macroRules__Lean__Parser__Tactic__tacticAdmit__1___closed__19;
 x_38 = lean_alloc_ctor(3, 4, 0);
 lean_ctor_set(x_38, 0, x_10);
 lean_ctor_set(x_38, 1, x_36);
@@ -6753,14 +6774,14 @@ lean_ctor_set(x_38, 2, x_35);
 lean_ctor_set(x_38, 3, x_37);
 x_39 = lean_array_push(x_22, x_33);
 x_40 = lean_array_push(x_39, x_38);
-x_41 = l_Lean_Parser_Tactic___aux__Init__Tactics______macroRules__Lean__Parser__Tactic__tacticNext___x3d_x3e____1___closed__3;
+x_41 = l_Lean_Parser_Tactic___aux__Init__Tactics______macroRules__Lean__Parser__Tactic__tacticNext___x3d_x3e____1___closed__7;
 x_42 = lean_alloc_ctor(1, 3, 0);
 lean_ctor_set(x_42, 0, x_25);
 lean_ctor_set(x_42, 1, x_41);
 lean_ctor_set(x_42, 2, x_40);
 x_43 = lean_array_push(x_22, x_27);
 x_44 = lean_array_push(x_43, x_42);
-x_45 = l_Lean_Parser_Tactic___aux__Init__Tactics______macroRules__Lean__Parser__Tactic__tacticAdmit__1___closed__4;
+x_45 = l_Lean_Parser_Tactic___aux__Init__Tactics______macroRules__Lean__Parser__Tactic__tacticAdmit__1___closed__2;
 x_46 = lean_alloc_ctor(1, 3, 0);
 lean_ctor_set(x_46, 0, x_25);
 lean_ctor_set(x_46, 1, x_45);
@@ -6804,17 +6825,17 @@ lean_inc(x_56);
 x_61 = lean_alloc_ctor(2, 2, 0);
 lean_ctor_set(x_61, 0, x_56);
 lean_ctor_set(x_61, 1, x_60);
-x_62 = l_Lean_Parser_Tactic___aux__Init__Tactics______macroRules__Lean__Parser__Tactic__tacticAdmit__1___closed__7;
+x_62 = l_Lean_Parser_Tactic___aux__Init__Tactics______macroRules__Lean__Parser__Tactic__tacticAdmit__1___closed__5;
 lean_inc(x_56);
 x_63 = lean_alloc_ctor(2, 2, 0);
 lean_ctor_set(x_63, 0, x_56);
 lean_ctor_set(x_63, 1, x_62);
-x_64 = l_Lean_Parser_Tactic___aux__Init__Tactics______macroRules__Lean__Parser__Tactic__tacticAdmit__1___closed__11;
+x_64 = l_Lean_Parser_Tactic___aux__Init__Tactics______macroRules__Lean__Parser__Tactic__tacticAdmit__1___closed__9;
 lean_inc(x_58);
 lean_inc(x_59);
 x_65 = l_Lean_addMacroScope(x_59, x_64, x_58);
-x_66 = l_Lean_Parser_Tactic___aux__Init__Tactics______macroRules__Lean__Parser__Tactic__tacticAdmit__1___closed__10;
-x_67 = l_Lean_Parser_Tactic___aux__Init__Tactics______macroRules__Lean__Parser__Tactic__tacticAdmit__1___closed__13;
+x_66 = l_Lean_Parser_Tactic___aux__Init__Tactics______macroRules__Lean__Parser__Tactic__tacticAdmit__1___closed__8;
+x_67 = l_Lean_Parser_Tactic___aux__Init__Tactics______macroRules__Lean__Parser__Tactic__tacticAdmit__1___closed__11;
 lean_inc(x_56);
 x_68 = lean_alloc_ctor(3, 4, 0);
 lean_ctor_set(x_68, 0, x_56);
@@ -6825,27 +6846,27 @@ x_69 = l_Lean_Parser_Tactic___aux__Init__Tactics______macroRules__Lean__Parser__
 x_70 = lean_array_push(x_69, x_63);
 x_71 = lean_array_push(x_70, x_68);
 x_72 = lean_box(2);
-x_73 = l_Lean_Parser_Tactic___aux__Init__Tactics______macroRules__Lean__Parser__Tactic__tacticAdmit__1___closed__6;
+x_73 = l_Lean_Parser_Tactic___aux__Init__Tactics______macroRules__Lean__Parser__Tactic__tacticAdmit__1___closed__4;
 x_74 = lean_alloc_ctor(1, 3, 0);
 lean_ctor_set(x_74, 0, x_72);
 lean_ctor_set(x_74, 1, x_73);
 lean_ctor_set(x_74, 2, x_71);
-x_75 = l_Lean_binderIdent___closed__10;
+x_75 = l_Lean_Parser_Tactic___aux__Init__Tactics______macroRules__Lean__Parser__Tactic__tacticNext___x3d_x3e____1___closed__4;
 lean_inc(x_56);
 x_76 = lean_alloc_ctor(2, 2, 0);
 lean_ctor_set(x_76, 0, x_56);
 lean_ctor_set(x_76, 1, x_75);
-x_77 = l_Lean_Parser_Tactic___aux__Init__Tactics______macroRules__Lean__Parser__Tactic__tacticNext___x3d_x3e____1___closed__1;
+x_77 = l_Lean_Parser_Tactic___aux__Init__Tactics______macroRules__Lean__Parser__Tactic__tacticNext___x3d_x3e____1___closed__5;
 x_78 = lean_array_push(x_77, x_76);
-x_79 = l_Lean_Parser_Tactic___aux__Init__Tactics______macroRules__Lean__Parser__Tactic__tacticAdmit__1___closed__15;
+x_79 = l_Lean_Parser_Tactic___aux__Init__Tactics______macroRules__Lean__Parser__Tactic__tacticNext___x3d_x3e____1___closed__3;
 x_80 = lean_alloc_ctor(1, 3, 0);
 lean_ctor_set(x_80, 0, x_72);
 lean_ctor_set(x_80, 1, x_79);
 lean_ctor_set(x_80, 2, x_78);
-x_81 = l_Lean_Parser_Tactic___aux__Init__Tactics______macroRules__Lean__Parser__Tactic__tacticAdmit__1___closed__18;
+x_81 = l_Lean_Parser_Tactic___aux__Init__Tactics______macroRules__Lean__Parser__Tactic__tacticAdmit__1___closed__14;
 x_82 = l_Lean_addMacroScope(x_59, x_81, x_58);
-x_83 = l_Lean_Parser_Tactic___aux__Init__Tactics______macroRules__Lean__Parser__Tactic__tacticAdmit__1___closed__17;
-x_84 = l_Lean_Parser_Tactic___aux__Init__Tactics______macroRules__Lean__Parser__Tactic__tacticAdmit__1___closed__23;
+x_83 = l_Lean_Parser_Tactic___aux__Init__Tactics______macroRules__Lean__Parser__Tactic__tacticAdmit__1___closed__13;
+x_84 = l_Lean_Parser_Tactic___aux__Init__Tactics______macroRules__Lean__Parser__Tactic__tacticAdmit__1___closed__19;
 x_85 = lean_alloc_ctor(3, 4, 0);
 lean_ctor_set(x_85, 0, x_56);
 lean_ctor_set(x_85, 1, x_83);
@@ -6853,14 +6874,14 @@ lean_ctor_set(x_85, 2, x_82);
 lean_ctor_set(x_85, 3, x_84);
 x_86 = lean_array_push(x_69, x_80);
 x_87 = lean_array_push(x_86, x_85);
-x_88 = l_Lean_Parser_Tactic___aux__Init__Tactics______macroRules__Lean__Parser__Tactic__tacticNext___x3d_x3e____1___closed__3;
+x_88 = l_Lean_Parser_Tactic___aux__Init__Tactics______macroRules__Lean__Parser__Tactic__tacticNext___x3d_x3e____1___closed__7;
 x_89 = lean_alloc_ctor(1, 3, 0);
 lean_ctor_set(x_89, 0, x_72);
 lean_ctor_set(x_89, 1, x_88);
 lean_ctor_set(x_89, 2, x_87);
 x_90 = lean_array_push(x_69, x_74);
 x_91 = lean_array_push(x_90, x_89);
-x_92 = l_Lean_Parser_Tactic___aux__Init__Tactics______macroRules__Lean__Parser__Tactic__tacticAdmit__1___closed__4;
+x_92 = l_Lean_Parser_Tactic___aux__Init__Tactics______macroRules__Lean__Parser__Tactic__tacticAdmit__1___closed__2;
 x_93 = lean_alloc_ctor(1, 3, 0);
 lean_ctor_set(x_93, 0, x_72);
 lean_ctor_set(x_93, 1, x_92);
@@ -7070,9 +7091,9 @@ x_25 = lean_alloc_ctor(1, 3, 0);
 lean_ctor_set(x_25, 0, x_23);
 lean_ctor_set(x_25, 1, x_24);
 lean_ctor_set(x_25, 2, x_22);
-x_26 = l_Lean_Parser_Tactic___aux__Init__Tactics______macroRules__Lean__Parser__Tactic__tacticNext___x3d_x3e____1___closed__1;
+x_26 = l_Lean_Parser_Tactic___aux__Init__Tactics______macroRules__Lean__Parser__Tactic__tacticNext___x3d_x3e____1___closed__5;
 x_27 = lean_array_push(x_26, x_25);
-x_28 = l_Lean_Parser_Tactic___aux__Init__Tactics______macroRules__Lean__Parser__Tactic__tacticNext___x3d_x3e____1___closed__3;
+x_28 = l_Lean_Parser_Tactic___aux__Init__Tactics______macroRules__Lean__Parser__Tactic__tacticNext___x3d_x3e____1___closed__7;
 x_29 = lean_alloc_ctor(1, 3, 0);
 lean_ctor_set(x_29, 0, x_23);
 lean_ctor_set(x_29, 1, x_28);
@@ -7122,9 +7143,9 @@ x_49 = lean_alloc_ctor(1, 3, 0);
 lean_ctor_set(x_49, 0, x_47);
 lean_ctor_set(x_49, 1, x_48);
 lean_ctor_set(x_49, 2, x_46);
-x_50 = l_Lean_Parser_Tactic___aux__Init__Tactics______macroRules__Lean__Parser__Tactic__tacticNext___x3d_x3e____1___closed__1;
+x_50 = l_Lean_Parser_Tactic___aux__Init__Tactics______macroRules__Lean__Parser__Tactic__tacticNext___x3d_x3e____1___closed__5;
 x_51 = lean_array_push(x_50, x_49);
-x_52 = l_Lean_Parser_Tactic___aux__Init__Tactics______macroRules__Lean__Parser__Tactic__tacticNext___x3d_x3e____1___closed__3;
+x_52 = l_Lean_Parser_Tactic___aux__Init__Tactics______macroRules__Lean__Parser__Tactic__tacticNext___x3d_x3e____1___closed__7;
 x_53 = lean_alloc_ctor(1, 3, 0);
 lean_ctor_set(x_53, 0, x_47);
 lean_ctor_set(x_53, 1, x_52);
@@ -8304,7 +8325,7 @@ static lean_object* _init_l_Lean_Parser_Tactic___aux__Init__Tactics______macroRu
 _start:
 {
 lean_object* x_1; lean_object* x_2; 
-x_1 = l_Lean_Parser_Tactic___aux__Init__Tactics______macroRules__Lean__Parser__Tactic__tacticNext___x3d_x3e____1___closed__4;
+x_1 = l_Lean_Parser_Tactic___aux__Init__Tactics______macroRules__Lean__Parser__Tactic__tacticNext___x3d_x3e____1___closed__8;
 x_2 = l_Array_appendCore___rarg(x_1, x_1);
 return x_2;
 }
@@ -8314,7 +8335,7 @@ _start:
 {
 lean_object* x_1; lean_object* x_2; lean_object* x_3; lean_object* x_4; 
 x_1 = lean_box(2);
-x_2 = l_Lean_Parser_Tactic___aux__Init__Tactics______macroRules__Lean__Parser__Tactic__tacticNext___x3d_x3e____1___closed__3;
+x_2 = l_Lean_Parser_Tactic___aux__Init__Tactics______macroRules__Lean__Parser__Tactic__tacticNext___x3d_x3e____1___closed__7;
 x_3 = l_Lean_Parser_Tactic___aux__Init__Tactics______macroRules__Lean__Parser__Tactic__rwSeq__1___closed__6;
 x_4 = lean_alloc_ctor(1, 3, 0);
 lean_ctor_set(x_4, 0, x_1);
@@ -8463,11 +8484,11 @@ lean_inc(x_26);
 x_32 = lean_alloc_ctor(2, 2, 0);
 lean_ctor_set(x_32, 0, x_26);
 lean_ctor_set(x_32, 1, x_31);
-x_33 = l_Lean_Parser_Tactic___aux__Init__Tactics______macroRules__Lean__Parser__Tactic__tacticNext___x3d_x3e____1___closed__4;
+x_33 = l_Lean_Parser_Tactic___aux__Init__Tactics______macroRules__Lean__Parser__Tactic__tacticNext___x3d_x3e____1___closed__8;
 x_34 = l_Array_appendCore___rarg(x_33, x_24);
 lean_dec(x_24);
 x_35 = lean_box(2);
-x_36 = l_Lean_Parser_Tactic___aux__Init__Tactics______macroRules__Lean__Parser__Tactic__tacticNext___x3d_x3e____1___closed__3;
+x_36 = l_Lean_Parser_Tactic___aux__Init__Tactics______macroRules__Lean__Parser__Tactic__tacticNext___x3d_x3e____1___closed__7;
 x_37 = lean_alloc_ctor(1, 3, 0);
 lean_ctor_set(x_37, 0, x_35);
 lean_ctor_set(x_37, 1, x_36);
@@ -8517,7 +8538,7 @@ lean_inc(x_26);
 x_58 = lean_alloc_ctor(2, 2, 0);
 lean_ctor_set(x_58, 0, x_26);
 lean_ctor_set(x_58, 1, x_57);
-x_59 = l_Lean_Parser_Tactic___aux__Init__Tactics______macroRules__Lean__Parser__Tactic__tacticNext___x3d_x3e____1___closed__1;
+x_59 = l_Lean_Parser_Tactic___aux__Init__Tactics______macroRules__Lean__Parser__Tactic__tacticNext___x3d_x3e____1___closed__5;
 x_60 = lean_array_push(x_59, x_58);
 x_61 = l_Lean_Parser_Tactic_tacticRfl___closed__2;
 x_62 = lean_alloc_ctor(1, 3, 0);
@@ -10253,7 +10274,7 @@ static lean_object* _init_l_Lean_Parser_Tactic___aux__Init__Tactics______macroRu
 _start:
 {
 lean_object* x_1; lean_object* x_2; lean_object* x_3; 
-x_1 = l_Lean_Parser_Tactic___aux__Init__Tactics______macroRules__Lean__Parser__Tactic__tacticAdmit__1___closed__2;
+x_1 = l_Lean_Parser_Tactic___aux__Init__Tactics______macroRules__Lean__Parser__Tactic__tacticNext___x3d_x3e____1___closed__2;
 x_2 = l_Lean_Parser_Tactic___aux__Init__Tactics______macroRules__Lean__Parser__Tactic__tacticRefine__lift____1___closed__1;
 x_3 = l_Lean_Name_str___override(x_1, x_2);
 return x_3;
@@ -10338,9 +10359,9 @@ lean_inc(x_12);
 x_32 = lean_alloc_ctor(2, 2, 0);
 lean_ctor_set(x_32, 0, x_12);
 lean_ctor_set(x_32, 1, x_31);
-x_33 = l_Lean_Parser_Tactic___aux__Init__Tactics______macroRules__Lean__Parser__Tactic__tacticNext___x3d_x3e____1___closed__1;
+x_33 = l_Lean_Parser_Tactic___aux__Init__Tactics______macroRules__Lean__Parser__Tactic__tacticNext___x3d_x3e____1___closed__5;
 x_34 = lean_array_push(x_33, x_32);
-x_35 = l_Lean_Parser_Tactic___aux__Init__Tactics______macroRules__Lean__Parser__Tactic__tacticNext___x3d_x3e____1___closed__3;
+x_35 = l_Lean_Parser_Tactic___aux__Init__Tactics______macroRules__Lean__Parser__Tactic__tacticNext___x3d_x3e____1___closed__7;
 x_36 = lean_alloc_ctor(1, 3, 0);
 lean_ctor_set(x_36, 0, x_24);
 lean_ctor_set(x_36, 1, x_35);
@@ -10493,9 +10514,9 @@ lean_inc(x_86);
 x_107 = lean_alloc_ctor(2, 2, 0);
 lean_ctor_set(x_107, 0, x_86);
 lean_ctor_set(x_107, 1, x_106);
-x_108 = l_Lean_Parser_Tactic___aux__Init__Tactics______macroRules__Lean__Parser__Tactic__tacticNext___x3d_x3e____1___closed__1;
+x_108 = l_Lean_Parser_Tactic___aux__Init__Tactics______macroRules__Lean__Parser__Tactic__tacticNext___x3d_x3e____1___closed__5;
 x_109 = lean_array_push(x_108, x_107);
-x_110 = l_Lean_Parser_Tactic___aux__Init__Tactics______macroRules__Lean__Parser__Tactic__tacticNext___x3d_x3e____1___closed__3;
+x_110 = l_Lean_Parser_Tactic___aux__Init__Tactics______macroRules__Lean__Parser__Tactic__tacticNext___x3d_x3e____1___closed__7;
 x_111 = lean_alloc_ctor(1, 3, 0);
 lean_ctor_set(x_111, 0, x_99);
 lean_ctor_set(x_111, 1, x_110);
@@ -10726,7 +10747,7 @@ static lean_object* _init_l_Lean_Parser_Tactic___aux__Init__Tactics______macroRu
 _start:
 {
 lean_object* x_1; lean_object* x_2; lean_object* x_3; 
-x_1 = l_Lean_Parser_Tactic___aux__Init__Tactics______macroRules__Lean__Parser__Tactic__tacticAdmit__1___closed__2;
+x_1 = l_Lean_Parser_Tactic___aux__Init__Tactics______macroRules__Lean__Parser__Tactic__tacticNext___x3d_x3e____1___closed__2;
 x_2 = l_Lean_Parser_Tactic___aux__Init__Tactics______macroRules__Lean__Parser__Tactic__tacticHave____1___closed__2;
 x_3 = l_Lean_Name_str___override(x_1, x_2);
 return x_3;
@@ -10744,7 +10765,7 @@ static lean_object* _init_l_Lean_Parser_Tactic___aux__Init__Tactics______macroRu
 _start:
 {
 lean_object* x_1; lean_object* x_2; lean_object* x_3; 
-x_1 = l_Lean_Parser_Tactic___aux__Init__Tactics______macroRules__Lean__Parser__Tactic__tacticAdmit__1___closed__2;
+x_1 = l_Lean_Parser_Tactic___aux__Init__Tactics______macroRules__Lean__Parser__Tactic__tacticNext___x3d_x3e____1___closed__2;
 x_2 = l_Lean_Parser_Tactic___aux__Init__Tactics______macroRules__Lean__Parser__Tactic__tacticHave____1___closed__4;
 x_3 = l_Lean_Name_str___override(x_1, x_2);
 return x_3;
@@ -10808,14 +10829,14 @@ lean_inc(x_12);
 x_20 = lean_alloc_ctor(2, 2, 0);
 lean_ctor_set(x_20, 0, x_12);
 lean_ctor_set(x_20, 1, x_19);
-x_21 = l_Lean_binderIdent___closed__10;
+x_21 = l_Lean_Parser_Tactic___aux__Init__Tactics______macroRules__Lean__Parser__Tactic__tacticNext___x3d_x3e____1___closed__4;
 x_22 = lean_alloc_ctor(2, 2, 0);
 lean_ctor_set(x_22, 0, x_12);
 lean_ctor_set(x_22, 1, x_21);
-x_23 = l_Lean_Parser_Tactic___aux__Init__Tactics______macroRules__Lean__Parser__Tactic__tacticNext___x3d_x3e____1___closed__1;
+x_23 = l_Lean_Parser_Tactic___aux__Init__Tactics______macroRules__Lean__Parser__Tactic__tacticNext___x3d_x3e____1___closed__5;
 x_24 = lean_array_push(x_23, x_22);
 x_25 = lean_box(2);
-x_26 = l_Lean_Parser_Tactic___aux__Init__Tactics______macroRules__Lean__Parser__Tactic__tacticAdmit__1___closed__15;
+x_26 = l_Lean_Parser_Tactic___aux__Init__Tactics______macroRules__Lean__Parser__Tactic__tacticNext___x3d_x3e____1___closed__3;
 x_27 = lean_alloc_ctor(1, 3, 0);
 lean_ctor_set(x_27, 0, x_25);
 lean_ctor_set(x_27, 1, x_26);
@@ -10846,7 +10867,7 @@ lean_ctor_set(x_43, 0, x_25);
 lean_ctor_set(x_43, 1, x_42);
 lean_ctor_set(x_43, 2, x_41);
 x_44 = lean_array_push(x_23, x_43);
-x_45 = l_Lean_Parser_Tactic___aux__Init__Tactics______macroRules__Lean__Parser__Tactic__tacticNext___x3d_x3e____1___closed__3;
+x_45 = l_Lean_Parser_Tactic___aux__Init__Tactics______macroRules__Lean__Parser__Tactic__tacticNext___x3d_x3e____1___closed__7;
 x_46 = lean_alloc_ctor(1, 3, 0);
 lean_ctor_set(x_46, 0, x_25);
 lean_ctor_set(x_46, 1, x_45);
@@ -10888,14 +10909,14 @@ lean_inc(x_50);
 x_59 = lean_alloc_ctor(2, 2, 0);
 lean_ctor_set(x_59, 0, x_50);
 lean_ctor_set(x_59, 1, x_58);
-x_60 = l_Lean_binderIdent___closed__10;
+x_60 = l_Lean_Parser_Tactic___aux__Init__Tactics______macroRules__Lean__Parser__Tactic__tacticNext___x3d_x3e____1___closed__4;
 x_61 = lean_alloc_ctor(2, 2, 0);
 lean_ctor_set(x_61, 0, x_50);
 lean_ctor_set(x_61, 1, x_60);
-x_62 = l_Lean_Parser_Tactic___aux__Init__Tactics______macroRules__Lean__Parser__Tactic__tacticNext___x3d_x3e____1___closed__1;
+x_62 = l_Lean_Parser_Tactic___aux__Init__Tactics______macroRules__Lean__Parser__Tactic__tacticNext___x3d_x3e____1___closed__5;
 x_63 = lean_array_push(x_62, x_61);
 x_64 = lean_box(2);
-x_65 = l_Lean_Parser_Tactic___aux__Init__Tactics______macroRules__Lean__Parser__Tactic__tacticAdmit__1___closed__15;
+x_65 = l_Lean_Parser_Tactic___aux__Init__Tactics______macroRules__Lean__Parser__Tactic__tacticNext___x3d_x3e____1___closed__3;
 x_66 = lean_alloc_ctor(1, 3, 0);
 lean_ctor_set(x_66, 0, x_64);
 lean_ctor_set(x_66, 1, x_65);
@@ -10926,7 +10947,7 @@ lean_ctor_set(x_82, 0, x_64);
 lean_ctor_set(x_82, 1, x_81);
 lean_ctor_set(x_82, 2, x_80);
 x_83 = lean_array_push(x_62, x_82);
-x_84 = l_Lean_Parser_Tactic___aux__Init__Tactics______macroRules__Lean__Parser__Tactic__tacticNext___x3d_x3e____1___closed__3;
+x_84 = l_Lean_Parser_Tactic___aux__Init__Tactics______macroRules__Lean__Parser__Tactic__tacticNext___x3d_x3e____1___closed__7;
 x_85 = lean_alloc_ctor(1, 3, 0);
 lean_ctor_set(x_85, 0, x_64);
 lean_ctor_set(x_85, 1, x_84);
@@ -11043,7 +11064,7 @@ static lean_object* _init_l_Lean_Parser_Tactic___aux__Init__Tactics______macroRu
 _start:
 {
 lean_object* x_1; lean_object* x_2; lean_object* x_3; 
-x_1 = l_Lean_Parser_Tactic___aux__Init__Tactics______macroRules__Lean__Parser__Tactic__tacticAdmit__1___closed__2;
+x_1 = l_Lean_Parser_Tactic___aux__Init__Tactics______macroRules__Lean__Parser__Tactic__tacticNext___x3d_x3e____1___closed__2;
 x_2 = l_Lean_Parser_Tactic_tacticHave_____closed__5;
 x_3 = l_Lean_Name_str___override(x_1, x_2);
 return x_3;
@@ -11061,7 +11082,7 @@ static lean_object* _init_l_Lean_Parser_Tactic___aux__Init__Tactics______macroRu
 _start:
 {
 lean_object* x_1; lean_object* x_2; lean_object* x_3; 
-x_1 = l_Lean_Parser_Tactic___aux__Init__Tactics______macroRules__Lean__Parser__Tactic__tacticAdmit__1___closed__2;
+x_1 = l_Lean_Parser_Tactic___aux__Init__Tactics______macroRules__Lean__Parser__Tactic__tacticNext___x3d_x3e____1___closed__2;
 x_2 = l_Lean_Parser_Tactic___aux__Init__Tactics______macroRules__Lean__Parser__Tactic__tacticHave___x3a_x3d____1___closed__2;
 x_3 = l_Lean_Name_str___override(x_1, x_2);
 return x_3;
@@ -11079,7 +11100,7 @@ static lean_object* _init_l_Lean_Parser_Tactic___aux__Init__Tactics______macroRu
 _start:
 {
 lean_object* x_1; lean_object* x_2; lean_object* x_3; 
-x_1 = l_Lean_Parser_Tactic___aux__Init__Tactics______macroRules__Lean__Parser__Tactic__tacticAdmit__1___closed__2;
+x_1 = l_Lean_Parser_Tactic___aux__Init__Tactics______macroRules__Lean__Parser__Tactic__tacticNext___x3d_x3e____1___closed__2;
 x_2 = l_Lean_Parser_Tactic___aux__Init__Tactics______macroRules__Lean__Parser__Tactic__tacticHave___x3a_x3d____1___closed__4;
 x_3 = l_Lean_Name_str___override(x_1, x_2);
 return x_3;
@@ -11143,7 +11164,7 @@ x_18 = lean_array_push(x_17, x_9);
 x_19 = l_Lean_Parser_Tactic___aux__Init__Tactics______macroRules__Lean__Parser__Tactic__tacticTry____1___closed__7;
 x_20 = lean_array_push(x_18, x_19);
 x_21 = lean_box(2);
-x_22 = l_Lean_Parser_Tactic___aux__Init__Tactics______macroRules__Lean__Parser__Tactic__tacticNext___x3d_x3e____1___closed__3;
+x_22 = l_Lean_Parser_Tactic___aux__Init__Tactics______macroRules__Lean__Parser__Tactic__tacticNext___x3d_x3e____1___closed__7;
 x_23 = lean_alloc_ctor(1, 3, 0);
 lean_ctor_set(x_23, 0, x_21);
 lean_ctor_set(x_23, 1, x_22);
@@ -11153,14 +11174,14 @@ lean_inc(x_14);
 x_25 = lean_alloc_ctor(2, 2, 0);
 lean_ctor_set(x_25, 0, x_14);
 lean_ctor_set(x_25, 1, x_24);
-x_26 = l_Lean_binderIdent___closed__10;
+x_26 = l_Lean_Parser_Tactic___aux__Init__Tactics______macroRules__Lean__Parser__Tactic__tacticNext___x3d_x3e____1___closed__4;
 lean_inc(x_14);
 x_27 = lean_alloc_ctor(2, 2, 0);
 lean_ctor_set(x_27, 0, x_14);
 lean_ctor_set(x_27, 1, x_26);
-x_28 = l_Lean_Parser_Tactic___aux__Init__Tactics______macroRules__Lean__Parser__Tactic__tacticNext___x3d_x3e____1___closed__1;
+x_28 = l_Lean_Parser_Tactic___aux__Init__Tactics______macroRules__Lean__Parser__Tactic__tacticNext___x3d_x3e____1___closed__5;
 x_29 = lean_array_push(x_28, x_27);
-x_30 = l_Lean_Parser_Tactic___aux__Init__Tactics______macroRules__Lean__Parser__Tactic__tacticAdmit__1___closed__15;
+x_30 = l_Lean_Parser_Tactic___aux__Init__Tactics______macroRules__Lean__Parser__Tactic__tacticNext___x3d_x3e____1___closed__3;
 x_31 = lean_alloc_ctor(1, 3, 0);
 lean_ctor_set(x_31, 0, x_21);
 lean_ctor_set(x_31, 1, x_30);
@@ -11236,7 +11257,7 @@ x_64 = lean_array_push(x_63, x_9);
 x_65 = l_Lean_Parser_Tactic___aux__Init__Tactics______macroRules__Lean__Parser__Tactic__tacticTry____1___closed__7;
 x_66 = lean_array_push(x_64, x_65);
 x_67 = lean_box(2);
-x_68 = l_Lean_Parser_Tactic___aux__Init__Tactics______macroRules__Lean__Parser__Tactic__tacticNext___x3d_x3e____1___closed__3;
+x_68 = l_Lean_Parser_Tactic___aux__Init__Tactics______macroRules__Lean__Parser__Tactic__tacticNext___x3d_x3e____1___closed__7;
 x_69 = lean_alloc_ctor(1, 3, 0);
 lean_ctor_set(x_69, 0, x_67);
 lean_ctor_set(x_69, 1, x_68);
@@ -11246,14 +11267,14 @@ lean_inc(x_59);
 x_71 = lean_alloc_ctor(2, 2, 0);
 lean_ctor_set(x_71, 0, x_59);
 lean_ctor_set(x_71, 1, x_70);
-x_72 = l_Lean_binderIdent___closed__10;
+x_72 = l_Lean_Parser_Tactic___aux__Init__Tactics______macroRules__Lean__Parser__Tactic__tacticNext___x3d_x3e____1___closed__4;
 lean_inc(x_59);
 x_73 = lean_alloc_ctor(2, 2, 0);
 lean_ctor_set(x_73, 0, x_59);
 lean_ctor_set(x_73, 1, x_72);
-x_74 = l_Lean_Parser_Tactic___aux__Init__Tactics______macroRules__Lean__Parser__Tactic__tacticNext___x3d_x3e____1___closed__1;
+x_74 = l_Lean_Parser_Tactic___aux__Init__Tactics______macroRules__Lean__Parser__Tactic__tacticNext___x3d_x3e____1___closed__5;
 x_75 = lean_array_push(x_74, x_73);
-x_76 = l_Lean_Parser_Tactic___aux__Init__Tactics______macroRules__Lean__Parser__Tactic__tacticAdmit__1___closed__15;
+x_76 = l_Lean_Parser_Tactic___aux__Init__Tactics______macroRules__Lean__Parser__Tactic__tacticNext___x3d_x3e____1___closed__3;
 x_77 = lean_alloc_ctor(1, 3, 0);
 lean_ctor_set(x_77, 0, x_67);
 lean_ctor_set(x_77, 1, x_76);
@@ -11430,7 +11451,7 @@ static lean_object* _init_l_Lean_Parser_Tactic___aux__Init__Tactics______macroRu
 _start:
 {
 lean_object* x_1; lean_object* x_2; lean_object* x_3; 
-x_1 = l_Lean_Parser_Tactic___aux__Init__Tactics______macroRules__Lean__Parser__Tactic__tacticAdmit__1___closed__2;
+x_1 = l_Lean_Parser_Tactic___aux__Init__Tactics______macroRules__Lean__Parser__Tactic__tacticNext___x3d_x3e____1___closed__2;
 x_2 = l_Lean_Parser_Tactic___aux__Init__Tactics______macroRules__Lean__Parser__Tactic__tacticSuffices____1___closed__1;
 x_3 = l_Lean_Name_str___override(x_1, x_2);
 return x_3;
@@ -11486,14 +11507,14 @@ lean_inc(x_12);
 x_20 = lean_alloc_ctor(2, 2, 0);
 lean_ctor_set(x_20, 0, x_12);
 lean_ctor_set(x_20, 1, x_19);
-x_21 = l_Lean_binderIdent___closed__10;
+x_21 = l_Lean_Parser_Tactic___aux__Init__Tactics______macroRules__Lean__Parser__Tactic__tacticNext___x3d_x3e____1___closed__4;
 x_22 = lean_alloc_ctor(2, 2, 0);
 lean_ctor_set(x_22, 0, x_12);
 lean_ctor_set(x_22, 1, x_21);
-x_23 = l_Lean_Parser_Tactic___aux__Init__Tactics______macroRules__Lean__Parser__Tactic__tacticNext___x3d_x3e____1___closed__1;
+x_23 = l_Lean_Parser_Tactic___aux__Init__Tactics______macroRules__Lean__Parser__Tactic__tacticNext___x3d_x3e____1___closed__5;
 x_24 = lean_array_push(x_23, x_22);
 x_25 = lean_box(2);
-x_26 = l_Lean_Parser_Tactic___aux__Init__Tactics______macroRules__Lean__Parser__Tactic__tacticAdmit__1___closed__15;
+x_26 = l_Lean_Parser_Tactic___aux__Init__Tactics______macroRules__Lean__Parser__Tactic__tacticNext___x3d_x3e____1___closed__3;
 x_27 = lean_alloc_ctor(1, 3, 0);
 lean_ctor_set(x_27, 0, x_25);
 lean_ctor_set(x_27, 1, x_26);
@@ -11524,7 +11545,7 @@ lean_ctor_set(x_43, 0, x_25);
 lean_ctor_set(x_43, 1, x_42);
 lean_ctor_set(x_43, 2, x_41);
 x_44 = lean_array_push(x_23, x_43);
-x_45 = l_Lean_Parser_Tactic___aux__Init__Tactics______macroRules__Lean__Parser__Tactic__tacticNext___x3d_x3e____1___closed__3;
+x_45 = l_Lean_Parser_Tactic___aux__Init__Tactics______macroRules__Lean__Parser__Tactic__tacticNext___x3d_x3e____1___closed__7;
 x_46 = lean_alloc_ctor(1, 3, 0);
 lean_ctor_set(x_46, 0, x_25);
 lean_ctor_set(x_46, 1, x_45);
@@ -11566,14 +11587,14 @@ lean_inc(x_50);
 x_59 = lean_alloc_ctor(2, 2, 0);
 lean_ctor_set(x_59, 0, x_50);
 lean_ctor_set(x_59, 1, x_58);
-x_60 = l_Lean_binderIdent___closed__10;
+x_60 = l_Lean_Parser_Tactic___aux__Init__Tactics______macroRules__Lean__Parser__Tactic__tacticNext___x3d_x3e____1___closed__4;
 x_61 = lean_alloc_ctor(2, 2, 0);
 lean_ctor_set(x_61, 0, x_50);
 lean_ctor_set(x_61, 1, x_60);
-x_62 = l_Lean_Parser_Tactic___aux__Init__Tactics______macroRules__Lean__Parser__Tactic__tacticNext___x3d_x3e____1___closed__1;
+x_62 = l_Lean_Parser_Tactic___aux__Init__Tactics______macroRules__Lean__Parser__Tactic__tacticNext___x3d_x3e____1___closed__5;
 x_63 = lean_array_push(x_62, x_61);
 x_64 = lean_box(2);
-x_65 = l_Lean_Parser_Tactic___aux__Init__Tactics______macroRules__Lean__Parser__Tactic__tacticAdmit__1___closed__15;
+x_65 = l_Lean_Parser_Tactic___aux__Init__Tactics______macroRules__Lean__Parser__Tactic__tacticNext___x3d_x3e____1___closed__3;
 x_66 = lean_alloc_ctor(1, 3, 0);
 lean_ctor_set(x_66, 0, x_64);
 lean_ctor_set(x_66, 1, x_65);
@@ -11604,7 +11625,7 @@ lean_ctor_set(x_82, 0, x_64);
 lean_ctor_set(x_82, 1, x_81);
 lean_ctor_set(x_82, 2, x_80);
 x_83 = lean_array_push(x_62, x_82);
-x_84 = l_Lean_Parser_Tactic___aux__Init__Tactics______macroRules__Lean__Parser__Tactic__tacticNext___x3d_x3e____1___closed__3;
+x_84 = l_Lean_Parser_Tactic___aux__Init__Tactics______macroRules__Lean__Parser__Tactic__tacticNext___x3d_x3e____1___closed__7;
 x_85 = lean_alloc_ctor(1, 3, 0);
 lean_ctor_set(x_85, 0, x_64);
 lean_ctor_set(x_85, 1, x_84);
@@ -11737,7 +11758,7 @@ static lean_object* _init_l_Lean_Parser_Tactic___aux__Init__Tactics______macroRu
 _start:
 {
 lean_object* x_1; lean_object* x_2; lean_object* x_3; 
-x_1 = l_Lean_Parser_Tactic___aux__Init__Tactics______macroRules__Lean__Parser__Tactic__tacticAdmit__1___closed__2;
+x_1 = l_Lean_Parser_Tactic___aux__Init__Tactics______macroRules__Lean__Parser__Tactic__tacticNext___x3d_x3e____1___closed__2;
 x_2 = l_Lean_Parser_Tactic___aux__Init__Tactics______macroRules__Lean__Parser__Tactic__tacticLet____1___closed__1;
 x_3 = l_Lean_Name_str___override(x_1, x_2);
 return x_3;
@@ -11793,14 +11814,14 @@ lean_inc(x_12);
 x_20 = lean_alloc_ctor(2, 2, 0);
 lean_ctor_set(x_20, 0, x_12);
 lean_ctor_set(x_20, 1, x_19);
-x_21 = l_Lean_binderIdent___closed__10;
+x_21 = l_Lean_Parser_Tactic___aux__Init__Tactics______macroRules__Lean__Parser__Tactic__tacticNext___x3d_x3e____1___closed__4;
 x_22 = lean_alloc_ctor(2, 2, 0);
 lean_ctor_set(x_22, 0, x_12);
 lean_ctor_set(x_22, 1, x_21);
-x_23 = l_Lean_Parser_Tactic___aux__Init__Tactics______macroRules__Lean__Parser__Tactic__tacticNext___x3d_x3e____1___closed__1;
+x_23 = l_Lean_Parser_Tactic___aux__Init__Tactics______macroRules__Lean__Parser__Tactic__tacticNext___x3d_x3e____1___closed__5;
 x_24 = lean_array_push(x_23, x_22);
 x_25 = lean_box(2);
-x_26 = l_Lean_Parser_Tactic___aux__Init__Tactics______macroRules__Lean__Parser__Tactic__tacticAdmit__1___closed__15;
+x_26 = l_Lean_Parser_Tactic___aux__Init__Tactics______macroRules__Lean__Parser__Tactic__tacticNext___x3d_x3e____1___closed__3;
 x_27 = lean_alloc_ctor(1, 3, 0);
 lean_ctor_set(x_27, 0, x_25);
 lean_ctor_set(x_27, 1, x_26);
@@ -11831,7 +11852,7 @@ lean_ctor_set(x_43, 0, x_25);
 lean_ctor_set(x_43, 1, x_42);
 lean_ctor_set(x_43, 2, x_41);
 x_44 = lean_array_push(x_23, x_43);
-x_45 = l_Lean_Parser_Tactic___aux__Init__Tactics______macroRules__Lean__Parser__Tactic__tacticNext___x3d_x3e____1___closed__3;
+x_45 = l_Lean_Parser_Tactic___aux__Init__Tactics______macroRules__Lean__Parser__Tactic__tacticNext___x3d_x3e____1___closed__7;
 x_46 = lean_alloc_ctor(1, 3, 0);
 lean_ctor_set(x_46, 0, x_25);
 lean_ctor_set(x_46, 1, x_45);
@@ -11873,14 +11894,14 @@ lean_inc(x_50);
 x_59 = lean_alloc_ctor(2, 2, 0);
 lean_ctor_set(x_59, 0, x_50);
 lean_ctor_set(x_59, 1, x_58);
-x_60 = l_Lean_binderIdent___closed__10;
+x_60 = l_Lean_Parser_Tactic___aux__Init__Tactics______macroRules__Lean__Parser__Tactic__tacticNext___x3d_x3e____1___closed__4;
 x_61 = lean_alloc_ctor(2, 2, 0);
 lean_ctor_set(x_61, 0, x_50);
 lean_ctor_set(x_61, 1, x_60);
-x_62 = l_Lean_Parser_Tactic___aux__Init__Tactics______macroRules__Lean__Parser__Tactic__tacticNext___x3d_x3e____1___closed__1;
+x_62 = l_Lean_Parser_Tactic___aux__Init__Tactics______macroRules__Lean__Parser__Tactic__tacticNext___x3d_x3e____1___closed__5;
 x_63 = lean_array_push(x_62, x_61);
 x_64 = lean_box(2);
-x_65 = l_Lean_Parser_Tactic___aux__Init__Tactics______macroRules__Lean__Parser__Tactic__tacticAdmit__1___closed__15;
+x_65 = l_Lean_Parser_Tactic___aux__Init__Tactics______macroRules__Lean__Parser__Tactic__tacticNext___x3d_x3e____1___closed__3;
 x_66 = lean_alloc_ctor(1, 3, 0);
 lean_ctor_set(x_66, 0, x_64);
 lean_ctor_set(x_66, 1, x_65);
@@ -11911,7 +11932,7 @@ lean_ctor_set(x_82, 0, x_64);
 lean_ctor_set(x_82, 1, x_81);
 lean_ctor_set(x_82, 2, x_80);
 x_83 = lean_array_push(x_62, x_82);
-x_84 = l_Lean_Parser_Tactic___aux__Init__Tactics______macroRules__Lean__Parser__Tactic__tacticNext___x3d_x3e____1___closed__3;
+x_84 = l_Lean_Parser_Tactic___aux__Init__Tactics______macroRules__Lean__Parser__Tactic__tacticNext___x3d_x3e____1___closed__7;
 x_85 = lean_alloc_ctor(1, 3, 0);
 lean_ctor_set(x_85, 0, x_64);
 lean_ctor_set(x_85, 1, x_84);
@@ -12016,7 +12037,7 @@ static lean_object* _init_l_Lean_Parser_Tactic___aux__Init__Tactics______macroRu
 _start:
 {
 lean_object* x_1; lean_object* x_2; lean_object* x_3; 
-x_1 = l_Lean_Parser_Tactic___aux__Init__Tactics______macroRules__Lean__Parser__Tactic__tacticAdmit__1___closed__2;
+x_1 = l_Lean_Parser_Tactic___aux__Init__Tactics______macroRules__Lean__Parser__Tactic__tacticNext___x3d_x3e____1___closed__2;
 x_2 = l_Lean_Parser_Tactic___aux__Init__Tactics______macroRules__Lean__Parser__Tactic__tacticShow____1___closed__1;
 x_3 = l_Lean_Name_str___override(x_1, x_2);
 return x_3;
@@ -12034,7 +12055,7 @@ static lean_object* _init_l_Lean_Parser_Tactic___aux__Init__Tactics______macroRu
 _start:
 {
 lean_object* x_1; lean_object* x_2; lean_object* x_3; 
-x_1 = l_Lean_Parser_Tactic___aux__Init__Tactics______macroRules__Lean__Parser__Tactic__tacticAdmit__1___closed__2;
+x_1 = l_Lean_Parser_Tactic___aux__Init__Tactics______macroRules__Lean__Parser__Tactic__tacticNext___x3d_x3e____1___closed__2;
 x_2 = l_Lean_Parser_Tactic___aux__Init__Tactics______macroRules__Lean__Parser__Tactic__tacticShow____1___closed__3;
 x_3 = l_Lean_Name_str___override(x_1, x_2);
 return x_3;
@@ -12098,14 +12119,14 @@ lean_inc(x_12);
 x_20 = lean_alloc_ctor(2, 2, 0);
 lean_ctor_set(x_20, 0, x_12);
 lean_ctor_set(x_20, 1, x_19);
-x_21 = l_Lean_binderIdent___closed__10;
+x_21 = l_Lean_Parser_Tactic___aux__Init__Tactics______macroRules__Lean__Parser__Tactic__tacticNext___x3d_x3e____1___closed__4;
 x_22 = lean_alloc_ctor(2, 2, 0);
 lean_ctor_set(x_22, 0, x_12);
 lean_ctor_set(x_22, 1, x_21);
-x_23 = l_Lean_Parser_Tactic___aux__Init__Tactics______macroRules__Lean__Parser__Tactic__tacticNext___x3d_x3e____1___closed__1;
+x_23 = l_Lean_Parser_Tactic___aux__Init__Tactics______macroRules__Lean__Parser__Tactic__tacticNext___x3d_x3e____1___closed__5;
 x_24 = lean_array_push(x_23, x_22);
 x_25 = lean_box(2);
-x_26 = l_Lean_Parser_Tactic___aux__Init__Tactics______macroRules__Lean__Parser__Tactic__tacticAdmit__1___closed__15;
+x_26 = l_Lean_Parser_Tactic___aux__Init__Tactics______macroRules__Lean__Parser__Tactic__tacticNext___x3d_x3e____1___closed__3;
 x_27 = lean_alloc_ctor(1, 3, 0);
 lean_ctor_set(x_27, 0, x_25);
 lean_ctor_set(x_27, 1, x_26);
@@ -12142,7 +12163,7 @@ lean_ctor_set(x_46, 0, x_25);
 lean_ctor_set(x_46, 1, x_45);
 lean_ctor_set(x_46, 2, x_44);
 x_47 = lean_array_push(x_23, x_46);
-x_48 = l_Lean_Parser_Tactic___aux__Init__Tactics______macroRules__Lean__Parser__Tactic__tacticNext___x3d_x3e____1___closed__3;
+x_48 = l_Lean_Parser_Tactic___aux__Init__Tactics______macroRules__Lean__Parser__Tactic__tacticNext___x3d_x3e____1___closed__7;
 x_49 = lean_alloc_ctor(1, 3, 0);
 lean_ctor_set(x_49, 0, x_25);
 lean_ctor_set(x_49, 1, x_48);
@@ -12184,14 +12205,14 @@ lean_inc(x_53);
 x_62 = lean_alloc_ctor(2, 2, 0);
 lean_ctor_set(x_62, 0, x_53);
 lean_ctor_set(x_62, 1, x_61);
-x_63 = l_Lean_binderIdent___closed__10;
+x_63 = l_Lean_Parser_Tactic___aux__Init__Tactics______macroRules__Lean__Parser__Tactic__tacticNext___x3d_x3e____1___closed__4;
 x_64 = lean_alloc_ctor(2, 2, 0);
 lean_ctor_set(x_64, 0, x_53);
 lean_ctor_set(x_64, 1, x_63);
-x_65 = l_Lean_Parser_Tactic___aux__Init__Tactics______macroRules__Lean__Parser__Tactic__tacticNext___x3d_x3e____1___closed__1;
+x_65 = l_Lean_Parser_Tactic___aux__Init__Tactics______macroRules__Lean__Parser__Tactic__tacticNext___x3d_x3e____1___closed__5;
 x_66 = lean_array_push(x_65, x_64);
 x_67 = lean_box(2);
-x_68 = l_Lean_Parser_Tactic___aux__Init__Tactics______macroRules__Lean__Parser__Tactic__tacticAdmit__1___closed__15;
+x_68 = l_Lean_Parser_Tactic___aux__Init__Tactics______macroRules__Lean__Parser__Tactic__tacticNext___x3d_x3e____1___closed__3;
 x_69 = lean_alloc_ctor(1, 3, 0);
 lean_ctor_set(x_69, 0, x_67);
 lean_ctor_set(x_69, 1, x_68);
@@ -12228,7 +12249,7 @@ lean_ctor_set(x_88, 0, x_67);
 lean_ctor_set(x_88, 1, x_87);
 lean_ctor_set(x_88, 2, x_86);
 x_89 = lean_array_push(x_65, x_88);
-x_90 = l_Lean_Parser_Tactic___aux__Init__Tactics______macroRules__Lean__Parser__Tactic__tacticNext___x3d_x3e____1___closed__3;
+x_90 = l_Lean_Parser_Tactic___aux__Init__Tactics______macroRules__Lean__Parser__Tactic__tacticNext___x3d_x3e____1___closed__7;
 x_91 = lean_alloc_ctor(1, 3, 0);
 lean_ctor_set(x_91, 0, x_67);
 lean_ctor_set(x_91, 1, x_90);
@@ -12401,7 +12422,7 @@ static lean_object* _init_l_Lean_Parser_Tactic___aux__Init__Tactics______macroRu
 _start:
 {
 lean_object* x_1; lean_object* x_2; lean_object* x_3; 
-x_1 = l_Lean_Parser_Tactic___aux__Init__Tactics______macroRules__Lean__Parser__Tactic__tacticAdmit__1___closed__2;
+x_1 = l_Lean_Parser_Tactic___aux__Init__Tactics______macroRules__Lean__Parser__Tactic__tacticNext___x3d_x3e____1___closed__2;
 x_2 = l_Lean_Parser_Tactic_letrec___closed__1;
 x_3 = l_Lean_Name_str___override(x_1, x_2);
 return x_3;
@@ -12479,13 +12500,13 @@ lean_inc(x_12);
 x_28 = lean_alloc_ctor(2, 2, 0);
 lean_ctor_set(x_28, 0, x_12);
 lean_ctor_set(x_28, 1, x_27);
-x_29 = l_Lean_binderIdent___closed__10;
+x_29 = l_Lean_Parser_Tactic___aux__Init__Tactics______macroRules__Lean__Parser__Tactic__tacticNext___x3d_x3e____1___closed__4;
 x_30 = lean_alloc_ctor(2, 2, 0);
 lean_ctor_set(x_30, 0, x_12);
 lean_ctor_set(x_30, 1, x_29);
-x_31 = l_Lean_Parser_Tactic___aux__Init__Tactics______macroRules__Lean__Parser__Tactic__tacticNext___x3d_x3e____1___closed__1;
+x_31 = l_Lean_Parser_Tactic___aux__Init__Tactics______macroRules__Lean__Parser__Tactic__tacticNext___x3d_x3e____1___closed__5;
 x_32 = lean_array_push(x_31, x_30);
-x_33 = l_Lean_Parser_Tactic___aux__Init__Tactics______macroRules__Lean__Parser__Tactic__tacticAdmit__1___closed__15;
+x_33 = l_Lean_Parser_Tactic___aux__Init__Tactics______macroRules__Lean__Parser__Tactic__tacticNext___x3d_x3e____1___closed__3;
 x_34 = lean_alloc_ctor(1, 3, 0);
 lean_ctor_set(x_34, 0, x_22);
 lean_ctor_set(x_34, 1, x_33);
@@ -12559,13 +12580,13 @@ lean_inc(x_50);
 x_67 = lean_alloc_ctor(2, 2, 0);
 lean_ctor_set(x_67, 0, x_50);
 lean_ctor_set(x_67, 1, x_66);
-x_68 = l_Lean_binderIdent___closed__10;
+x_68 = l_Lean_Parser_Tactic___aux__Init__Tactics______macroRules__Lean__Parser__Tactic__tacticNext___x3d_x3e____1___closed__4;
 x_69 = lean_alloc_ctor(2, 2, 0);
 lean_ctor_set(x_69, 0, x_50);
 lean_ctor_set(x_69, 1, x_68);
-x_70 = l_Lean_Parser_Tactic___aux__Init__Tactics______macroRules__Lean__Parser__Tactic__tacticNext___x3d_x3e____1___closed__1;
+x_70 = l_Lean_Parser_Tactic___aux__Init__Tactics______macroRules__Lean__Parser__Tactic__tacticNext___x3d_x3e____1___closed__5;
 x_71 = lean_array_push(x_70, x_69);
-x_72 = l_Lean_Parser_Tactic___aux__Init__Tactics______macroRules__Lean__Parser__Tactic__tacticAdmit__1___closed__15;
+x_72 = l_Lean_Parser_Tactic___aux__Init__Tactics______macroRules__Lean__Parser__Tactic__tacticNext___x3d_x3e____1___closed__3;
 x_73 = lean_alloc_ctor(1, 3, 0);
 lean_ctor_set(x_73, 0, x_61);
 lean_ctor_set(x_73, 1, x_72);
@@ -12747,9 +12768,9 @@ lean_inc(x_12);
 x_32 = lean_alloc_ctor(2, 2, 0);
 lean_ctor_set(x_32, 0, x_12);
 lean_ctor_set(x_32, 1, x_31);
-x_33 = l_Lean_Parser_Tactic___aux__Init__Tactics______macroRules__Lean__Parser__Tactic__tacticNext___x3d_x3e____1___closed__1;
+x_33 = l_Lean_Parser_Tactic___aux__Init__Tactics______macroRules__Lean__Parser__Tactic__tacticNext___x3d_x3e____1___closed__5;
 x_34 = lean_array_push(x_33, x_32);
-x_35 = l_Lean_Parser_Tactic___aux__Init__Tactics______macroRules__Lean__Parser__Tactic__tacticNext___x3d_x3e____1___closed__3;
+x_35 = l_Lean_Parser_Tactic___aux__Init__Tactics______macroRules__Lean__Parser__Tactic__tacticNext___x3d_x3e____1___closed__7;
 x_36 = lean_alloc_ctor(1, 3, 0);
 lean_ctor_set(x_36, 0, x_24);
 lean_ctor_set(x_36, 1, x_35);
@@ -12902,9 +12923,9 @@ lean_inc(x_86);
 x_107 = lean_alloc_ctor(2, 2, 0);
 lean_ctor_set(x_107, 0, x_86);
 lean_ctor_set(x_107, 1, x_106);
-x_108 = l_Lean_Parser_Tactic___aux__Init__Tactics______macroRules__Lean__Parser__Tactic__tacticNext___x3d_x3e____1___closed__1;
+x_108 = l_Lean_Parser_Tactic___aux__Init__Tactics______macroRules__Lean__Parser__Tactic__tacticNext___x3d_x3e____1___closed__5;
 x_109 = lean_array_push(x_108, x_107);
-x_110 = l_Lean_Parser_Tactic___aux__Init__Tactics______macroRules__Lean__Parser__Tactic__tacticNext___x3d_x3e____1___closed__3;
+x_110 = l_Lean_Parser_Tactic___aux__Init__Tactics______macroRules__Lean__Parser__Tactic__tacticNext___x3d_x3e____1___closed__7;
 x_111 = lean_alloc_ctor(1, 3, 0);
 lean_ctor_set(x_111, 0, x_99);
 lean_ctor_set(x_111, 1, x_110);
@@ -13145,14 +13166,14 @@ lean_inc(x_12);
 x_20 = lean_alloc_ctor(2, 2, 0);
 lean_ctor_set(x_20, 0, x_12);
 lean_ctor_set(x_20, 1, x_19);
-x_21 = l_Lean_binderIdent___closed__10;
+x_21 = l_Lean_Parser_Tactic___aux__Init__Tactics______macroRules__Lean__Parser__Tactic__tacticNext___x3d_x3e____1___closed__4;
 x_22 = lean_alloc_ctor(2, 2, 0);
 lean_ctor_set(x_22, 0, x_12);
 lean_ctor_set(x_22, 1, x_21);
-x_23 = l_Lean_Parser_Tactic___aux__Init__Tactics______macroRules__Lean__Parser__Tactic__tacticNext___x3d_x3e____1___closed__1;
+x_23 = l_Lean_Parser_Tactic___aux__Init__Tactics______macroRules__Lean__Parser__Tactic__tacticNext___x3d_x3e____1___closed__5;
 x_24 = lean_array_push(x_23, x_22);
 x_25 = lean_box(2);
-x_26 = l_Lean_Parser_Tactic___aux__Init__Tactics______macroRules__Lean__Parser__Tactic__tacticAdmit__1___closed__15;
+x_26 = l_Lean_Parser_Tactic___aux__Init__Tactics______macroRules__Lean__Parser__Tactic__tacticNext___x3d_x3e____1___closed__3;
 x_27 = lean_alloc_ctor(1, 3, 0);
 lean_ctor_set(x_27, 0, x_25);
 lean_ctor_set(x_27, 1, x_26);
@@ -13183,7 +13204,7 @@ lean_ctor_set(x_43, 0, x_25);
 lean_ctor_set(x_43, 1, x_42);
 lean_ctor_set(x_43, 2, x_41);
 x_44 = lean_array_push(x_23, x_43);
-x_45 = l_Lean_Parser_Tactic___aux__Init__Tactics______macroRules__Lean__Parser__Tactic__tacticNext___x3d_x3e____1___closed__3;
+x_45 = l_Lean_Parser_Tactic___aux__Init__Tactics______macroRules__Lean__Parser__Tactic__tacticNext___x3d_x3e____1___closed__7;
 x_46 = lean_alloc_ctor(1, 3, 0);
 lean_ctor_set(x_46, 0, x_25);
 lean_ctor_set(x_46, 1, x_45);
@@ -13225,14 +13246,14 @@ lean_inc(x_50);
 x_59 = lean_alloc_ctor(2, 2, 0);
 lean_ctor_set(x_59, 0, x_50);
 lean_ctor_set(x_59, 1, x_58);
-x_60 = l_Lean_binderIdent___closed__10;
+x_60 = l_Lean_Parser_Tactic___aux__Init__Tactics______macroRules__Lean__Parser__Tactic__tacticNext___x3d_x3e____1___closed__4;
 x_61 = lean_alloc_ctor(2, 2, 0);
 lean_ctor_set(x_61, 0, x_50);
 lean_ctor_set(x_61, 1, x_60);
-x_62 = l_Lean_Parser_Tactic___aux__Init__Tactics______macroRules__Lean__Parser__Tactic__tacticNext___x3d_x3e____1___closed__1;
+x_62 = l_Lean_Parser_Tactic___aux__Init__Tactics______macroRules__Lean__Parser__Tactic__tacticNext___x3d_x3e____1___closed__5;
 x_63 = lean_array_push(x_62, x_61);
 x_64 = lean_box(2);
-x_65 = l_Lean_Parser_Tactic___aux__Init__Tactics______macroRules__Lean__Parser__Tactic__tacticAdmit__1___closed__15;
+x_65 = l_Lean_Parser_Tactic___aux__Init__Tactics______macroRules__Lean__Parser__Tactic__tacticNext___x3d_x3e____1___closed__3;
 x_66 = lean_alloc_ctor(1, 3, 0);
 lean_ctor_set(x_66, 0, x_64);
 lean_ctor_set(x_66, 1, x_65);
@@ -13263,7 +13284,7 @@ lean_ctor_set(x_82, 0, x_64);
 lean_ctor_set(x_82, 1, x_81);
 lean_ctor_set(x_82, 2, x_80);
 x_83 = lean_array_push(x_62, x_82);
-x_84 = l_Lean_Parser_Tactic___aux__Init__Tactics______macroRules__Lean__Parser__Tactic__tacticNext___x3d_x3e____1___closed__3;
+x_84 = l_Lean_Parser_Tactic___aux__Init__Tactics______macroRules__Lean__Parser__Tactic__tacticNext___x3d_x3e____1___closed__7;
 x_85 = lean_alloc_ctor(1, 3, 0);
 lean_ctor_set(x_85, 0, x_64);
 lean_ctor_set(x_85, 1, x_84);
@@ -13426,7 +13447,7 @@ x_18 = lean_array_push(x_17, x_9);
 x_19 = l_Lean_Parser_Tactic___aux__Init__Tactics______macroRules__Lean__Parser__Tactic__tacticTry____1___closed__7;
 x_20 = lean_array_push(x_18, x_19);
 x_21 = lean_box(2);
-x_22 = l_Lean_Parser_Tactic___aux__Init__Tactics______macroRules__Lean__Parser__Tactic__tacticNext___x3d_x3e____1___closed__3;
+x_22 = l_Lean_Parser_Tactic___aux__Init__Tactics______macroRules__Lean__Parser__Tactic__tacticNext___x3d_x3e____1___closed__7;
 x_23 = lean_alloc_ctor(1, 3, 0);
 lean_ctor_set(x_23, 0, x_21);
 lean_ctor_set(x_23, 1, x_22);
@@ -13436,14 +13457,14 @@ lean_inc(x_14);
 x_25 = lean_alloc_ctor(2, 2, 0);
 lean_ctor_set(x_25, 0, x_14);
 lean_ctor_set(x_25, 1, x_24);
-x_26 = l_Lean_binderIdent___closed__10;
+x_26 = l_Lean_Parser_Tactic___aux__Init__Tactics______macroRules__Lean__Parser__Tactic__tacticNext___x3d_x3e____1___closed__4;
 lean_inc(x_14);
 x_27 = lean_alloc_ctor(2, 2, 0);
 lean_ctor_set(x_27, 0, x_14);
 lean_ctor_set(x_27, 1, x_26);
-x_28 = l_Lean_Parser_Tactic___aux__Init__Tactics______macroRules__Lean__Parser__Tactic__tacticNext___x3d_x3e____1___closed__1;
+x_28 = l_Lean_Parser_Tactic___aux__Init__Tactics______macroRules__Lean__Parser__Tactic__tacticNext___x3d_x3e____1___closed__5;
 x_29 = lean_array_push(x_28, x_27);
-x_30 = l_Lean_Parser_Tactic___aux__Init__Tactics______macroRules__Lean__Parser__Tactic__tacticAdmit__1___closed__15;
+x_30 = l_Lean_Parser_Tactic___aux__Init__Tactics______macroRules__Lean__Parser__Tactic__tacticNext___x3d_x3e____1___closed__3;
 x_31 = lean_alloc_ctor(1, 3, 0);
 lean_ctor_set(x_31, 0, x_21);
 lean_ctor_set(x_31, 1, x_30);
@@ -13519,7 +13540,7 @@ x_64 = lean_array_push(x_63, x_9);
 x_65 = l_Lean_Parser_Tactic___aux__Init__Tactics______macroRules__Lean__Parser__Tactic__tacticTry____1___closed__7;
 x_66 = lean_array_push(x_64, x_65);
 x_67 = lean_box(2);
-x_68 = l_Lean_Parser_Tactic___aux__Init__Tactics______macroRules__Lean__Parser__Tactic__tacticNext___x3d_x3e____1___closed__3;
+x_68 = l_Lean_Parser_Tactic___aux__Init__Tactics______macroRules__Lean__Parser__Tactic__tacticNext___x3d_x3e____1___closed__7;
 x_69 = lean_alloc_ctor(1, 3, 0);
 lean_ctor_set(x_69, 0, x_67);
 lean_ctor_set(x_69, 1, x_68);
@@ -13529,14 +13550,14 @@ lean_inc(x_59);
 x_71 = lean_alloc_ctor(2, 2, 0);
 lean_ctor_set(x_71, 0, x_59);
 lean_ctor_set(x_71, 1, x_70);
-x_72 = l_Lean_binderIdent___closed__10;
+x_72 = l_Lean_Parser_Tactic___aux__Init__Tactics______macroRules__Lean__Parser__Tactic__tacticNext___x3d_x3e____1___closed__4;
 lean_inc(x_59);
 x_73 = lean_alloc_ctor(2, 2, 0);
 lean_ctor_set(x_73, 0, x_59);
 lean_ctor_set(x_73, 1, x_72);
-x_74 = l_Lean_Parser_Tactic___aux__Init__Tactics______macroRules__Lean__Parser__Tactic__tacticNext___x3d_x3e____1___closed__1;
+x_74 = l_Lean_Parser_Tactic___aux__Init__Tactics______macroRules__Lean__Parser__Tactic__tacticNext___x3d_x3e____1___closed__5;
 x_75 = lean_array_push(x_74, x_73);
-x_76 = l_Lean_Parser_Tactic___aux__Init__Tactics______macroRules__Lean__Parser__Tactic__tacticAdmit__1___closed__15;
+x_76 = l_Lean_Parser_Tactic___aux__Init__Tactics______macroRules__Lean__Parser__Tactic__tacticNext___x3d_x3e____1___closed__3;
 x_77 = lean_alloc_ctor(1, 3, 0);
 lean_ctor_set(x_77, 0, x_67);
 lean_ctor_set(x_77, 1, x_76);
@@ -13723,14 +13744,14 @@ lean_inc(x_12);
 x_20 = lean_alloc_ctor(2, 2, 0);
 lean_ctor_set(x_20, 0, x_12);
 lean_ctor_set(x_20, 1, x_19);
-x_21 = l_Lean_binderIdent___closed__10;
+x_21 = l_Lean_Parser_Tactic___aux__Init__Tactics______macroRules__Lean__Parser__Tactic__tacticNext___x3d_x3e____1___closed__4;
 x_22 = lean_alloc_ctor(2, 2, 0);
 lean_ctor_set(x_22, 0, x_12);
 lean_ctor_set(x_22, 1, x_21);
-x_23 = l_Lean_Parser_Tactic___aux__Init__Tactics______macroRules__Lean__Parser__Tactic__tacticNext___x3d_x3e____1___closed__1;
+x_23 = l_Lean_Parser_Tactic___aux__Init__Tactics______macroRules__Lean__Parser__Tactic__tacticNext___x3d_x3e____1___closed__5;
 x_24 = lean_array_push(x_23, x_22);
 x_25 = lean_box(2);
-x_26 = l_Lean_Parser_Tactic___aux__Init__Tactics______macroRules__Lean__Parser__Tactic__tacticAdmit__1___closed__15;
+x_26 = l_Lean_Parser_Tactic___aux__Init__Tactics______macroRules__Lean__Parser__Tactic__tacticNext___x3d_x3e____1___closed__3;
 x_27 = lean_alloc_ctor(1, 3, 0);
 lean_ctor_set(x_27, 0, x_25);
 lean_ctor_set(x_27, 1, x_26);
@@ -13761,7 +13782,7 @@ lean_ctor_set(x_43, 0, x_25);
 lean_ctor_set(x_43, 1, x_42);
 lean_ctor_set(x_43, 2, x_41);
 x_44 = lean_array_push(x_23, x_43);
-x_45 = l_Lean_Parser_Tactic___aux__Init__Tactics______macroRules__Lean__Parser__Tactic__tacticNext___x3d_x3e____1___closed__3;
+x_45 = l_Lean_Parser_Tactic___aux__Init__Tactics______macroRules__Lean__Parser__Tactic__tacticNext___x3d_x3e____1___closed__7;
 x_46 = lean_alloc_ctor(1, 3, 0);
 lean_ctor_set(x_46, 0, x_25);
 lean_ctor_set(x_46, 1, x_45);
@@ -13803,14 +13824,14 @@ lean_inc(x_50);
 x_59 = lean_alloc_ctor(2, 2, 0);
 lean_ctor_set(x_59, 0, x_50);
 lean_ctor_set(x_59, 1, x_58);
-x_60 = l_Lean_binderIdent___closed__10;
+x_60 = l_Lean_Parser_Tactic___aux__Init__Tactics______macroRules__Lean__Parser__Tactic__tacticNext___x3d_x3e____1___closed__4;
 x_61 = lean_alloc_ctor(2, 2, 0);
 lean_ctor_set(x_61, 0, x_50);
 lean_ctor_set(x_61, 1, x_60);
-x_62 = l_Lean_Parser_Tactic___aux__Init__Tactics______macroRules__Lean__Parser__Tactic__tacticNext___x3d_x3e____1___closed__1;
+x_62 = l_Lean_Parser_Tactic___aux__Init__Tactics______macroRules__Lean__Parser__Tactic__tacticNext___x3d_x3e____1___closed__5;
 x_63 = lean_array_push(x_62, x_61);
 x_64 = lean_box(2);
-x_65 = l_Lean_Parser_Tactic___aux__Init__Tactics______macroRules__Lean__Parser__Tactic__tacticAdmit__1___closed__15;
+x_65 = l_Lean_Parser_Tactic___aux__Init__Tactics______macroRules__Lean__Parser__Tactic__tacticNext___x3d_x3e____1___closed__3;
 x_66 = lean_alloc_ctor(1, 3, 0);
 lean_ctor_set(x_66, 0, x_64);
 lean_ctor_set(x_66, 1, x_65);
@@ -13841,7 +13862,7 @@ lean_ctor_set(x_82, 0, x_64);
 lean_ctor_set(x_82, 1, x_81);
 lean_ctor_set(x_82, 2, x_80);
 x_83 = lean_array_push(x_62, x_82);
-x_84 = l_Lean_Parser_Tactic___aux__Init__Tactics______macroRules__Lean__Parser__Tactic__tacticNext___x3d_x3e____1___closed__3;
+x_84 = l_Lean_Parser_Tactic___aux__Init__Tactics______macroRules__Lean__Parser__Tactic__tacticNext___x3d_x3e____1___closed__7;
 x_85 = lean_alloc_ctor(1, 3, 0);
 lean_ctor_set(x_85, 0, x_64);
 lean_ctor_set(x_85, 1, x_84);
@@ -13900,7 +13921,7 @@ static lean_object* _init_l_Lean_Parser_Tactic_inductionAltLHS___closed__5() {
 _start:
 {
 lean_object* x_1; lean_object* x_2; 
-x_1 = l_Lean_Parser_Tactic___aux__Init__Tactics______macroRules__Lean__Parser__Tactic__tacticAdmit__1___closed__7;
+x_1 = l_Lean_Parser_Tactic___aux__Init__Tactics______macroRules__Lean__Parser__Tactic__tacticAdmit__1___closed__5;
 x_2 = lean_alloc_ctor(5, 1, 0);
 lean_ctor_set(x_2, 0, x_1);
 return x_2;
@@ -13950,7 +13971,7 @@ _start:
 lean_object* x_1; lean_object* x_2; lean_object* x_3; lean_object* x_4; 
 x_1 = l_Lean_binderIdent___closed__6;
 x_2 = l_Lean_Parser_Tactic_inductionAltLHS___closed__8;
-x_3 = l_Lean_binderIdent___closed__11;
+x_3 = l_Lean_binderIdent___closed__12;
 x_4 = lean_alloc_ctor(2, 3, 0);
 lean_ctor_set(x_4, 0, x_1);
 lean_ctor_set(x_4, 1, x_2);
@@ -13977,7 +13998,7 @@ _start:
 {
 lean_object* x_1; lean_object* x_2; lean_object* x_3; 
 x_1 = l_Lean_Parser_Tactic_intro___closed__12;
-x_2 = l_Lean_binderIdent___closed__12;
+x_2 = l_Lean_binderIdent___closed__13;
 x_3 = lean_alloc_ctor(1, 2, 0);
 lean_ctor_set(x_3, 0, x_1);
 lean_ctor_set(x_3, 1, x_2);
@@ -14141,7 +14162,7 @@ _start:
 {
 lean_object* x_1; lean_object* x_2; lean_object* x_3; 
 x_1 = lean_box(0);
-x_2 = l_Lean_Parser_Tactic___aux__Init__Tactics______macroRules__Lean__Parser__Tactic__tacticAdmit__1___closed__14;
+x_2 = l_Lean_Parser_Tactic___aux__Init__Tactics______macroRules__Lean__Parser__Tactic__tacticHave____1___closed__4;
 x_3 = l_Lean_Name_str___override(x_1, x_2);
 return x_3;
 }
@@ -14159,30 +14180,38 @@ return x_2;
 static lean_object* _init_l_Lean_Parser_Tactic_inductionAlt___closed__14() {
 _start:
 {
-lean_object* x_1; lean_object* x_2; lean_object* x_3; 
-x_1 = lean_box(0);
-x_2 = l_Lean_Parser_Tactic___aux__Init__Tactics______macroRules__Lean__Parser__Tactic__tacticHave____1___closed__4;
-x_3 = l_Lean_Name_str___override(x_1, x_2);
-return x_3;
+lean_object* x_1; lean_object* x_2; lean_object* x_3; lean_object* x_4; 
+x_1 = l_Lean_binderIdent___closed__6;
+x_2 = l_Lean_Parser_Tactic_inductionAlt___closed__13;
+x_3 = l_Lean_Parser_Tactic_case___closed__11;
+x_4 = lean_alloc_ctor(2, 3, 0);
+lean_ctor_set(x_4, 0, x_1);
+lean_ctor_set(x_4, 1, x_2);
+lean_ctor_set(x_4, 2, x_3);
+return x_4;
 }
 }
 static lean_object* _init_l_Lean_Parser_Tactic_inductionAlt___closed__15() {
 _start:
 {
-lean_object* x_1; lean_object* x_2; 
-x_1 = l_Lean_Parser_Tactic_inductionAlt___closed__14;
-x_2 = lean_alloc_ctor(0, 1, 0);
-lean_ctor_set(x_2, 0, x_1);
-return x_2;
+lean_object* x_1; lean_object* x_2; lean_object* x_3; lean_object* x_4; 
+x_1 = l_Lean_binderIdent___closed__6;
+x_2 = l_Lean_binderIdent___closed__12;
+x_3 = l_Lean_Parser_Tactic_inductionAlt___closed__14;
+x_4 = lean_alloc_ctor(2, 3, 0);
+lean_ctor_set(x_4, 0, x_1);
+lean_ctor_set(x_4, 1, x_2);
+lean_ctor_set(x_4, 2, x_3);
+return x_4;
 }
 }
 static lean_object* _init_l_Lean_Parser_Tactic_inductionAlt___closed__16() {
 _start:
 {
 lean_object* x_1; lean_object* x_2; lean_object* x_3; lean_object* x_4; 
-x_1 = l_Lean_binderIdent___closed__6;
-x_2 = l_Lean_Parser_Tactic_inductionAlt___closed__15;
-x_3 = l_Lean_Parser_Tactic_case___closed__11;
+x_1 = l_Lean_Parser_Tactic_withAnnotateState___closed__8;
+x_2 = l_Lean_Parser_Tactic_inductionAlt___closed__11;
+x_3 = l_Lean_Parser_Tactic_inductionAlt___closed__15;
 x_4 = lean_alloc_ctor(2, 3, 0);
 lean_ctor_set(x_4, 0, x_1);
 lean_ctor_set(x_4, 1, x_2);
@@ -14194,37 +14223,9 @@ static lean_object* _init_l_Lean_Parser_Tactic_inductionAlt___closed__17() {
 _start:
 {
 lean_object* x_1; lean_object* x_2; lean_object* x_3; lean_object* x_4; 
-x_1 = l_Lean_binderIdent___closed__6;
-x_2 = l_Lean_Parser_Tactic_inductionAlt___closed__13;
-x_3 = l_Lean_Parser_Tactic_inductionAlt___closed__16;
-x_4 = lean_alloc_ctor(2, 3, 0);
-lean_ctor_set(x_4, 0, x_1);
-lean_ctor_set(x_4, 1, x_2);
-lean_ctor_set(x_4, 2, x_3);
-return x_4;
-}
-}
-static lean_object* _init_l_Lean_Parser_Tactic_inductionAlt___closed__18() {
-_start:
-{
-lean_object* x_1; lean_object* x_2; lean_object* x_3; lean_object* x_4; 
-x_1 = l_Lean_Parser_Tactic_withAnnotateState___closed__8;
-x_2 = l_Lean_Parser_Tactic_inductionAlt___closed__11;
-x_3 = l_Lean_Parser_Tactic_inductionAlt___closed__17;
-x_4 = lean_alloc_ctor(2, 3, 0);
-lean_ctor_set(x_4, 0, x_1);
-lean_ctor_set(x_4, 1, x_2);
-lean_ctor_set(x_4, 2, x_3);
-return x_4;
-}
-}
-static lean_object* _init_l_Lean_Parser_Tactic_inductionAlt___closed__19() {
-_start:
-{
-lean_object* x_1; lean_object* x_2; lean_object* x_3; lean_object* x_4; 
 x_1 = l_Lean_Parser_Tactic_inductionAlt___closed__1;
 x_2 = l_Lean_Parser_Tactic_inductionAlt___closed__2;
-x_3 = l_Lean_Parser_Tactic_inductionAlt___closed__18;
+x_3 = l_Lean_Parser_Tactic_inductionAlt___closed__16;
 x_4 = lean_alloc_ctor(9, 3, 0);
 lean_ctor_set(x_4, 0, x_1);
 lean_ctor_set(x_4, 1, x_2);
@@ -14236,7 +14237,7 @@ static lean_object* _init_l_Lean_Parser_Tactic_inductionAlt() {
 _start:
 {
 lean_object* x_1; 
-x_1 = l_Lean_Parser_Tactic_inductionAlt___closed__19;
+x_1 = l_Lean_Parser_Tactic_inductionAlt___closed__17;
 return x_1;
 }
 }
@@ -15286,9 +15287,9 @@ lean_inc(x_12);
 x_29 = lean_alloc_ctor(2, 2, 0);
 lean_ctor_set(x_29, 0, x_12);
 lean_ctor_set(x_29, 1, x_28);
-x_30 = l_Lean_Parser_Tactic___aux__Init__Tactics______macroRules__Lean__Parser__Tactic__tacticNext___x3d_x3e____1___closed__1;
+x_30 = l_Lean_Parser_Tactic___aux__Init__Tactics______macroRules__Lean__Parser__Tactic__tacticNext___x3d_x3e____1___closed__5;
 x_31 = lean_array_push(x_30, x_29);
-x_32 = l_Lean_Parser_Tactic___aux__Init__Tactics______macroRules__Lean__Parser__Tactic__tacticNext___x3d_x3e____1___closed__3;
+x_32 = l_Lean_Parser_Tactic___aux__Init__Tactics______macroRules__Lean__Parser__Tactic__tacticNext___x3d_x3e____1___closed__7;
 x_33 = lean_alloc_ctor(1, 3, 0);
 lean_ctor_set(x_33, 0, x_25);
 lean_ctor_set(x_33, 1, x_32);
@@ -15440,9 +15441,9 @@ lean_inc(x_83);
 x_101 = lean_alloc_ctor(2, 2, 0);
 lean_ctor_set(x_101, 0, x_83);
 lean_ctor_set(x_101, 1, x_100);
-x_102 = l_Lean_Parser_Tactic___aux__Init__Tactics______macroRules__Lean__Parser__Tactic__tacticNext___x3d_x3e____1___closed__1;
+x_102 = l_Lean_Parser_Tactic___aux__Init__Tactics______macroRules__Lean__Parser__Tactic__tacticNext___x3d_x3e____1___closed__5;
 x_103 = lean_array_push(x_102, x_101);
-x_104 = l_Lean_Parser_Tactic___aux__Init__Tactics______macroRules__Lean__Parser__Tactic__tacticNext___x3d_x3e____1___closed__3;
+x_104 = l_Lean_Parser_Tactic___aux__Init__Tactics______macroRules__Lean__Parser__Tactic__tacticNext___x3d_x3e____1___closed__7;
 x_105 = lean_alloc_ctor(1, 3, 0);
 lean_ctor_set(x_105, 0, x_97);
 lean_ctor_set(x_105, 1, x_104);
@@ -15923,7 +15924,7 @@ x_13 = l_Lean_Parser_Tactic_tacticSorry___closed__3;
 x_14 = lean_alloc_ctor(2, 2, 0);
 lean_ctor_set(x_14, 0, x_10);
 lean_ctor_set(x_14, 1, x_13);
-x_15 = l_Lean_Parser_Tactic___aux__Init__Tactics______macroRules__Lean__Parser__Tactic__tacticNext___x3d_x3e____1___closed__1;
+x_15 = l_Lean_Parser_Tactic___aux__Init__Tactics______macroRules__Lean__Parser__Tactic__tacticNext___x3d_x3e____1___closed__5;
 x_16 = lean_array_push(x_15, x_14);
 x_17 = lean_box(2);
 x_18 = l_Lean_Parser_Tactic_tacticSorry___closed__2;
@@ -15941,7 +15942,7 @@ lean_ctor_set(x_25, 0, x_17);
 lean_ctor_set(x_25, 1, x_24);
 lean_ctor_set(x_25, 2, x_23);
 x_26 = lean_array_push(x_15, x_25);
-x_27 = l_Lean_Parser_Tactic___aux__Init__Tactics______macroRules__Lean__Parser__Tactic__tacticNext___x3d_x3e____1___closed__3;
+x_27 = l_Lean_Parser_Tactic___aux__Init__Tactics______macroRules__Lean__Parser__Tactic__tacticNext___x3d_x3e____1___closed__7;
 x_28 = lean_alloc_ctor(1, 3, 0);
 lean_ctor_set(x_28, 0, x_17);
 lean_ctor_set(x_28, 1, x_27);
@@ -15996,7 +15997,7 @@ x_48 = l_Lean_Parser_Tactic_tacticSorry___closed__3;
 x_49 = lean_alloc_ctor(2, 2, 0);
 lean_ctor_set(x_49, 0, x_44);
 lean_ctor_set(x_49, 1, x_48);
-x_50 = l_Lean_Parser_Tactic___aux__Init__Tactics______macroRules__Lean__Parser__Tactic__tacticNext___x3d_x3e____1___closed__1;
+x_50 = l_Lean_Parser_Tactic___aux__Init__Tactics______macroRules__Lean__Parser__Tactic__tacticNext___x3d_x3e____1___closed__5;
 x_51 = lean_array_push(x_50, x_49);
 x_52 = lean_box(2);
 x_53 = l_Lean_Parser_Tactic_tacticSorry___closed__2;
@@ -16014,7 +16015,7 @@ lean_ctor_set(x_60, 0, x_52);
 lean_ctor_set(x_60, 1, x_59);
 lean_ctor_set(x_60, 2, x_58);
 x_61 = lean_array_push(x_50, x_60);
-x_62 = l_Lean_Parser_Tactic___aux__Init__Tactics______macroRules__Lean__Parser__Tactic__tacticNext___x3d_x3e____1___closed__3;
+x_62 = l_Lean_Parser_Tactic___aux__Init__Tactics______macroRules__Lean__Parser__Tactic__tacticNext___x3d_x3e____1___closed__7;
 x_63 = lean_alloc_ctor(1, 3, 0);
 lean_ctor_set(x_63, 0, x_52);
 lean_ctor_set(x_63, 1, x_62);
@@ -16160,7 +16161,7 @@ x_11 = l_Lean_Parser_Tactic_assumption___closed__1;
 x_12 = lean_alloc_ctor(2, 2, 0);
 lean_ctor_set(x_12, 0, x_10);
 lean_ctor_set(x_12, 1, x_11);
-x_13 = l_Lean_Parser_Tactic___aux__Init__Tactics______macroRules__Lean__Parser__Tactic__tacticNext___x3d_x3e____1___closed__1;
+x_13 = l_Lean_Parser_Tactic___aux__Init__Tactics______macroRules__Lean__Parser__Tactic__tacticNext___x3d_x3e____1___closed__5;
 x_14 = lean_array_push(x_13, x_12);
 x_15 = lean_box(2);
 x_16 = l_Lean_Parser_Tactic_assumption___closed__2;
@@ -16183,7 +16184,7 @@ x_20 = l_Lean_Parser_Tactic_assumption___closed__1;
 x_21 = lean_alloc_ctor(2, 2, 0);
 lean_ctor_set(x_21, 0, x_18);
 lean_ctor_set(x_21, 1, x_20);
-x_22 = l_Lean_Parser_Tactic___aux__Init__Tactics______macroRules__Lean__Parser__Tactic__tacticNext___x3d_x3e____1___closed__1;
+x_22 = l_Lean_Parser_Tactic___aux__Init__Tactics______macroRules__Lean__Parser__Tactic__tacticNext___x3d_x3e____1___closed__5;
 x_23 = lean_array_push(x_22, x_21);
 x_24 = lean_box(2);
 x_25 = l_Lean_Parser_Tactic_assumption___closed__2;
@@ -16228,7 +16229,7 @@ x_11 = l_Lean_Parser_Tactic_tacticRfl___closed__3;
 x_12 = lean_alloc_ctor(2, 2, 0);
 lean_ctor_set(x_12, 0, x_10);
 lean_ctor_set(x_12, 1, x_11);
-x_13 = l_Lean_Parser_Tactic___aux__Init__Tactics______macroRules__Lean__Parser__Tactic__tacticNext___x3d_x3e____1___closed__1;
+x_13 = l_Lean_Parser_Tactic___aux__Init__Tactics______macroRules__Lean__Parser__Tactic__tacticNext___x3d_x3e____1___closed__5;
 x_14 = lean_array_push(x_13, x_12);
 x_15 = lean_box(2);
 x_16 = l_Lean_Parser_Tactic_tacticRfl___closed__2;
@@ -16251,7 +16252,7 @@ x_20 = l_Lean_Parser_Tactic_tacticRfl___closed__3;
 x_21 = lean_alloc_ctor(2, 2, 0);
 lean_ctor_set(x_21, 0, x_18);
 lean_ctor_set(x_21, 1, x_20);
-x_22 = l_Lean_Parser_Tactic___aux__Init__Tactics______macroRules__Lean__Parser__Tactic__tacticNext___x3d_x3e____1___closed__1;
+x_22 = l_Lean_Parser_Tactic___aux__Init__Tactics______macroRules__Lean__Parser__Tactic__tacticNext___x3d_x3e____1___closed__5;
 x_23 = lean_array_push(x_22, x_21);
 x_24 = lean_box(2);
 x_25 = l_Lean_Parser_Tactic_tacticRfl___closed__2;
@@ -16296,7 +16297,7 @@ x_11 = l_Lean_Parser_Tactic_contradiction___closed__1;
 x_12 = lean_alloc_ctor(2, 2, 0);
 lean_ctor_set(x_12, 0, x_10);
 lean_ctor_set(x_12, 1, x_11);
-x_13 = l_Lean_Parser_Tactic___aux__Init__Tactics______macroRules__Lean__Parser__Tactic__tacticNext___x3d_x3e____1___closed__1;
+x_13 = l_Lean_Parser_Tactic___aux__Init__Tactics______macroRules__Lean__Parser__Tactic__tacticNext___x3d_x3e____1___closed__5;
 x_14 = lean_array_push(x_13, x_12);
 x_15 = lean_box(2);
 x_16 = l_Lean_Parser_Tactic_contradiction___closed__2;
@@ -16319,7 +16320,7 @@ x_20 = l_Lean_Parser_Tactic_contradiction___closed__1;
 x_21 = lean_alloc_ctor(2, 2, 0);
 lean_ctor_set(x_21, 0, x_18);
 lean_ctor_set(x_21, 1, x_20);
-x_22 = l_Lean_Parser_Tactic___aux__Init__Tactics______macroRules__Lean__Parser__Tactic__tacticNext___x3d_x3e____1___closed__1;
+x_22 = l_Lean_Parser_Tactic___aux__Init__Tactics______macroRules__Lean__Parser__Tactic__tacticNext___x3d_x3e____1___closed__5;
 x_23 = lean_array_push(x_22, x_21);
 x_24 = lean_box(2);
 x_25 = l_Lean_Parser_Tactic_contradiction___closed__2;
@@ -16382,7 +16383,7 @@ x_11 = l_Lean_Parser_Tactic___aux__Init__Tactics______macroRules__Lean__Parser__
 x_12 = lean_alloc_ctor(2, 2, 0);
 lean_ctor_set(x_12, 0, x_10);
 lean_ctor_set(x_12, 1, x_11);
-x_13 = l_Lean_Parser_Tactic___aux__Init__Tactics______macroRules__Lean__Parser__Tactic__tacticNext___x3d_x3e____1___closed__1;
+x_13 = l_Lean_Parser_Tactic___aux__Init__Tactics______macroRules__Lean__Parser__Tactic__tacticNext___x3d_x3e____1___closed__5;
 x_14 = lean_array_push(x_13, x_12);
 x_15 = lean_box(2);
 x_16 = l_Lean_Parser_Tactic___aux__Init__Tactics______macroRules__Lean__Parser__Tactic__tacticTrivial__4___closed__2;
@@ -16405,7 +16406,7 @@ x_20 = l_Lean_Parser_Tactic___aux__Init__Tactics______macroRules__Lean__Parser__
 x_21 = lean_alloc_ctor(2, 2, 0);
 lean_ctor_set(x_21, 0, x_18);
 lean_ctor_set(x_21, 1, x_20);
-x_22 = l_Lean_Parser_Tactic___aux__Init__Tactics______macroRules__Lean__Parser__Tactic__tacticNext___x3d_x3e____1___closed__1;
+x_22 = l_Lean_Parser_Tactic___aux__Init__Tactics______macroRules__Lean__Parser__Tactic__tacticNext___x3d_x3e____1___closed__5;
 x_23 = lean_array_push(x_22, x_21);
 x_24 = lean_box(2);
 x_25 = l_Lean_Parser_Tactic___aux__Init__Tactics______macroRules__Lean__Parser__Tactic__tacticTrivial__4___closed__2;
@@ -16760,7 +16761,7 @@ x_28 = l_Lean_Parser_Tactic_tacticTrivial___closed__3;
 x_29 = lean_alloc_ctor(2, 2, 0);
 lean_ctor_set(x_29, 0, x_10);
 lean_ctor_set(x_29, 1, x_28);
-x_30 = l_Lean_Parser_Tactic___aux__Init__Tactics______macroRules__Lean__Parser__Tactic__tacticNext___x3d_x3e____1___closed__1;
+x_30 = l_Lean_Parser_Tactic___aux__Init__Tactics______macroRules__Lean__Parser__Tactic__tacticNext___x3d_x3e____1___closed__5;
 x_31 = lean_array_push(x_30, x_29);
 x_32 = lean_alloc_ctor(1, 3, 0);
 lean_ctor_set(x_32, 0, x_23);
@@ -16824,7 +16825,7 @@ x_58 = l_Lean_Parser_Tactic_tacticTrivial___closed__3;
 x_59 = lean_alloc_ctor(2, 2, 0);
 lean_ctor_set(x_59, 0, x_39);
 lean_ctor_set(x_59, 1, x_58);
-x_60 = l_Lean_Parser_Tactic___aux__Init__Tactics______macroRules__Lean__Parser__Tactic__tacticNext___x3d_x3e____1___closed__1;
+x_60 = l_Lean_Parser_Tactic___aux__Init__Tactics______macroRules__Lean__Parser__Tactic__tacticNext___x3d_x3e____1___closed__5;
 x_61 = lean_array_push(x_60, x_59);
 x_62 = lean_alloc_ctor(1, 3, 0);
 lean_ctor_set(x_62, 0, x_53);
@@ -17030,7 +17031,7 @@ x_24 = l_Lean_Parser_Tactic___aux__Init__Tactics______macroRules__Lean__Parser__
 x_25 = lean_alloc_ctor(2, 2, 0);
 lean_ctor_set(x_25, 0, x_12);
 lean_ctor_set(x_25, 1, x_24);
-x_26 = l_Lean_Parser_Tactic___aux__Init__Tactics______macroRules__Lean__Parser__Tactic__tacticNext___x3d_x3e____1___closed__6;
+x_26 = l_Lean_Parser_Tactic___aux__Init__Tactics______macroRules__Lean__Parser__Tactic__tacticNext___x3d_x3e____1___closed__10;
 x_27 = lean_array_push(x_26, x_16);
 x_28 = lean_array_push(x_27, x_21);
 x_29 = lean_array_push(x_28, x_23);
@@ -17042,9 +17043,9 @@ x_34 = lean_alloc_ctor(1, 3, 0);
 lean_ctor_set(x_34, 0, x_32);
 lean_ctor_set(x_34, 1, x_33);
 lean_ctor_set(x_34, 2, x_31);
-x_35 = l_Lean_Parser_Tactic___aux__Init__Tactics______macroRules__Lean__Parser__Tactic__tacticNext___x3d_x3e____1___closed__1;
+x_35 = l_Lean_Parser_Tactic___aux__Init__Tactics______macroRules__Lean__Parser__Tactic__tacticNext___x3d_x3e____1___closed__5;
 x_36 = lean_array_push(x_35, x_34);
-x_37 = l_Lean_Parser_Tactic___aux__Init__Tactics______macroRules__Lean__Parser__Tactic__tacticNext___x3d_x3e____1___closed__3;
+x_37 = l_Lean_Parser_Tactic___aux__Init__Tactics______macroRules__Lean__Parser__Tactic__tacticNext___x3d_x3e____1___closed__7;
 x_38 = lean_alloc_ctor(1, 3, 0);
 lean_ctor_set(x_38, 0, x_32);
 lean_ctor_set(x_38, 1, x_37);
@@ -17095,7 +17096,7 @@ x_55 = l_Lean_Parser_Tactic___aux__Init__Tactics______macroRules__Lean__Parser__
 x_56 = lean_alloc_ctor(2, 2, 0);
 lean_ctor_set(x_56, 0, x_42);
 lean_ctor_set(x_56, 1, x_55);
-x_57 = l_Lean_Parser_Tactic___aux__Init__Tactics______macroRules__Lean__Parser__Tactic__tacticNext___x3d_x3e____1___closed__6;
+x_57 = l_Lean_Parser_Tactic___aux__Init__Tactics______macroRules__Lean__Parser__Tactic__tacticNext___x3d_x3e____1___closed__10;
 x_58 = lean_array_push(x_57, x_47);
 x_59 = lean_array_push(x_58, x_52);
 x_60 = lean_array_push(x_59, x_54);
@@ -17107,9 +17108,9 @@ x_65 = lean_alloc_ctor(1, 3, 0);
 lean_ctor_set(x_65, 0, x_63);
 lean_ctor_set(x_65, 1, x_64);
 lean_ctor_set(x_65, 2, x_62);
-x_66 = l_Lean_Parser_Tactic___aux__Init__Tactics______macroRules__Lean__Parser__Tactic__tacticNext___x3d_x3e____1___closed__1;
+x_66 = l_Lean_Parser_Tactic___aux__Init__Tactics______macroRules__Lean__Parser__Tactic__tacticNext___x3d_x3e____1___closed__5;
 x_67 = lean_array_push(x_66, x_65);
-x_68 = l_Lean_Parser_Tactic___aux__Init__Tactics______macroRules__Lean__Parser__Tactic__tacticNext___x3d_x3e____1___closed__3;
+x_68 = l_Lean_Parser_Tactic___aux__Init__Tactics______macroRules__Lean__Parser__Tactic__tacticNext___x3d_x3e____1___closed__7;
 x_69 = lean_alloc_ctor(1, 3, 0);
 lean_ctor_set(x_69, 0, x_63);
 lean_ctor_set(x_69, 1, x_68);
@@ -17369,7 +17370,7 @@ x_11 = l_Lean_Parser_Tactic_skip___closed__1;
 x_12 = lean_alloc_ctor(2, 2, 0);
 lean_ctor_set(x_12, 0, x_10);
 lean_ctor_set(x_12, 1, x_11);
-x_13 = l_Lean_Parser_Tactic___aux__Init__Tactics______macroRules__Lean__Parser__Tactic__tacticNext___x3d_x3e____1___closed__1;
+x_13 = l_Lean_Parser_Tactic___aux__Init__Tactics______macroRules__Lean__Parser__Tactic__tacticNext___x3d_x3e____1___closed__5;
 x_14 = lean_array_push(x_13, x_12);
 x_15 = lean_box(2);
 x_16 = l_Lean_Parser_Tactic_skip___closed__2;
@@ -17378,7 +17379,7 @@ lean_ctor_set(x_17, 0, x_15);
 lean_ctor_set(x_17, 1, x_16);
 lean_ctor_set(x_17, 2, x_14);
 x_18 = lean_array_push(x_13, x_17);
-x_19 = l_Lean_Parser_Tactic___aux__Init__Tactics______macroRules__Lean__Parser__Tactic__tacticNext___x3d_x3e____1___closed__3;
+x_19 = l_Lean_Parser_Tactic___aux__Init__Tactics______macroRules__Lean__Parser__Tactic__tacticNext___x3d_x3e____1___closed__7;
 x_20 = lean_alloc_ctor(1, 3, 0);
 lean_ctor_set(x_20, 0, x_15);
 lean_ctor_set(x_20, 1, x_19);
@@ -17404,7 +17405,7 @@ x_26 = l_Lean_Parser_Tactic_skip___closed__1;
 x_27 = lean_alloc_ctor(2, 2, 0);
 lean_ctor_set(x_27, 0, x_24);
 lean_ctor_set(x_27, 1, x_26);
-x_28 = l_Lean_Parser_Tactic___aux__Init__Tactics______macroRules__Lean__Parser__Tactic__tacticNext___x3d_x3e____1___closed__1;
+x_28 = l_Lean_Parser_Tactic___aux__Init__Tactics______macroRules__Lean__Parser__Tactic__tacticNext___x3d_x3e____1___closed__5;
 x_29 = lean_array_push(x_28, x_27);
 x_30 = lean_box(2);
 x_31 = l_Lean_Parser_Tactic_skip___closed__2;
@@ -17413,7 +17414,7 @@ lean_ctor_set(x_32, 0, x_30);
 lean_ctor_set(x_32, 1, x_31);
 lean_ctor_set(x_32, 2, x_29);
 x_33 = lean_array_push(x_28, x_32);
-x_34 = l_Lean_Parser_Tactic___aux__Init__Tactics______macroRules__Lean__Parser__Tactic__tacticNext___x3d_x3e____1___closed__3;
+x_34 = l_Lean_Parser_Tactic___aux__Init__Tactics______macroRules__Lean__Parser__Tactic__tacticNext___x3d_x3e____1___closed__7;
 x_35 = lean_alloc_ctor(1, 3, 0);
 lean_ctor_set(x_35, 0, x_30);
 lean_ctor_set(x_35, 1, x_34);
@@ -17584,7 +17585,7 @@ static lean_object* _init_l_Lean_Parser_Tactic___aux__Init__Tactics______macroRu
 _start:
 {
 lean_object* x_1; lean_object* x_2; lean_object* x_3; 
-x_1 = l_Lean_Parser_Tactic___aux__Init__Tactics______macroRules__Lean__Parser__Tactic__tacticAdmit__1___closed__2;
+x_1 = l_Lean_Parser_Tactic___aux__Init__Tactics______macroRules__Lean__Parser__Tactic__tacticNext___x3d_x3e____1___closed__2;
 x_2 = l_Lean_Parser_Tactic___aux__Init__Tactics______macroRules__Lean__Parser__Tactic__tacticExists___x2c_x2c__1___closed__1;
 x_3 = l_Lean_Name_str___override(x_1, x_2);
 return x_3;
@@ -17653,7 +17654,7 @@ lean_inc(x_13);
 x_19 = lean_alloc_ctor(2, 2, 0);
 lean_ctor_set(x_19, 0, x_13);
 lean_ctor_set(x_19, 1, x_18);
-x_20 = l_Lean_Parser_Tactic___aux__Init__Tactics______macroRules__Lean__Parser__Tactic__tacticNext___x3d_x3e____1___closed__4;
+x_20 = l_Lean_Parser_Tactic___aux__Init__Tactics______macroRules__Lean__Parser__Tactic__tacticNext___x3d_x3e____1___closed__8;
 x_21 = l_Array_appendCore___rarg(x_20, x_10);
 lean_dec(x_10);
 x_22 = l_Lean_Parser_Tactic_rwRuleSeq___closed__7;
@@ -17667,15 +17668,15 @@ lean_inc(x_13);
 x_26 = lean_alloc_ctor(2, 2, 0);
 lean_ctor_set(x_26, 0, x_13);
 lean_ctor_set(x_26, 1, x_25);
-x_27 = l_Lean_binderIdent___closed__10;
+x_27 = l_Lean_Parser_Tactic___aux__Init__Tactics______macroRules__Lean__Parser__Tactic__tacticNext___x3d_x3e____1___closed__4;
 lean_inc(x_13);
 x_28 = lean_alloc_ctor(2, 2, 0);
 lean_ctor_set(x_28, 0, x_13);
 lean_ctor_set(x_28, 1, x_27);
-x_29 = l_Lean_Parser_Tactic___aux__Init__Tactics______macroRules__Lean__Parser__Tactic__tacticNext___x3d_x3e____1___closed__1;
+x_29 = l_Lean_Parser_Tactic___aux__Init__Tactics______macroRules__Lean__Parser__Tactic__tacticNext___x3d_x3e____1___closed__5;
 x_30 = lean_array_push(x_29, x_28);
 x_31 = lean_box(2);
-x_32 = l_Lean_Parser_Tactic___aux__Init__Tactics______macroRules__Lean__Parser__Tactic__tacticAdmit__1___closed__15;
+x_32 = l_Lean_Parser_Tactic___aux__Init__Tactics______macroRules__Lean__Parser__Tactic__tacticNext___x3d_x3e____1___closed__3;
 x_33 = lean_alloc_ctor(1, 3, 0);
 lean_ctor_set(x_33, 0, x_31);
 lean_ctor_set(x_33, 1, x_32);
@@ -17689,7 +17690,7 @@ lean_ctor_set(x_38, 0, x_31);
 lean_ctor_set(x_38, 1, x_37);
 lean_ctor_set(x_38, 2, x_36);
 x_39 = lean_array_push(x_24, x_38);
-x_40 = l_Lean_Parser_Tactic___aux__Init__Tactics______macroRules__Lean__Parser__Tactic__tacticNext___x3d_x3e____1___closed__3;
+x_40 = l_Lean_Parser_Tactic___aux__Init__Tactics______macroRules__Lean__Parser__Tactic__tacticNext___x3d_x3e____1___closed__7;
 x_41 = lean_alloc_ctor(1, 3, 0);
 lean_ctor_set(x_41, 0, x_31);
 lean_ctor_set(x_41, 1, x_40);
@@ -17839,7 +17840,7 @@ lean_inc(x_102);
 x_109 = lean_alloc_ctor(2, 2, 0);
 lean_ctor_set(x_109, 0, x_102);
 lean_ctor_set(x_109, 1, x_108);
-x_110 = l_Lean_Parser_Tactic___aux__Init__Tactics______macroRules__Lean__Parser__Tactic__tacticNext___x3d_x3e____1___closed__4;
+x_110 = l_Lean_Parser_Tactic___aux__Init__Tactics______macroRules__Lean__Parser__Tactic__tacticNext___x3d_x3e____1___closed__8;
 x_111 = l_Array_appendCore___rarg(x_110, x_10);
 lean_dec(x_10);
 x_112 = l_Lean_Parser_Tactic_rwRuleSeq___closed__7;
@@ -17853,15 +17854,15 @@ lean_inc(x_102);
 x_116 = lean_alloc_ctor(2, 2, 0);
 lean_ctor_set(x_116, 0, x_102);
 lean_ctor_set(x_116, 1, x_115);
-x_117 = l_Lean_binderIdent___closed__10;
+x_117 = l_Lean_Parser_Tactic___aux__Init__Tactics______macroRules__Lean__Parser__Tactic__tacticNext___x3d_x3e____1___closed__4;
 lean_inc(x_102);
 x_118 = lean_alloc_ctor(2, 2, 0);
 lean_ctor_set(x_118, 0, x_102);
 lean_ctor_set(x_118, 1, x_117);
-x_119 = l_Lean_Parser_Tactic___aux__Init__Tactics______macroRules__Lean__Parser__Tactic__tacticNext___x3d_x3e____1___closed__1;
+x_119 = l_Lean_Parser_Tactic___aux__Init__Tactics______macroRules__Lean__Parser__Tactic__tacticNext___x3d_x3e____1___closed__5;
 x_120 = lean_array_push(x_119, x_118);
 x_121 = lean_box(2);
-x_122 = l_Lean_Parser_Tactic___aux__Init__Tactics______macroRules__Lean__Parser__Tactic__tacticAdmit__1___closed__15;
+x_122 = l_Lean_Parser_Tactic___aux__Init__Tactics______macroRules__Lean__Parser__Tactic__tacticNext___x3d_x3e____1___closed__3;
 x_123 = lean_alloc_ctor(1, 3, 0);
 lean_ctor_set(x_123, 0, x_121);
 lean_ctor_set(x_123, 1, x_122);
@@ -17875,7 +17876,7 @@ lean_ctor_set(x_128, 0, x_121);
 lean_ctor_set(x_128, 1, x_127);
 lean_ctor_set(x_128, 2, x_126);
 x_129 = lean_array_push(x_114, x_128);
-x_130 = l_Lean_Parser_Tactic___aux__Init__Tactics______macroRules__Lean__Parser__Tactic__tacticNext___x3d_x3e____1___closed__3;
+x_130 = l_Lean_Parser_Tactic___aux__Init__Tactics______macroRules__Lean__Parser__Tactic__tacticNext___x3d_x3e____1___closed__7;
 x_131 = lean_alloc_ctor(1, 3, 0);
 lean_ctor_set(x_131, 0, x_121);
 lean_ctor_set(x_131, 1, x_130);
@@ -18321,7 +18322,7 @@ static lean_object* _init_l___aux__Init__Tactics______macroRules__term_u2039___u
 _start:
 {
 lean_object* x_1; lean_object* x_2; lean_object* x_3; 
-x_1 = l_Lean_Parser_Tactic___aux__Init__Tactics______macroRules__Lean__Parser__Tactic__tacticAdmit__1___closed__2;
+x_1 = l_Lean_Parser_Tactic___aux__Init__Tactics______macroRules__Lean__Parser__Tactic__tacticNext___x3d_x3e____1___closed__2;
 x_2 = l_Lean_Parser_Tactic_paren___closed__1;
 x_3 = l_Lean_Name_str___override(x_1, x_2);
 return x_3;
@@ -18339,7 +18340,7 @@ static lean_object* _init_l___aux__Init__Tactics______macroRules__term_u2039___u
 _start:
 {
 lean_object* x_1; lean_object* x_2; lean_object* x_3; 
-x_1 = l_Lean_Parser_Tactic___aux__Init__Tactics______macroRules__Lean__Parser__Tactic__tacticAdmit__1___closed__2;
+x_1 = l_Lean_Parser_Tactic___aux__Init__Tactics______macroRules__Lean__Parser__Tactic__tacticNext___x3d_x3e____1___closed__2;
 x_2 = l___aux__Init__Tactics______macroRules__term_u2039___u203a__1___closed__2;
 x_3 = l_Lean_Name_str___override(x_1, x_2);
 return x_3;
@@ -18365,7 +18366,7 @@ static lean_object* _init_l___aux__Init__Tactics______macroRules__term_u2039___u
 _start:
 {
 lean_object* x_1; lean_object* x_2; lean_object* x_3; 
-x_1 = l_Lean_Parser_Tactic___aux__Init__Tactics______macroRules__Lean__Parser__Tactic__tacticAdmit__1___closed__2;
+x_1 = l_Lean_Parser_Tactic___aux__Init__Tactics______macroRules__Lean__Parser__Tactic__tacticNext___x3d_x3e____1___closed__2;
 x_2 = l___aux__Init__Tactics______macroRules__term_u2039___u203a__1___closed__5;
 x_3 = l_Lean_Name_str___override(x_1, x_2);
 return x_3;
@@ -18416,7 +18417,7 @@ lean_inc(x_12);
 x_18 = lean_alloc_ctor(2, 2, 0);
 lean_ctor_set(x_18, 0, x_12);
 lean_ctor_set(x_18, 1, x_17);
-x_19 = l_Lean_Parser_Tactic___aux__Init__Tactics______macroRules__Lean__Parser__Tactic__tacticNext___x3d_x3e____1___closed__1;
+x_19 = l_Lean_Parser_Tactic___aux__Init__Tactics______macroRules__Lean__Parser__Tactic__tacticNext___x3d_x3e____1___closed__5;
 x_20 = lean_array_push(x_19, x_18);
 x_21 = lean_box(2);
 x_22 = l_Lean_Parser_Tactic_assumption___closed__2;
@@ -18434,7 +18435,7 @@ lean_ctor_set(x_29, 0, x_21);
 lean_ctor_set(x_29, 1, x_28);
 lean_ctor_set(x_29, 2, x_27);
 x_30 = lean_array_push(x_19, x_29);
-x_31 = l_Lean_Parser_Tactic___aux__Init__Tactics______macroRules__Lean__Parser__Tactic__tacticNext___x3d_x3e____1___closed__3;
+x_31 = l_Lean_Parser_Tactic___aux__Init__Tactics______macroRules__Lean__Parser__Tactic__tacticNext___x3d_x3e____1___closed__7;
 x_32 = lean_alloc_ctor(1, 3, 0);
 lean_ctor_set(x_32, 0, x_21);
 lean_ctor_set(x_32, 1, x_31);
@@ -18520,7 +18521,7 @@ lean_inc(x_62);
 x_69 = lean_alloc_ctor(2, 2, 0);
 lean_ctor_set(x_69, 0, x_62);
 lean_ctor_set(x_69, 1, x_68);
-x_70 = l_Lean_Parser_Tactic___aux__Init__Tactics______macroRules__Lean__Parser__Tactic__tacticNext___x3d_x3e____1___closed__1;
+x_70 = l_Lean_Parser_Tactic___aux__Init__Tactics______macroRules__Lean__Parser__Tactic__tacticNext___x3d_x3e____1___closed__5;
 x_71 = lean_array_push(x_70, x_69);
 x_72 = lean_box(2);
 x_73 = l_Lean_Parser_Tactic_assumption___closed__2;
@@ -18538,7 +18539,7 @@ lean_ctor_set(x_80, 0, x_72);
 lean_ctor_set(x_80, 1, x_79);
 lean_ctor_set(x_80, 2, x_78);
 x_81 = lean_array_push(x_70, x_80);
-x_82 = l_Lean_Parser_Tactic___aux__Init__Tactics______macroRules__Lean__Parser__Tactic__tacticNext___x3d_x3e____1___closed__3;
+x_82 = l_Lean_Parser_Tactic___aux__Init__Tactics______macroRules__Lean__Parser__Tactic__tacticNext___x3d_x3e____1___closed__7;
 x_83 = lean_alloc_ctor(1, 3, 0);
 lean_ctor_set(x_83, 0, x_72);
 lean_ctor_set(x_83, 1, x_82);
@@ -18695,7 +18696,7 @@ x_11 = l_Lean_Parser_Tactic_tacticTrivial___closed__3;
 x_12 = lean_alloc_ctor(2, 2, 0);
 lean_ctor_set(x_12, 0, x_10);
 lean_ctor_set(x_12, 1, x_11);
-x_13 = l_Lean_Parser_Tactic___aux__Init__Tactics______macroRules__Lean__Parser__Tactic__tacticNext___x3d_x3e____1___closed__1;
+x_13 = l_Lean_Parser_Tactic___aux__Init__Tactics______macroRules__Lean__Parser__Tactic__tacticNext___x3d_x3e____1___closed__5;
 x_14 = lean_array_push(x_13, x_12);
 x_15 = lean_box(2);
 x_16 = l_Lean_Parser_Tactic_tacticTrivial___closed__2;
@@ -18718,7 +18719,7 @@ x_20 = l_Lean_Parser_Tactic_tacticTrivial___closed__3;
 x_21 = lean_alloc_ctor(2, 2, 0);
 lean_ctor_set(x_21, 0, x_18);
 lean_ctor_set(x_21, 1, x_20);
-x_22 = l_Lean_Parser_Tactic___aux__Init__Tactics______macroRules__Lean__Parser__Tactic__tacticNext___x3d_x3e____1___closed__1;
+x_22 = l_Lean_Parser_Tactic___aux__Init__Tactics______macroRules__Lean__Parser__Tactic__tacticNext___x3d_x3e____1___closed__5;
 x_23 = lean_array_push(x_22, x_21);
 x_24 = lean_box(2);
 x_25 = l_Lean_Parser_Tactic_tacticTrivial___closed__2;
@@ -18746,7 +18747,7 @@ static lean_object* _init_l___aux__Init__Tactics______macroRules__tacticGet__ele
 _start:
 {
 lean_object* x_1; lean_object* x_2; lean_object* x_3; 
-x_1 = l_Lean_Parser_Tactic___aux__Init__Tactics______macroRules__Lean__Parser__Tactic__tacticAdmit__1___closed__2;
+x_1 = l_Lean_Parser_Tactic___aux__Init__Tactics______macroRules__Lean__Parser__Tactic__tacticNext___x3d_x3e____1___closed__2;
 x_2 = l___aux__Init__Tactics______macroRules__tacticGet__elem__tactic__trivial__2___closed__1;
 x_3 = l_Lean_Name_str___override(x_1, x_2);
 return x_3;
@@ -18772,7 +18773,7 @@ static lean_object* _init_l___aux__Init__Tactics______macroRules__tacticGet__ele
 _start:
 {
 lean_object* x_1; lean_object* x_2; lean_object* x_3; 
-x_1 = l_Lean_Parser_Tactic___aux__Init__Tactics______macroRules__Lean__Parser__Tactic__tacticAdmit__1___closed__2;
+x_1 = l_Lean_Parser_Tactic___aux__Init__Tactics______macroRules__Lean__Parser__Tactic__tacticNext___x3d_x3e____1___closed__2;
 x_2 = l___aux__Init__Tactics______macroRules__tacticGet__elem__tactic__trivial__2___closed__4;
 x_3 = l_Lean_Name_str___override(x_1, x_2);
 return x_3;
@@ -18790,7 +18791,7 @@ static lean_object* _init_l___aux__Init__Tactics______macroRules__tacticGet__ele
 _start:
 {
 lean_object* x_1; lean_object* x_2; lean_object* x_3; 
-x_1 = l_Lean_Parser_Tactic___aux__Init__Tactics______macroRules__Lean__Parser__Tactic__tacticAdmit__1___closed__2;
+x_1 = l_Lean_Parser_Tactic___aux__Init__Tactics______macroRules__Lean__Parser__Tactic__tacticNext___x3d_x3e____1___closed__2;
 x_2 = l___aux__Init__Tactics______macroRules__tacticGet__elem__tactic__trivial__2___closed__6;
 x_3 = l_Lean_Name_str___override(x_1, x_2);
 return x_3;
@@ -18882,7 +18883,7 @@ static lean_object* _init_l___aux__Init__Tactics______macroRules__tacticGet__ele
 _start:
 {
 lean_object* x_1; lean_object* x_2; lean_object* x_3; 
-x_1 = l_Lean_Parser_Tactic___aux__Init__Tactics______macroRules__Lean__Parser__Tactic__tacticAdmit__1___closed__20;
+x_1 = l_Lean_Parser_Tactic___aux__Init__Tactics______macroRules__Lean__Parser__Tactic__tacticAdmit__1___closed__16;
 x_2 = l___aux__Init__Tactics______macroRules__tacticGet__elem__tactic__trivial__2___closed__12;
 x_3 = l_Lean_Name_str___override(x_1, x_2);
 return x_3;
@@ -18924,7 +18925,7 @@ static lean_object* _init_l___aux__Init__Tactics______macroRules__tacticGet__ele
 _start:
 {
 lean_object* x_1; lean_object* x_2; lean_object* x_3; 
-x_1 = l_Lean_Parser_Tactic___aux__Init__Tactics______macroRules__Lean__Parser__Tactic__tacticAdmit__1___closed__2;
+x_1 = l_Lean_Parser_Tactic___aux__Init__Tactics______macroRules__Lean__Parser__Tactic__tacticNext___x3d_x3e____1___closed__2;
 x_2 = l___aux__Init__Tactics______macroRules__tacticGet__elem__tactic__trivial__2___closed__19;
 x_3 = l_Lean_Name_str___override(x_1, x_2);
 return x_3;
@@ -18934,7 +18935,7 @@ static lean_object* _init_l___aux__Init__Tactics______macroRules__tacticGet__ele
 _start:
 {
 lean_object* x_1; lean_object* x_2; lean_object* x_3; 
-x_1 = l_Lean_Parser_Tactic___aux__Init__Tactics______macroRules__Lean__Parser__Tactic__tacticNext___x3d_x3e____1___closed__1;
+x_1 = l_Lean_Parser_Tactic___aux__Init__Tactics______macroRules__Lean__Parser__Tactic__tacticNext___x3d_x3e____1___closed__5;
 x_2 = l_Lean_Parser_Tactic___aux__Init__Tactics______macroRules__Lean__Parser__Tactic__tacticTry____1___closed__7;
 x_3 = lean_array_push(x_1, x_2);
 return x_3;
@@ -19069,9 +19070,9 @@ x_45 = lean_alloc_ctor(1, 3, 0);
 lean_ctor_set(x_45, 0, x_32);
 lean_ctor_set(x_45, 1, x_44);
 lean_ctor_set(x_45, 2, x_43);
-x_46 = l_Lean_Parser_Tactic___aux__Init__Tactics______macroRules__Lean__Parser__Tactic__tacticNext___x3d_x3e____1___closed__1;
+x_46 = l_Lean_Parser_Tactic___aux__Init__Tactics______macroRules__Lean__Parser__Tactic__tacticNext___x3d_x3e____1___closed__5;
 x_47 = lean_array_push(x_46, x_45);
-x_48 = l_Lean_Parser_Tactic___aux__Init__Tactics______macroRules__Lean__Parser__Tactic__tacticNext___x3d_x3e____1___closed__3;
+x_48 = l_Lean_Parser_Tactic___aux__Init__Tactics______macroRules__Lean__Parser__Tactic__tacticNext___x3d_x3e____1___closed__7;
 x_49 = lean_alloc_ctor(1, 3, 0);
 lean_ctor_set(x_49, 0, x_32);
 lean_ctor_set(x_49, 1, x_48);
@@ -19099,7 +19100,7 @@ lean_inc(x_10);
 x_63 = lean_alloc_ctor(2, 2, 0);
 lean_ctor_set(x_63, 0, x_10);
 lean_ctor_set(x_63, 1, x_62);
-x_64 = l_Lean_Parser_Tactic___aux__Init__Tactics______macroRules__Lean__Parser__Tactic__tacticNext___x3d_x3e____1___closed__6;
+x_64 = l_Lean_Parser_Tactic___aux__Init__Tactics______macroRules__Lean__Parser__Tactic__tacticNext___x3d_x3e____1___closed__10;
 x_65 = lean_array_push(x_64, x_16);
 x_66 = lean_array_push(x_65, x_18);
 x_67 = lean_array_push(x_66, x_20);
@@ -19237,9 +19238,9 @@ x_132 = lean_alloc_ctor(1, 3, 0);
 lean_ctor_set(x_132, 0, x_119);
 lean_ctor_set(x_132, 1, x_131);
 lean_ctor_set(x_132, 2, x_130);
-x_133 = l_Lean_Parser_Tactic___aux__Init__Tactics______macroRules__Lean__Parser__Tactic__tacticNext___x3d_x3e____1___closed__1;
+x_133 = l_Lean_Parser_Tactic___aux__Init__Tactics______macroRules__Lean__Parser__Tactic__tacticNext___x3d_x3e____1___closed__5;
 x_134 = lean_array_push(x_133, x_132);
-x_135 = l_Lean_Parser_Tactic___aux__Init__Tactics______macroRules__Lean__Parser__Tactic__tacticNext___x3d_x3e____1___closed__3;
+x_135 = l_Lean_Parser_Tactic___aux__Init__Tactics______macroRules__Lean__Parser__Tactic__tacticNext___x3d_x3e____1___closed__7;
 x_136 = lean_alloc_ctor(1, 3, 0);
 lean_ctor_set(x_136, 0, x_119);
 lean_ctor_set(x_136, 1, x_135);
@@ -19267,7 +19268,7 @@ lean_inc(x_96);
 x_150 = lean_alloc_ctor(2, 2, 0);
 lean_ctor_set(x_150, 0, x_96);
 lean_ctor_set(x_150, 1, x_149);
-x_151 = l_Lean_Parser_Tactic___aux__Init__Tactics______macroRules__Lean__Parser__Tactic__tacticNext___x3d_x3e____1___closed__6;
+x_151 = l_Lean_Parser_Tactic___aux__Init__Tactics______macroRules__Lean__Parser__Tactic__tacticNext___x3d_x3e____1___closed__10;
 x_152 = lean_array_push(x_151, x_103);
 x_153 = lean_array_push(x_152, x_105);
 x_154 = lean_array_push(x_153, x_107);
@@ -19438,7 +19439,7 @@ lean_inc(x_10);
 x_16 = lean_alloc_ctor(2, 2, 0);
 lean_ctor_set(x_16, 0, x_10);
 lean_ctor_set(x_16, 1, x_15);
-x_17 = l_Lean_Parser_Tactic___aux__Init__Tactics______macroRules__Lean__Parser__Tactic__tacticNext___x3d_x3e____1___closed__1;
+x_17 = l_Lean_Parser_Tactic___aux__Init__Tactics______macroRules__Lean__Parser__Tactic__tacticNext___x3d_x3e____1___closed__5;
 x_18 = lean_array_push(x_17, x_16);
 x_19 = lean_box(2);
 x_20 = l_tacticGet__elem__tactic__trivial___closed__2;
@@ -19456,7 +19457,7 @@ lean_ctor_set(x_27, 0, x_19);
 lean_ctor_set(x_27, 1, x_26);
 lean_ctor_set(x_27, 2, x_25);
 x_28 = lean_array_push(x_17, x_27);
-x_29 = l_Lean_Parser_Tactic___aux__Init__Tactics______macroRules__Lean__Parser__Tactic__tacticNext___x3d_x3e____1___closed__3;
+x_29 = l_Lean_Parser_Tactic___aux__Init__Tactics______macroRules__Lean__Parser__Tactic__tacticNext___x3d_x3e____1___closed__7;
 x_30 = lean_alloc_ctor(1, 3, 0);
 lean_ctor_set(x_30, 0, x_19);
 lean_ctor_set(x_30, 1, x_29);
@@ -19583,7 +19584,7 @@ lean_inc(x_76);
 x_83 = lean_alloc_ctor(2, 2, 0);
 lean_ctor_set(x_83, 0, x_76);
 lean_ctor_set(x_83, 1, x_82);
-x_84 = l_Lean_Parser_Tactic___aux__Init__Tactics______macroRules__Lean__Parser__Tactic__tacticNext___x3d_x3e____1___closed__1;
+x_84 = l_Lean_Parser_Tactic___aux__Init__Tactics______macroRules__Lean__Parser__Tactic__tacticNext___x3d_x3e____1___closed__5;
 x_85 = lean_array_push(x_84, x_83);
 x_86 = lean_box(2);
 x_87 = l_tacticGet__elem__tactic__trivial___closed__2;
@@ -19601,7 +19602,7 @@ lean_ctor_set(x_94, 0, x_86);
 lean_ctor_set(x_94, 1, x_93);
 lean_ctor_set(x_94, 2, x_92);
 x_95 = lean_array_push(x_84, x_94);
-x_96 = l_Lean_Parser_Tactic___aux__Init__Tactics______macroRules__Lean__Parser__Tactic__tacticNext___x3d_x3e____1___closed__3;
+x_96 = l_Lean_Parser_Tactic___aux__Init__Tactics______macroRules__Lean__Parser__Tactic__tacticNext___x3d_x3e____1___closed__7;
 x_97 = lean_alloc_ctor(1, 3, 0);
 lean_ctor_set(x_97, 0, x_86);
 lean_ctor_set(x_97, 1, x_96);
@@ -19990,7 +19991,7 @@ lean_inc(x_14);
 x_27 = lean_alloc_ctor(2, 2, 0);
 lean_ctor_set(x_27, 0, x_14);
 lean_ctor_set(x_27, 1, x_26);
-x_28 = l_Lean_Parser_Tactic___aux__Init__Tactics______macroRules__Lean__Parser__Tactic__tacticNext___x3d_x3e____1___closed__1;
+x_28 = l_Lean_Parser_Tactic___aux__Init__Tactics______macroRules__Lean__Parser__Tactic__tacticNext___x3d_x3e____1___closed__5;
 x_29 = lean_array_push(x_28, x_27);
 x_30 = lean_box(2);
 x_31 = l_tacticGet__elem__tactic___closed__2;
@@ -20008,7 +20009,7 @@ lean_ctor_set(x_38, 0, x_30);
 lean_ctor_set(x_38, 1, x_37);
 lean_ctor_set(x_38, 2, x_36);
 x_39 = lean_array_push(x_28, x_38);
-x_40 = l_Lean_Parser_Tactic___aux__Init__Tactics______macroRules__Lean__Parser__Tactic__tacticNext___x3d_x3e____1___closed__3;
+x_40 = l_Lean_Parser_Tactic___aux__Init__Tactics______macroRules__Lean__Parser__Tactic__tacticNext___x3d_x3e____1___closed__7;
 x_41 = lean_alloc_ctor(1, 3, 0);
 lean_ctor_set(x_41, 0, x_30);
 lean_ctor_set(x_41, 1, x_40);
@@ -20060,7 +20061,7 @@ lean_ctor_set(x_66, 1, x_40);
 lean_ctor_set(x_66, 2, x_65);
 x_67 = lean_array_push(x_33, x_21);
 x_68 = lean_array_push(x_67, x_66);
-x_69 = l_Lean_Parser_Tactic___aux__Init__Tactics______macroRules__Lean__Parser__Tactic__tacticAdmit__1___closed__4;
+x_69 = l_Lean_Parser_Tactic___aux__Init__Tactics______macroRules__Lean__Parser__Tactic__tacticAdmit__1___closed__2;
 x_70 = lean_alloc_ctor(1, 3, 0);
 lean_ctor_set(x_70, 0, x_30);
 lean_ctor_set(x_70, 1, x_69);
@@ -20106,7 +20107,7 @@ lean_inc(x_71);
 x_85 = lean_alloc_ctor(2, 2, 0);
 lean_ctor_set(x_85, 0, x_71);
 lean_ctor_set(x_85, 1, x_84);
-x_86 = l_Lean_Parser_Tactic___aux__Init__Tactics______macroRules__Lean__Parser__Tactic__tacticNext___x3d_x3e____1___closed__1;
+x_86 = l_Lean_Parser_Tactic___aux__Init__Tactics______macroRules__Lean__Parser__Tactic__tacticNext___x3d_x3e____1___closed__5;
 x_87 = lean_array_push(x_86, x_85);
 x_88 = lean_box(2);
 x_89 = l_tacticGet__elem__tactic___closed__2;
@@ -20124,7 +20125,7 @@ lean_ctor_set(x_96, 0, x_88);
 lean_ctor_set(x_96, 1, x_95);
 lean_ctor_set(x_96, 2, x_94);
 x_97 = lean_array_push(x_86, x_96);
-x_98 = l_Lean_Parser_Tactic___aux__Init__Tactics______macroRules__Lean__Parser__Tactic__tacticNext___x3d_x3e____1___closed__3;
+x_98 = l_Lean_Parser_Tactic___aux__Init__Tactics______macroRules__Lean__Parser__Tactic__tacticNext___x3d_x3e____1___closed__7;
 x_99 = lean_alloc_ctor(1, 3, 0);
 lean_ctor_set(x_99, 0, x_88);
 lean_ctor_set(x_99, 1, x_98);
@@ -20176,7 +20177,7 @@ lean_ctor_set(x_124, 1, x_98);
 lean_ctor_set(x_124, 2, x_123);
 x_125 = lean_array_push(x_91, x_79);
 x_126 = lean_array_push(x_125, x_124);
-x_127 = l_Lean_Parser_Tactic___aux__Init__Tactics______macroRules__Lean__Parser__Tactic__tacticAdmit__1___closed__4;
+x_127 = l_Lean_Parser_Tactic___aux__Init__Tactics______macroRules__Lean__Parser__Tactic__tacticAdmit__1___closed__2;
 x_128 = lean_alloc_ctor(1, 3, 0);
 lean_ctor_set(x_128, 0, x_88);
 lean_ctor_set(x_128, 1, x_127);
@@ -20412,7 +20413,7 @@ x_25 = lean_array_push(x_24, x_9);
 x_26 = lean_array_push(x_25, x_11);
 x_27 = lean_array_push(x_26, x_13);
 x_28 = lean_box(2);
-x_29 = l_Lean_Parser_Tactic___aux__Init__Tactics______macroRules__Lean__Parser__Tactic__tacticNext___x3d_x3e____1___closed__3;
+x_29 = l_Lean_Parser_Tactic___aux__Init__Tactics______macroRules__Lean__Parser__Tactic__tacticNext___x3d_x3e____1___closed__7;
 x_30 = lean_alloc_ctor(1, 3, 0);
 lean_ctor_set(x_30, 0, x_28);
 lean_ctor_set(x_30, 1, x_29);
@@ -20420,7 +20421,7 @@ lean_ctor_set(x_30, 2, x_27);
 x_31 = l_Lean_Parser_Tactic___aux__Init__Tactics______macroRules__Lean__Parser__Tactic__tacticTry____1___closed__4;
 x_32 = lean_array_push(x_31, x_23);
 x_33 = lean_array_push(x_32, x_30);
-x_34 = l_Lean_Parser_Tactic___aux__Init__Tactics______macroRules__Lean__Parser__Tactic__tacticAdmit__1___closed__4;
+x_34 = l_Lean_Parser_Tactic___aux__Init__Tactics______macroRules__Lean__Parser__Tactic__tacticAdmit__1___closed__2;
 x_35 = lean_alloc_ctor(1, 3, 0);
 lean_ctor_set(x_35, 0, x_28);
 lean_ctor_set(x_35, 1, x_34);
@@ -20455,7 +20456,7 @@ x_46 = lean_array_push(x_45, x_9);
 x_47 = lean_array_push(x_46, x_11);
 x_48 = lean_array_push(x_47, x_13);
 x_49 = lean_box(2);
-x_50 = l_Lean_Parser_Tactic___aux__Init__Tactics______macroRules__Lean__Parser__Tactic__tacticNext___x3d_x3e____1___closed__3;
+x_50 = l_Lean_Parser_Tactic___aux__Init__Tactics______macroRules__Lean__Parser__Tactic__tacticNext___x3d_x3e____1___closed__7;
 x_51 = lean_alloc_ctor(1, 3, 0);
 lean_ctor_set(x_51, 0, x_49);
 lean_ctor_set(x_51, 1, x_50);
@@ -20463,7 +20464,7 @@ lean_ctor_set(x_51, 2, x_48);
 x_52 = l_Lean_Parser_Tactic___aux__Init__Tactics______macroRules__Lean__Parser__Tactic__tacticTry____1___closed__4;
 x_53 = lean_array_push(x_52, x_44);
 x_54 = lean_array_push(x_53, x_51);
-x_55 = l_Lean_Parser_Tactic___aux__Init__Tactics______macroRules__Lean__Parser__Tactic__tacticAdmit__1___closed__4;
+x_55 = l_Lean_Parser_Tactic___aux__Init__Tactics______macroRules__Lean__Parser__Tactic__tacticAdmit__1___closed__2;
 x_56 = lean_alloc_ctor(1, 3, 0);
 lean_ctor_set(x_56, 0, x_49);
 lean_ctor_set(x_56, 1, x_55);
@@ -20511,6 +20512,8 @@ l_Lean_binderIdent___closed__12 = _init_l_Lean_binderIdent___closed__12();
 lean_mark_persistent(l_Lean_binderIdent___closed__12);
 l_Lean_binderIdent___closed__13 = _init_l_Lean_binderIdent___closed__13();
 lean_mark_persistent(l_Lean_binderIdent___closed__13);
+l_Lean_binderIdent___closed__14 = _init_l_Lean_binderIdent___closed__14();
+lean_mark_persistent(l_Lean_binderIdent___closed__14);
 l_Lean_binderIdent = _init_l_Lean_binderIdent();
 lean_mark_persistent(l_Lean_binderIdent);
 l_Lean_Parser_Tactic_withAnnotateState___closed__1 = _init_l_Lean_Parser_Tactic_withAnnotateState___closed__1();
@@ -20873,6 +20876,14 @@ l_Lean_Parser_Tactic___aux__Init__Tactics______macroRules__Lean__Parser__Tactic_
 lean_mark_persistent(l_Lean_Parser_Tactic___aux__Init__Tactics______macroRules__Lean__Parser__Tactic__tacticNext___x3d_x3e____1___closed__5);
 l_Lean_Parser_Tactic___aux__Init__Tactics______macroRules__Lean__Parser__Tactic__tacticNext___x3d_x3e____1___closed__6 = _init_l_Lean_Parser_Tactic___aux__Init__Tactics______macroRules__Lean__Parser__Tactic__tacticNext___x3d_x3e____1___closed__6();
 lean_mark_persistent(l_Lean_Parser_Tactic___aux__Init__Tactics______macroRules__Lean__Parser__Tactic__tacticNext___x3d_x3e____1___closed__6);
+l_Lean_Parser_Tactic___aux__Init__Tactics______macroRules__Lean__Parser__Tactic__tacticNext___x3d_x3e____1___closed__7 = _init_l_Lean_Parser_Tactic___aux__Init__Tactics______macroRules__Lean__Parser__Tactic__tacticNext___x3d_x3e____1___closed__7();
+lean_mark_persistent(l_Lean_Parser_Tactic___aux__Init__Tactics______macroRules__Lean__Parser__Tactic__tacticNext___x3d_x3e____1___closed__7);
+l_Lean_Parser_Tactic___aux__Init__Tactics______macroRules__Lean__Parser__Tactic__tacticNext___x3d_x3e____1___closed__8 = _init_l_Lean_Parser_Tactic___aux__Init__Tactics______macroRules__Lean__Parser__Tactic__tacticNext___x3d_x3e____1___closed__8();
+lean_mark_persistent(l_Lean_Parser_Tactic___aux__Init__Tactics______macroRules__Lean__Parser__Tactic__tacticNext___x3d_x3e____1___closed__8);
+l_Lean_Parser_Tactic___aux__Init__Tactics______macroRules__Lean__Parser__Tactic__tacticNext___x3d_x3e____1___closed__9 = _init_l_Lean_Parser_Tactic___aux__Init__Tactics______macroRules__Lean__Parser__Tactic__tacticNext___x3d_x3e____1___closed__9();
+lean_mark_persistent(l_Lean_Parser_Tactic___aux__Init__Tactics______macroRules__Lean__Parser__Tactic__tacticNext___x3d_x3e____1___closed__9);
+l_Lean_Parser_Tactic___aux__Init__Tactics______macroRules__Lean__Parser__Tactic__tacticNext___x3d_x3e____1___closed__10 = _init_l_Lean_Parser_Tactic___aux__Init__Tactics______macroRules__Lean__Parser__Tactic__tacticNext___x3d_x3e____1___closed__10();
+lean_mark_persistent(l_Lean_Parser_Tactic___aux__Init__Tactics______macroRules__Lean__Parser__Tactic__tacticNext___x3d_x3e____1___closed__10);
 l_Lean_Parser_Tactic_allGoals___closed__1 = _init_l_Lean_Parser_Tactic_allGoals___closed__1();
 lean_mark_persistent(l_Lean_Parser_Tactic_allGoals___closed__1);
 l_Lean_Parser_Tactic_allGoals___closed__2 = _init_l_Lean_Parser_Tactic_allGoals___closed__2();
@@ -21285,14 +21296,6 @@ l_Lean_Parser_Tactic___aux__Init__Tactics______macroRules__Lean__Parser__Tactic_
 lean_mark_persistent(l_Lean_Parser_Tactic___aux__Init__Tactics______macroRules__Lean__Parser__Tactic__tacticAdmit__1___closed__18);
 l_Lean_Parser_Tactic___aux__Init__Tactics______macroRules__Lean__Parser__Tactic__tacticAdmit__1___closed__19 = _init_l_Lean_Parser_Tactic___aux__Init__Tactics______macroRules__Lean__Parser__Tactic__tacticAdmit__1___closed__19();
 lean_mark_persistent(l_Lean_Parser_Tactic___aux__Init__Tactics______macroRules__Lean__Parser__Tactic__tacticAdmit__1___closed__19);
-l_Lean_Parser_Tactic___aux__Init__Tactics______macroRules__Lean__Parser__Tactic__tacticAdmit__1___closed__20 = _init_l_Lean_Parser_Tactic___aux__Init__Tactics______macroRules__Lean__Parser__Tactic__tacticAdmit__1___closed__20();
-lean_mark_persistent(l_Lean_Parser_Tactic___aux__Init__Tactics______macroRules__Lean__Parser__Tactic__tacticAdmit__1___closed__20);
-l_Lean_Parser_Tactic___aux__Init__Tactics______macroRules__Lean__Parser__Tactic__tacticAdmit__1___closed__21 = _init_l_Lean_Parser_Tactic___aux__Init__Tactics______macroRules__Lean__Parser__Tactic__tacticAdmit__1___closed__21();
-lean_mark_persistent(l_Lean_Parser_Tactic___aux__Init__Tactics______macroRules__Lean__Parser__Tactic__tacticAdmit__1___closed__21);
-l_Lean_Parser_Tactic___aux__Init__Tactics______macroRules__Lean__Parser__Tactic__tacticAdmit__1___closed__22 = _init_l_Lean_Parser_Tactic___aux__Init__Tactics______macroRules__Lean__Parser__Tactic__tacticAdmit__1___closed__22();
-lean_mark_persistent(l_Lean_Parser_Tactic___aux__Init__Tactics______macroRules__Lean__Parser__Tactic__tacticAdmit__1___closed__22);
-l_Lean_Parser_Tactic___aux__Init__Tactics______macroRules__Lean__Parser__Tactic__tacticAdmit__1___closed__23 = _init_l_Lean_Parser_Tactic___aux__Init__Tactics______macroRules__Lean__Parser__Tactic__tacticAdmit__1___closed__23();
-lean_mark_persistent(l_Lean_Parser_Tactic___aux__Init__Tactics______macroRules__Lean__Parser__Tactic__tacticAdmit__1___closed__23);
 l_Lean_Parser_Tactic_tacticSorry___closed__1 = _init_l_Lean_Parser_Tactic_tacticSorry___closed__1();
 lean_mark_persistent(l_Lean_Parser_Tactic_tacticSorry___closed__1);
 l_Lean_Parser_Tactic_tacticSorry___closed__2 = _init_l_Lean_Parser_Tactic_tacticSorry___closed__2();
@@ -22105,10 +22108,6 @@ l_Lean_Parser_Tactic_inductionAlt___closed__16 = _init_l_Lean_Parser_Tactic_indu
 lean_mark_persistent(l_Lean_Parser_Tactic_inductionAlt___closed__16);
 l_Lean_Parser_Tactic_inductionAlt___closed__17 = _init_l_Lean_Parser_Tactic_inductionAlt___closed__17();
 lean_mark_persistent(l_Lean_Parser_Tactic_inductionAlt___closed__17);
-l_Lean_Parser_Tactic_inductionAlt___closed__18 = _init_l_Lean_Parser_Tactic_inductionAlt___closed__18();
-lean_mark_persistent(l_Lean_Parser_Tactic_inductionAlt___closed__18);
-l_Lean_Parser_Tactic_inductionAlt___closed__19 = _init_l_Lean_Parser_Tactic_inductionAlt___closed__19();
-lean_mark_persistent(l_Lean_Parser_Tactic_inductionAlt___closed__19);
 l_Lean_Parser_Tactic_inductionAlt = _init_l_Lean_Parser_Tactic_inductionAlt();
 lean_mark_persistent(l_Lean_Parser_Tactic_inductionAlt);
 l_Lean_Parser_Tactic_inductionAlts___closed__1 = _init_l_Lean_Parser_Tactic_inductionAlts___closed__1();
